@prefix cas:   <http://www.broker-cloud.eu/service-descriptions/CAS/broker#> .
@prefix vann:  <http://purl.org/vocab/vann/> .
@prefix usdl-pref: <http://www.linked-usdl.org/ns/usdl-pref#> .
@prefix pref-att: <http://www.brokeratcloud.eu/v1/opt/SERVICE-ATTRIBUTE/> .
@prefix org:   <http://www.w3.org/ns/org#> .
@prefix dcterms: <http://purl.org/dc/terms/> .
@prefix cpp-fld-profile: <http://www.brokeratcloud.eu/v1/opt/CONSUMER-PREFERENCE-PROFILE/> .
@prefix rdfs:  <http://www.w3.org/2000/01/rdf-schema#> .
@prefix time:  <http://www.w3.org/2006/time#> .
@prefix bp:    <http://guide.broker-cloud.eu/esocc2015#> .
@prefix ctag:  <http://commontag.org/ns#> .
@prefix rdf:   <http://www.w3.org/1999/02/22-rdf-syntax-ns#> .
@prefix usdl-core-cb: <http://www.linked-usdl.org/ns/usdl-core/cloud-broker> .
@prefix cpp-profile: <http://www.brokeratcloud.eu/v1/opt/CONSUMER-PREFERENCE-PROFILE#> .
@prefix usdl-sla: <http://www.linked-usdl.org/ns/usdl-sla#> .
@prefix dc:    <http://purl.org/dc/elements/1.1/> .
@prefix usdl-testing: <http://www.linked-usdl.org/ns/usdl-core/cloud-broker/testing#> .
@prefix cpp-pref: <http://www.brokeratcloud.eu/v1/opt/CONSUMER-PREFERENCE#> .
@prefix foaf:  <http://xmlns.com/foaf/0.1/> .
@prefix sp:    <http://www.broker-cloud.eu/service-descriptions/CAS/service-provider#> .
@prefix usdl-business-roles: <http://www.linked-usdl.org/ns/usdl-business-roles#> .
@prefix att:   <http://www.brokeratcloud.eu/v1/opt/SERVICE-ATTRIBUTE#> .
@prefix xml:   <http://www.w3.org/XML/1998/namespace> .
@prefix attr:  <http://www.brokeratcloud.eu/v1/opt/SERVICE-ATTRIBUTE#> .
@prefix msm:   <http://iserve.kmi.open.ac.uk/ns/msm#> .
@prefix vcard: <http://www.w3.org/TR/vcard-rdf/> .
@prefix usdl-core: <http://www.linked-usdl.org/ns/usdl-core#> .
@prefix fc:    <http://www.broker-cloud.eu/service-descriptions/CAS/categories#> .
@prefix cpp-fld-expr: <http://www.brokeratcloud.eu/v1/opt/CONSUMER-PREFERENCE-EXPRESSION/> .
@prefix s:     <http://schema.org/> .
@prefix cpp-fld-pref: <http://www.brokeratcloud.eu/v1/opt/CONSUMER-PREFERENCE/> .
@prefix xsd:   <http://www.w3.org/2001/XMLSchema#> .
@prefix owl:   <http://www.w3.org/2002/07/owl#> .
@prefix usdl-sla-cb: <http://www.linked-usdl.org/ns/usdl-core/cloud-broker#> .
@prefix pulsar: <http://www.brokeratcloud.eu/persist/types#> .
@prefix blueprint: <http://bizweb.sap.com/TR/blueprint#> .
@prefix gr:    <http://purl.org/goodrelations/v1#> .
@prefix doap:  <http://usefulinc.com/ns/doap#> .
@prefix skos:  <http://www.w3.org/2004/02/skos/core#> .
@prefix cpp-expr: <http://www.brokeratcloud.eu/v1/opt/CONSUMER-PREFERENCE-EXPRESSION#> .
@prefix cas-pref-att: <http://www.broker-cloud.eu/service-descriptions/CAS/broker-pref-attr#> .

attr:attr-performance-capacity-network-throughput
        a                    usdl-pref:ServiceAttribute ;
        dcterms:created      "2014-07-18T14:59:00+03:00"^^xsd:dateTime ;
        dcterms:description  ""^^xsd:string ;
        dcterms:identifier   "attr-performance-capacity-network-throughput"^^xsd:string ;
        dcterms:modified     "2014-07-18T14:59:00+03:00"^^xsd:dateTime ;
        dcterms:title        "Network Throughput"^^xsd:string ;
        skos:broader         attr:attr-performance-capacity .

<http://www.linked-usdl.org/ns/machine-to-human>
        a                usdl-core:InteractionType ;
        rdfs:label       "Machine to Human"@en ;
        skos:altLabel    "Machine to Human Interaction"@en ;
        skos:broader     <http://www.linked-usdl.org/ns/semi-automated> ;
        skos:definition  "<p>The interaction between the two parties is semi-automated. It is triggered by a machine and processed manually.</p>"@en ;
        skos:inScheme    <http://www.linked-usdl.org/ns/usdl-interaction-types> ;
        skos:prefLabel   "Machine to Human"@en .

gr:DeliveryModePickUp
        a                 gr:DeliveryMethod ;
        rdfs:comment      "Delivery of the goods by picking them up at one of the stores etc. (gr:Location) during the opening hours as specified by respective instances of gr:OpeningHoursSpecification."@en ;
        rdfs:isDefinedBy  <http://purl.org/goodrelations/v1> ;
        rdfs:label        "Delivery mode pick up (delivery method)"@en .

usdl-core:Service  a      owl:Class , rdfs:Class ;
        rdfs:comment      "<p>A Service is a 'black box' description of a service for the purpose of describing the service in a way that the information can help consumers in deciding which services are more suited for their needs. The description contains functional properties of the service, described by the interaction protocol as well as non-functional properties described by qualitative or quantitative values. Any composite implementation of a service that is internal is invisible to consumers and not captured by the specification. The support of complex service compositions can be described using supplemental service network vocabularies, which are beyond the Linked USDL Core vocabulary (we foresee the introduction of a network vocabulary in the near future).</p>"@en ;
        rdfs:isDefinedBy  <http://www.linked-usdl.org/ns/usdl-core> ;
        rdfs:label        "Service"@en ;
        rdfs:subClassOf   gr:ProductOrService .

attr:attr-performance-capacity-swap-disc
        a                    usdl-pref:ServiceAttribute ;
        dcterms:created      "2015-09-08T10:40:25.768+03:00"^^xsd:dateTime ;
        dcterms:description  "Amount of space on the hard disc used as a virtual memory extension as computers main memory"^^xsd:string ;
        dcterms:identifier   "attr-performance-capacity-swap-disc"^^xsd:string ;
        dcterms:modified     "2015-09-08T10:40:25.768+03:00"^^xsd:dateTime ;
        dcterms:title        "Swap Disc"^^xsd:string ;
        skos:broader         attr:attr-performance-capacity .

gr:includesObject  a      owl:ObjectProperty ;
        rdfs:comment      "This object property links a gr:Offering to one or multiple gr:TypeAndQuantityNode or nodes that specify the components that are included in the respective offer."@en ;
        rdfs:domain       [ a            owl:Class ;
                            owl:unionOf  ( gr:Offering s:Offer )
                          ] ;
        rdfs:isDefinedBy  <http://purl.org/goodrelations/v1> ;
        rdfs:label        "includes object (0..*)"@en ;
        rdfs:range        gr:TypeAndQuantityNode .

gr:Thursday  a              gr:DayOfWeek ;
        rdfs:comment        "Thursday as a day of the week."@en ;
        rdfs:isDefinedBy    <http://purl.org/goodrelations/v1> ;
        rdfs:label          "Thursday (day of week)"@en ;
        gr:displayPosition  4 ;
        gr:hasNext          gr:Friday ;
        gr:hasPrevious      gr:Wednesday .

usdl-testing:TestGenerationStrategy
        a                 owl:Class , rdfs:Class ;
        rdfs:comment      "<p> Test Generation Strategy serves as a root class for a taxonomy providing vocabulary for classification of the test generation strategy of a testing method. </p>"@en ;
        rdfs:isDefinedBy  <http://www.linked-usdl.org/ns/usdl-core/cloud-broker/testing> ;
        rdfs:label        "Test Generation Strategy"@en ;
        rdfs:subClassOf   skos:Concept .

attr:attr-assurance-availability
        a                    usdl-pref:ServiceAttribute ;
        dcterms:created      "2014-05-23T21:27:57+03:00"^^xsd:dateTime ;
        dcterms:description  "The amount of time that a client can make use of a service"^^xsd:string ;
        dcterms:identifier   "attr-assurance-availability"^^xsd:string ;
        dcterms:modified     "2014-07-18T11:48:14+03:00"^^xsd:dateTime ;
        dcterms:title        "Availability"^^xsd:string ;
        skos:broader         attr:attr-assurance .

usdl-sla-cb:higherIsBetter
        a                 rdf:Property ;
        rdfs:comment      "<p>Indicates if a higher value corresponds to a better value of the utility function, e.g., 99% availability is better than 95%. True means higher is better. False means lower is better. </p>"@en ;
        rdfs:domain       gr:QuantitativeValue ;
        rdfs:isDefinedBy  usdl-core-cb: ;
        rdfs:label        "interpretation direction of a quantitative value range as a utility function"@en ;
        rdfs:range        xsd:boolean .

gr:QuantitativeValueInteger
        a                 owl:Class ;
        rdfs:comment      "An instance of this class is an actual integer value for a quantitative property of a product. This instance is usually characterized by a minimal value, a maximal value, and a unit of measurement. \n\nExample: A seating capacity between 1 and 8 persons.\n\nNote: Users must keep in mind that ranges in here mean that ALL possible values in this interval are covered. (Sometimes, the actual commitment may be less than that: \"We sell cars from 2 - 12 seats\" does often not really mean that they have cars with 2,3,4,...12 seats.). Someone renting out two types of rowing boats, one that fits for 1 or 2 people, and another that must be operated by 4 people cannot claim to rent boats with a seating capacity between 1 and 4 people. He or she is offering two boat types for 1-2 and 4 persons.\n\t\t\nCompatibility with schema.org: This class is a subclass of http://schema.org/Quantity."@en ;
        rdfs:isDefinedBy  <http://purl.org/goodrelations/v1> ;
        rdfs:label        "Quantitative value integer"@en ;
        rdfs:subClassOf   gr:QuantitativeValue ;
        owl:disjointWith  gr:QuantitativeValueFloat .

usdl-core:jcardoso  a  foaf:Person ;
        foaf:homepage  <http://eden.dei.uc.pt/~jcardoso/> ;
        foaf:name      "Jorge Cardoso" .

usdl-core-cb:  a                       owl:Ontology ;
        rdfs:label                     "Linked USDL SLA Cloud Broker"@en , "Linked USDL Core Cloud Broker"@en ;
        dcterms:created                "2014-09-30"^^xsd:date ;
        dcterms:creator                usdl-sla-cb:afriesen ;
        dcterms:description            "<p>This vocabulary provides a Broker@Cloud extension to the core module of Linked USDL required by the optimization mechanism. It introduces a root class for multi-dimensional classification taxonomies and provides a specification for fuzzy values .</p>"@en , "<p>This vocabulary provides a Broker@Cloud extension to the SLA module of Linked USDL. It introduces properties allowing to use not only quantitative but also qualitative and fuzzy values in SLA specifications .</p>"@en ;
        dcterms:issued                 "2014-09-30"^^xsd:date ;
        dcterms:modified               "2014-09-30"^^xsd:date ;
        dcterms:title                  "Linked USDL SLA Cloud Broker"@en , "Linked USDL Core Cloud Broker"@en ;
        vann:preferredNamespacePrefix  "usdl-core-cb" ;
        vann:preferredNamespaceUri     "http://www.linked-usdl.org/ns/usdl-core/cloud-broker#" ;
        owl:versionInfo                "1.0" .

gr:seeks  a               owl:ObjectProperty ;
        rdfs:comment      "This links a gr:BusinessEntity to gr:Offering nodes that describe what the business entity is interested in (i.e., the buy side). If you want to express interest in offering something, use gr:offers instead. Note that this substitutes the former gr:BusinessFunction gr:Buy, which is now deprecated."@en ;
        rdfs:domain       [ a            owl:Class ;
                            owl:unionOf  ( gr:BusinessEntity s:Organization s:Person )
                          ] ;
        rdfs:isDefinedBy  <http://purl.org/goodrelations/v1> ;
        rdfs:label        "seeks (0..*)"@en ;
        rdfs:range        gr:Offering .

attr:attr-assurance-service-stability-uptime
        a                    usdl-pref:ServiceAttribute ;
        dcterms:created      "2014-05-23T21:29:02+03:00"^^xsd:dateTime ;
        dcterms:description  ""^^xsd:string ;
        dcterms:identifier   "attr-assurance-service-stability-uptime"^^xsd:string ;
        dcterms:modified     "2014-07-18T11:55:15+03:00"^^xsd:dateTime ;
        dcterms:title        "Uptime"^^xsd:string ;
        skos:broader         attr:attr-assurance-service-stability .

gr:qualitativeProductOrServiceProperty
        a                 owl:ObjectProperty ;
        rdfs:comment      "This is the super property of all qualitative properties for products and services. All properties in product or service ontologies for which gr:QualitativeValue instances are specified are subproperties of this property."@en ;
        rdfs:domain       [ a            owl:Class ;
                            owl:unionOf  ( gr:ProductOrService s:Product )
                          ] ;
        rdfs:isDefinedBy  <http://purl.org/goodrelations/v1> ;
        rdfs:label        "qualitative product or service property (0..*)"@en ;
        rdfs:range        gr:QualitativeValue .

attr:attr-security-data-integrity
        a                    usdl-pref:ServiceAttribute ;
        dcterms:created      "2014-07-18T12:53:07Z"^^xsd:dateTime ;
        dcterms:creator      ""^^xsd:string ;
        dcterms:description  "Keeping the data that is created, used, and stored in its correct form so that clients may be confident that it is accurate and valid"^^xsd:string ;
        dcterms:identifier   "attr-security-data-integrity"^^xsd:string ;
        dcterms:modified     "2014-07-18T12:53:07Z"^^xsd:dateTime ;
        dcterms:title        "Data Integrity"^^xsd:string ;
        skos:broader         attr:attr-security .

gr:eligibleTransactionVolume
        a                 owl:ObjectProperty ;
        rdfs:comment      "This property can be used to indicate the transaction volume, in a monetary unit, for which the gr:Offering or gr:PriceSpecification is valid. This is mostly used to specify a minimal purchasing volume, to express free shipping above a certain order volume, or to limit the acceptance of credit cards to purchases above a certain amount.\n\nThe object is a gr:PriceSpecification that uses the properties gr:hasMaxCurrencyValue and gr:hasMinCurrencyValue to indicate the lower and upper boundaries and gr:hasCurrency to indicate the currency using the ISO 4217 standard (3 characters)."@en ;
        rdfs:domain       [ a            owl:Class ;
                            owl:unionOf  ( gr:Offering gr:PriceSpecification s:Offer )
                          ] ;
        rdfs:isDefinedBy  <http://purl.org/goodrelations/v1> ;
        rdfs:label        "eligible transaction volume (0..1)"@en ;
        rdfs:range        gr:PriceSpecification .

attr:attr-assurance-recoverability
        a                    usdl-pref:ServiceAttribute ;
        dcterms:created      "2014-07-18T08:48:56Z"^^xsd:dateTime ;
        dcterms:creator      ""^^xsd:string ;
        dcterms:description  "It is the degree to which a service is able to quickly resume a normal state of operation after an unplanned disruption"^^xsd:string ;
        dcterms:identifier   "attr-assurance-recoverability"^^xsd:string ;
        dcterms:modified     "2014-07-18T08:48:56Z"^^xsd:dateTime ;
        dcterms:title        "Recoverability"^^xsd:string ;
        skos:broader         attr:attr-assurance .

usdl-pref:belongsTo  a    rdf:Property ;
        rdfs:comment      "<p> Associating optimisation attributes with any of the available service dimensions for which they are meaningful. </p>\r\n" ;
        rdfs:domain       usdl-pref:PreferenceVariable ;
        rdfs:isDefinedBy  <http://www.linked-usdl.org/ns/usdl-pref> ;
        rdfs:label        "belongs to" ;
        rdfs:range        usdl-sla-cb:ClassificationDimension .

gr:Monday  a                gr:DayOfWeek ;
        rdfs:comment        "Monday as a day of the week."@en ;
        rdfs:isDefinedBy    <http://purl.org/goodrelations/v1> ;
        rdfs:label          "Monday (day of week)"@en ;
        gr:displayPosition  1 ;
        gr:hasNext          gr:Tuesday ;
        gr:hasPrevious      gr:Sunday .

usdl-sla-cb:ClassificationDimension
        a                 owl:Class , rdfs:Class ;
        rdfs:comment      "<p>Classification Dimension serves as a root class for platform-specific taxonomies providing vocabularies for classification of services according to different aspects (dimensions) available for classification on a cloud service brokerage platform according to Broker@Cloud methodology. This class is used by the optimization mechanism developed in the Broker@Cloud project for identification of applicable taxonomies.</p>"@en ;
        rdfs:isDefinedBy  usdl-core-cb: ;
        rdfs:label        "Classification Dimension"@en ;
        rdfs:subClassOf   skos:Concept .

usdl-sla-cb:hasMinKernel
        a                   rdf:Property ;
        rdfs:comment        "<p>Indicates a min kernel.</p>"@en ;
        rdfs:domain         usdl-sla-cb:FuzzyValue ;
        rdfs:isDefinedBy    usdl-core-cb: ;
        rdfs:label          "has min kernel"@en ;
        rdfs:range          xsd:float ;
        rdfs:subPropertyOf  gr:hasMinValueFloat .

gr:hasOpeningHoursSpecification
        a                 owl:ObjectProperty ;
        rdfs:comment      "This property links a gr:Location to a gr:OpeningHoursSpecification."@en ;
        rdfs:domain       [ a            owl:Class ;
                            owl:unionOf  ( gr:Location s:Place )
                          ] ;
        rdfs:isDefinedBy  <http://purl.org/goodrelations/v1> ;
        rdfs:label        "has opening hours specification (0..*)"@en ;
        rdfs:range        gr:OpeningHoursSpecification .

attr:attr-agility-robustness
        a                    usdl-pref:ServiceAttribute ;
        dcterms:created      "2014-07-18T08:47:23Z"^^xsd:dateTime ;
        dcterms:creator      ""^^xsd:string ;
        dcterms:description  "Refers to the extent to which a service keeps working even in the presence of inconsistent or incomplete data"^^xsd:string ;
        dcterms:identifier   "attr-agility-robustness"^^xsd:string ;
        dcterms:modified     "2014-07-18T08:47:23Z"^^xsd:dateTime ;
        dcterms:title        "Robustness"^^xsd:string ;
        skos:broader         attr:attr-agility .

attr:attr-performance-monitoring
        a                    usdl-pref:ServiceAttribute ;
        dcterms:created      "2014-07-18T12:05:46Z"^^xsd:dateTime ;
        dcterms:creator      ""^^xsd:string ;
        dcterms:description  "It indicates how much the monitoring capability is supported regarding the offered cloud services"^^xsd:string ;
        dcterms:identifier   "attr-performance-monitoring"^^xsd:string ;
        dcterms:modified     "2014-07-18T12:05:46Z"^^xsd:dateTime ;
        dcterms:title        "Monitoring"^^xsd:string ;
        skos:broader         attr:attr-performance .

gr:datatypeProductOrServiceProperty
        a                 owl:DatatypeProperty ;
        rdfs:comment      "This property is the super property for all pure datatype properties that can be used to describe a gr:ProductOrService.\n\nIn products and services ontologies, only such properties that are no quantitative properties and that have no predefined gr:QualitativeValue instances are subproperties of this property. In practice, this refers to a few integer properties for which the integer value represents qualitative aspects, for string datatypes (as long as no predefined values exist), for boolean datatype properties, and for dates and times."@en ;
        rdfs:domain       [ a            owl:Class ;
                            owl:unionOf  ( gr:ProductOrService s:Product )
                          ] ;
        rdfs:isDefinedBy  <http://purl.org/goodrelations/v1> ;
        rdfs:label        "datatype product or service property (0..*)"@en ;
        rdfs:range        rdfs:Literal .

attr:attr-usability-learnability
        a                    usdl-pref:ServiceAttribute ;
        dcterms:created      "2014-07-18T16:23:48+03:00"^^xsd:dateTime ;
        dcterms:description  "The effort required of users to learn to use the service"^^xsd:string ;
        dcterms:identifier   "attr-usability-learnability"^^xsd:string ;
        dcterms:modified     "2014-07-18T16:23:48+03:00"^^xsd:dateTime ;
        dcterms:title        "Learnability"^^xsd:string ;
        skos:broader         attr:attr-usability .

attr:attr-security-access-control-privilege-management-authentication-schemes
        a                    usdl-pref:ServiceAttribute ;
        dcterms:created      "2014-07-18T12:51:22Z"^^xsd:dateTime ;
        dcterms:creator      ""^^xsd:string ;
        dcterms:description  ""^^xsd:string ;
        dcterms:identifier   "attr-security-access-control-privilege-management-authentication-schemes"^^xsd:string ;
        dcterms:modified     "2014-07-18T12:51:22Z"^^xsd:dateTime ;
        dcterms:title        "Supported authentication schemes"^^xsd:string ;
        skos:broader         attr:attr-security-access-control-privilege-management .

attr:attr-accountability-personnel-requirements
        a                    usdl-pref:ServiceAttribute ;
        dcterms:created      "2014-07-18T07:36:10Z"^^xsd:dateTime ;
        dcterms:creator      ""^^xsd:string ;
        dcterms:description  "The extent to which service provider personnel have the skills, experience, education, and certifications required to effectively deliver a service"^^xsd:string ;
        dcterms:identifier   "attr-accountability-personnel-requirements"^^xsd:string ;
        dcterms:modified     "2014-07-18T07:36:10Z"^^xsd:dateTime ;
        dcterms:title        "Provider Personnel Requirements"^^xsd:string ;
        skos:broader         attr:attr-accountability .

attr:attr-accountability-contract-sla-verification
        a                    usdl-pref:ServiceAttribute ;
        dcterms:created      "2014-07-18T07:35:43Z"^^xsd:dateTime ;
        dcterms:creator      ""^^xsd:string ;
        dcterms:description  "The service provider makes available to clients SLAs adequate to manage the service and mitigate risks of service failure"^^xsd:string ;
        dcterms:identifier   "attr-accountability-contract-sla-verification"^^xsd:string ;
        dcterms:modified     "2014-07-18T07:35:43Z"^^xsd:dateTime ;
        dcterms:title        "Provider Contract/SLA Verification"^^xsd:string ;
        skos:broader         attr:attr-accountability .

gr:Tuesday  a               gr:DayOfWeek ;
        rdfs:comment        "Tuesday as a day of the week."@en ;
        rdfs:isDefinedBy    <http://purl.org/goodrelations/v1> ;
        rdfs:label          "Tuesday (day of week)"@en ;
        gr:displayPosition  2 ;
        gr:hasNext          gr:Wednesday ;
        gr:hasPrevious      gr:Monday .

attr:attr-agility-elasticity
        a                    usdl-pref:ServiceAttribute ;
        dcterms:created      "2014-05-23T18:24:03Z"^^xsd:dateTime ;
        dcterms:creator      ""^^xsd:string ;
        dcterms:description  "The ability of a service to adjust its resource consumption to meet demand"^^xsd:string ;
        dcterms:identifier   "attr-agility-elasticity"^^xsd:string ;
        dcterms:modified     "2014-07-18T08:13:32Z"^^xsd:dateTime ;
        dcterms:title        "Elasticity"^^xsd:string ;
        skos:broader         attr:attr-agility .

usdl-testing:TestingFocusClassificationScheme
        a                    skos:ConceptScheme ;
        dcterms:description  "<p>This vocabulary provides the concepts to classify testing focus dimension. </p>"@en ;
        dcterms:title        "Testing Focus classification concept scheme" ;
        skos:hasTopConcept   usdl-testing:AcceptanceTesting , usdl-testing:NonFunctionalTesting , usdl-testing:FunctionalTesting ;
        skos:prefLabel       "Testing Focus Classification"@en .

usdl-testing:hasAdequacy
        a                 rdf:Property ;
        rdfs:comment      "<p>Connects TestingMethod to TestAdequacyCriteria classification dimension.</p>"@en ;
        rdfs:domain       usdl-testing:TestingMethod ;
        rdfs:isDefinedBy  <http://www.linked-usdl.org/ns/usdl-core/cloud-broker/testing> ;
        rdfs:label        "has adequacy"@en ;
        rdfs:range        usdl-testing:TestAdequacyCriteria .

gr:DeliveryModeMail  a    gr:DeliveryMethod ;
        rdfs:comment      "Delivery via regular mail service (private or public postal services)."@en ;
        rdfs:isDefinedBy  <http://purl.org/goodrelations/v1> ;
        rdfs:label        "Delivery mode mail (delivery method)"@en .

<http://www.linked-usdl.org/ns/usdl-pref#SAP%20SE>
        a              foaf:Organization ;
        foaf:homepage  <http://www.sap.com> ;
        foaf:member    usdl-pref:afriesen ;
        foaf:name      "SAP SE" .

gr:legalName  a           owl:DatatypeProperty ;
        rdfs:comment      "The legal name of the gr:BusinessEntity."@en ;
        rdfs:domain       [ a            owl:Class ;
                            owl:unionOf  ( gr:BusinessEntity s:Organization )
                          ] ;
        rdfs:isDefinedBy  <http://purl.org/goodrelations/v1> ;
        rdfs:label        "legal name (0..1)"@en ;
        rdfs:range        rdfs:Literal .

gr:DeliveryModeFreight
        a                 gr:DeliveryMethod ;
        rdfs:comment      "Delivery by an unspecified air, sea, or ground freight carrier or cargo company."@en ;
        rdfs:isDefinedBy  <http://purl.org/goodrelations/v1> ;
        rdfs:label        "Delivery mode freight (delivery method)"@en .

gr:CheckInAdvance  a      gr:PaymentMethod ;
        rdfs:comment      "Payment by sending a check in advance, i.e., the offering gr:BusinessEntity will deliver the goods upon receipt of a check over the due amount. There are variations in handling payment by check - sometimes, shipment will be upon receipt of the check as a document, sometimes the shipment will take place only upon successful crediting of the check."@en ;
        rdfs:isDefinedBy  <http://purl.org/goodrelations/v1> ;
        rdfs:label        "Check in advance (payment method)"@en .

usdl-testing:TestingFocus
        a                 owl:Class , rdfs:Class ;
        rdfs:comment      "<p> Testing Focus serves as a root class for a taxonomy providing vocabulary for classification of the testing focus of a testing method. </p>"@en ;
        rdfs:isDefinedBy  <http://www.linked-usdl.org/ns/usdl-core/cloud-broker/testing> ;
        rdfs:label        "Testing Focus"@en ;
        rdfs:subClassOf   skos:Concept .

attr:attr-assurance-serviceability-documentation
        a                    usdl-pref:ServiceAttribute ;
        dcterms:created      "2014-05-23T21:30:49+03:00"^^xsd:dateTime ;
        dcterms:description  ""^^xsd:string ;
        dcterms:identifier   "attr-assurance-serviceability-documentation"^^xsd:string ;
        dcterms:modified     "2014-07-18T12:13:51+03:00"^^xsd:dateTime ;
        dcterms:title        "Documentation"^^xsd:string ;
        skos:broader         attr:attr-assurance-serviceability .

gr:hasMaxCurrencyValue
        a                 owl:DatatypeProperty ;
        rdfs:comment      "This property specifies the UPPER BOUND of the amount of money for a price RANGE per unit, shipping charges, or payment charges. The currency and other relevant details are attached to the respective gr:PriceSpecification etc.\nFor a gr:UnitPriceSpecification, this is the UPPER BOUND for the price for one unit or bundle (as specified in the unit of measurement of the unit price specification) of the respective gr:ProductOrService. For a gr:DeliveryChargeSpecification or a gr:PaymentChargeSpecification, it is the UPPER BOUND of the price per delivery or payment.\n\nUsing gr:hasCurrencyValue sets the upper and lower bounds to the same given value, i.e., x gr:hasCurrencyValue y implies x gr:hasMinCurrencyValue y, x gr:hasMaxCurrencyValue y."@en ;
        rdfs:domain       gr:PriceSpecification ;
        rdfs:isDefinedBy  <http://purl.org/goodrelations/v1> ;
        rdfs:label        "has max currency value (1..1)"@en ;
        rdfs:range        xsd:float .

gr:QuantitativeValueFloat
        a                 owl:Class ;
        rdfs:comment      "An instance of this class is an actual float value for a quantitative property of a product. This instance is usually characterized by a minimal value, a maximal value, and a unit of measurement.\n\nExamples: The intervals \"between 10.0  and 25.4 kilogramms\" or \"10.2 and 15.5 milimeters\".\n\nCompatibility with schema.org: This class is a subclass of http://schema.org/Quantity."@en ;
        rdfs:isDefinedBy  <http://purl.org/goodrelations/v1> ;
        rdfs:label        "Quantitative value float"@en ;
        rdfs:subClassOf   gr:QuantitativeValue ;
        owl:disjointWith  gr:QuantitativeValueInteger .

gr:Cash  a                gr:PaymentMethod ;
        rdfs:comment      "Payment by cash upon delivery or pickup."@en ;
        rdfs:isDefinedBy  <http://purl.org/goodrelations/v1> ;
        rdfs:label        "Cash (payment method)"@en .

gr:displayPosition  a     owl:AnnotationProperty ;
        rdfs:comment      "The position at which the option or element should be listed in a menu or user dialog, lower numbers come first.\n\nThe main usage of this property are the days of the week (gr:DayOfWeek), but it is also possible to apply it e.g. to product features or any other conceptual element.\nNote: Rely on this property only for data originating from a single RDF graph; otherwise, unpredictable results are possible."@en ;
        rdfs:isDefinedBy  <http://purl.org/goodrelations/v1> ;
        rdfs:label        "display position (0..1)"@en .

gr:Sunday  a                gr:DayOfWeek ;
        rdfs:comment        "Sunday as a day of the week."@en ;
        rdfs:isDefinedBy    <http://purl.org/goodrelations/v1> ;
        rdfs:label          "Sunday (day of week)"@en ;
        gr:displayPosition  7 ;
        gr:hasNext          gr:Monday ;
        gr:hasPrevious      gr:Saturday .

gr:successorOf  a         owl:TransitiveProperty , owl:ObjectProperty ;
        rdfs:comment      "This property indicates that the subject is a newer, often updated or improved variant of the gr:ProductOrServiceModel used as the object.\n\nExample: Golf III successorOf Golf II\n\nThis relation is transitive."@en ;
        rdfs:domain       gr:ProductOrServiceModel ;
        rdfs:isDefinedBy  <http://purl.org/goodrelations/v1> ;
        rdfs:label        "successor of (0..*)"@en ;
        rdfs:range        gr:ProductOrServiceModel ;
        owl:inverseOf     gr:predecessorOf .

s:Place  a                   owl:Class ;
        owl:equivalentClass  gr:Location .

attr:attr-security-proactive-threat-vulnerability-management-security-level
        a                    usdl-pref:ServiceAttribute ;
        dcterms:created      "2015-09-08T10:41:29.655+03:00"^^xsd:dateTime ;
        dcterms:description  "Defines the protection level of the virtual machine instance, which is applied by the IaaS networking controller"^^xsd:string ;
        dcterms:identifier   "attr-security-proactive-threat-vulnerability-management-security-level"^^xsd:string ;
        dcterms:modified     "2015-09-08T10:41:29.655+03:00"^^xsd:dateTime ;
        dcterms:title        "Security Level"^^xsd:string ;
        skos:broader         attr:attr-security-proactive-threat-vulnerability-management .

attr:attr-accountability-auditability
        a                    usdl-pref:ServiceAttribute ;
        dcterms:created      "2014-07-18T07:29:34Z"^^xsd:dateTime ;
        dcterms:creator      ""^^xsd:string ;
        dcterms:description  "The ability of a client to verify that the service provider is adhering to the standards, processes, and policies that they follow"^^xsd:string ;
        dcterms:identifier   "attr-accountability-auditability"^^xsd:string ;
        dcterms:modified     "2014-07-18T07:29:34Z"^^xsd:dateTime ;
        dcterms:title        "Auditability"^^xsd:string ;
        skos:broader         attr:attr-accountability .

gr:QuantitativeValue  a   owl:Class ;
        rdfs:comment      "A quantitative value is a numerical interval that represents the range of a certain gr:quantitativeProductOrServiceProperty in terms of the lower and upper bounds for a particular gr:ProductOrService. It is to be interpreted in combination with the respective unit of measurement. Most quantitative values are intervals even if they are in practice often treated as a single point value.\n\t\nExample: a weight between 10 and 25 kilogramms, a length between 10 and 15 milimeters.\n\nCompatibility with schema.org: This class is equivalent to http://schema.org/Quantity."@en ;
        rdfs:isDefinedBy  <http://purl.org/goodrelations/v1> ;
        rdfs:label        "Quantitative value"@en ;
        owl:disjointWith  gr:Location , gr:DeliveryMethod , gr:BusinessEntity , gr:WarrantyPromise , gr:PriceSpecification , gr:BusinessEntityType , gr:PaymentMethod , gr:TypeAndQuantityNode , gr:Brand , gr:OpeningHoursSpecification , gr:Offering , gr:QualitativeValue , gr:ProductOrService , gr:BusinessFunction , gr:DayOfWeek , gr:WarrantyScope .

<http://www.linked-usdl.org/ns/initiator>
        a                usdl-core:InteractionRole ;
        rdfs:label       "initiator"@en ;
        skos:broader     <http://www.linked-usdl.org/ns/participant> ;
        skos:definition  "<p>An Initiator within an Interaction is the entity that should initiate the interaction.</p>"@en ;
        skos:inScheme    <http://www.linked-usdl.org/ns/usdl-interaction-roles> ;
        skos:prefLabel   "initiator"@en .

attr:attr-financial-billing-process
        a                    usdl-pref:ServiceAttribute ;
        dcterms:created      "2014-07-18T09:23:02Z"^^xsd:dateTime ;
        dcterms:creator      ""^^xsd:string ;
        dcterms:description  "The level of integration that is available between the client and cloud service provider's billing systems and the predictability of periodic bills"^^xsd:string ;
        dcterms:identifier   "attr-financial-billing-process"^^xsd:string ;
        dcterms:modified     "2014-07-18T09:23:02Z"^^xsd:dateTime ;
        dcterms:title        "Billing Process"^^xsd:string ;
        skos:broader         attr:attr-financial .

gr:hasInventoryLevel  a   owl:ObjectProperty ;
        rdfs:comment      "This property specifies the current approximate inventory level for gr:SomeItems. The unit of measurement and the point value or interval are indicated using the attached gr:QuantitativeValueFloat instance.\n\nThis property can also be attached to a gr:Offering in cases where the included products are not modeled in more detail."@en ;
        rdfs:domain       [ a            owl:Class ;
                            owl:unionOf  ( gr:Offering gr:SomeItems s:Offer )
                          ] ;
        rdfs:isDefinedBy  <http://purl.org/goodrelations/v1> ;
        rdfs:label        "has inventory level (0..1)"@en ;
        rdfs:range        gr:QuantitativeValueFloat .

gr:hasWarrantyScope  a    owl:ObjectProperty ;
        rdfs:comment      "This states the gr:WarrantyScope of a given gr:WarrantyPromise."@en ;
        rdfs:domain       gr:WarrantyPromise ;
        rdfs:isDefinedBy  <http://purl.org/goodrelations/v1> ;
        rdfs:label        "has warranty scope (0..1)"@en ;
        rdfs:range        gr:WarrantyScope .

attr:attr-accountability-certifications
        a                    usdl-pref:ServiceAttribute ;
        dcterms:created      "2014-07-18T07:35:05Z"^^xsd:dateTime ;
        dcterms:creator      ""^^xsd:string ;
        dcterms:description  "The service provider maintains current certifications for standards relevant to their clients' requirements"^^xsd:string ;
        dcterms:identifier   "attr-accountability-certifications"^^xsd:string ;
        dcterms:modified     "2014-07-18T07:35:05Z"^^xsd:dateTime ;
        dcterms:title        "Provider Certifications"^^xsd:string ;
        skos:broader         attr:attr-accountability .

usdl-core:BusinessRole
        a                 owl:Class , rdfs:Class ;
        rdfs:comment      "<p>The BusinessRoles that an entity may play within a service delivery chain (e.g., Provider). One may define as many roles as necessary by defining subclasses of BusinessRole or by creating SKOS concept schemes. For completeness Linked USDL Core provides a basic concept scheme for these roles that can be used out of the box or as reference for specific extensions. See Linked USDL Business Roles Module.</p>"@en ;
        rdfs:isDefinedBy  <http://www.linked-usdl.org/ns/usdl-core> ;
        rdfs:label        "Business Role"@en ;
        rdfs:subClassOf   usdl-core:Role .

attr:attr-financial-cost-storage
        a                    usdl-pref:ServiceAttribute ;
        dcterms:created      "2014-05-23T18:32:46Z"^^xsd:dateTime ;
        dcterms:description  ""^^xsd:string ;
        dcterms:identifier   "attr-financial-cost-storage"^^xsd:string ;
        dcterms:modified     "2014-05-23T18:32:46Z"^^xsd:dateTime ;
        dcterms:title        "Storage"^^xsd:string ;
        skos:broader         attr:attr-financial-cost .

<http://www.linked-usdl.org/ns/receiver>
        a                usdl-core:InteractionRole ;
        rdfs:label       "receiver"@en ;
        skos:broader     <http://www.linked-usdl.org/ns/participant> ;
        skos:definition  "<p>A Receiver is the final destination of a given interaction. Once an interaction has reacher the receiver, the interaction is considered to be concluded.</p>"@en ;
        skos:inScheme    <http://www.linked-usdl.org/ns/usdl-interaction-roles> ;
        skos:prefLabel   "receiver"@en .

gr:hasMinValue  a         owl:DatatypeProperty ;
        rdfs:comment      "This property captures the lower limit of a gr:QuantitativeValue instance."@en ;
        rdfs:domain       gr:QuantitativeValue ;
        rdfs:isDefinedBy  <http://purl.org/goodrelations/v1> ;
        rdfs:label        "has min value (0..1)"@en ;
        rdfs:range        rdfs:Literal .

gr:hasCurrency  a         owl:DatatypeProperty ;
        rdfs:comment      "The currency for all prices in the gr:PriceSpecification given using the ISO 4217 standard (3 characters)."@en ;
        rdfs:domain       gr:PriceSpecification ;
        rdfs:isDefinedBy  <http://purl.org/goodrelations/v1> ;
        rdfs:label        "has currency (1..1)"@en ;
        rdfs:range        xsd:string .

gr:offers  a              owl:ObjectProperty ;
        rdfs:comment      "This links a gr:BusinessEntity to the offers (gr:Offering) it makes. If you want to express interest in receiving offers, use gr:seeks instead."@en ;
        rdfs:domain       [ a            owl:Class ;
                            owl:unionOf  ( gr:BusinessEntity s:Organization )
                          ] ;
        rdfs:isDefinedBy  <http://purl.org/goodrelations/v1> ;
        rdfs:label        "offers (0..*)"@en ;
        rdfs:range        gr:Offering .

usdl-testing:RandomTesting
        a                  usdl-testing:TestGenerationStrategy ;
        rdfs:label         "Random Testing"@en ;
        skos:altLabel      "Random Testing"@en ;
        skos:definition    "<p>A testing method is a random testing method.</p>"@en ;
        skos:inScheme      usdl-testing:TestGenerationStrategyClassificationScheme ;
        skos:prefLabel     "Random Testing"@en ;
        skos:topConceptOf  usdl-testing:TestGenerationStrategyClassificationScheme .

s:image  a                      owl:ObjectProperty ;
        owl:equivalentProperty  foaf:depiction .

usdl-sla-cb:SAP-Karlsruhe
        a              foaf:Organization ;
        foaf:homepage  <http://www.sap.com> ;
        foaf:member    usdl-sla-cb:afriesen ;
        foaf:name      "SAP Research Center Karlsruhe, SAP SE" .

<http://www.linked-usdl.org/ns/semi-automated>
        a                  usdl-core:InteractionType ;
        rdfs:label         "Semi-Automated"@en ;
        skos:altLabel      "Semi-Automated Interaction"@en ;
        skos:definition    "<p>The interaction between the two parties is semi-automated.</p>"@en ;
        skos:inScheme      <http://www.linked-usdl.org/ns/usdl-interaction-types> ;
        skos:narrower      <http://www.linked-usdl.org/ns/machine-to-human> , <http://www.linked-usdl.org/ns/human-to-machine> ;
        skos:prefLabel     "Semi-Automated"@en ;
        skos:topConceptOf  <http://www.linked-usdl.org/ns/usdl-interaction-types> .

usdl-core:ServiceModel
        a                 owl:Class , rdfs:Class ;
        rdfs:comment      "<p>A ServiceModel is used to represent 'classes' of services, i.e. services that share a number of characteristics.  ServiceModel enables the capturing of these characteristics.</p>"@en ;
        rdfs:isDefinedBy  <http://www.linked-usdl.org/ns/usdl-core> ;
        rdfs:label        "Service Model"@en ;
        rdfs:subClassOf   gr:ProductOrServiceModel , usdl-core:Service .

usdl-testing:CodeBasedTesting
        a                  usdl-testing:TestAdequacyCriteria ;
        rdfs:label         "Code-based Testing"@en ;
        skos:altLabel      "Code-based Testing"@en ;
        skos:definition    "<p>A testing method is a code-based testing method.</p>"@en ;
        skos:inScheme      usdl-testing:TestAdequacyCriteriaClassificationScheme ;
        skos:prefLabel     "Code-based Testing"@en ;
        skos:topConceptOf  usdl-testing:TestAdequacyCriteriaClassificationScheme .

attr:attr-assurance-maintainability
        a                    usdl-pref:ServiceAttribute ;
        dcterms:created      "2014-07-18T08:48:37Z"^^xsd:dateTime ;
        dcterms:creator      ""^^xsd:string ;
        dcterms:description  "It refers to the ability for the service provider to make modifications to the service to keep the service in a condition of good repair"^^xsd:string ;
        dcterms:identifier   "attr-assurance-maintainability"^^xsd:string ;
        dcterms:modified     "2014-07-18T08:48:37Z"^^xsd:dateTime ;
        dcterms:title        "Maintainability"^^xsd:string ;
        skos:broader         attr:attr-assurance .

gr:equal  a               owl:TransitiveProperty , owl:SymmetricProperty , owl:ObjectProperty ;
        rdfs:comment      "This ordering relation for qualitative values indicates that the subject is equal to the object."@en ;
        rdfs:domain       gr:QualitativeValue ;
        rdfs:isDefinedBy  <http://purl.org/goodrelations/v1> ;
        rdfs:label        "equal (0..*)"@en ;
        rdfs:range        gr:QualitativeValue ;
        owl:inverseOf     gr:equal .

usdl-testing:SAP-Karlsruhe
        a              foaf:Organization ;
        foaf:homepage  <http://www.sap.com> ;
        foaf:member    usdl-testing:afriesen ;
        foaf:name      "SAP Research Center Karlsruhe, SAP SE" .

usdl-core:hasInteractionPoint
        a                 rdf:Property ;
        rdfs:comment      "<p>Interactions that are part of the interaction protocol.</p>"@en ;
        rdfs:domain       [ a            owl:Class ;
                            owl:unionOf  ( usdl-core:Service usdl-core:ServiceModel )
                          ] ;
        rdfs:isDefinedBy  <http://www.linked-usdl.org/ns/usdl-core> ;
        rdfs:label        "has interaction"@en ;
        rdfs:range        usdl-core:InteractionPoint .

gr:hasBusinessFunction
        a                 owl:ObjectProperty ;
        rdfs:comment      "This specifies the business function of the gr:Offering, i.e. whether the gr:BusinessEntity is offering to sell, to lease, or to repair the particular type of product. In the case of bundles, it is also possible to attach individual business functions to each gr:TypeAndQuantityNode. The business function of the main gr:Offering determines the business function for all included objects or services, unless a business function attached to a gr:TypeAndQuantityNode overrides it.\n\t\nNote: While it is possible that an entity is offering multiple types of business functions for the same set of objects (e.g. rental and sales), this should usually not be stated by attaching multiple business functions to the same gr:Offering, since the gr:UnitPriceSpecification for the varying business functions will typically be very different."@en ;
        rdfs:domain       [ a            owl:Class ;
                            owl:unionOf  ( gr:Offering gr:TypeAndQuantityNode s:Offer )
                          ] ;
        rdfs:isDefinedBy  <http://purl.org/goodrelations/v1> ;
        rdfs:label        "has business function (1..*)"@en ;
        rdfs:range        gr:BusinessFunction .

gr:ByInvoice  a           gr:PaymentMethod ;
        rdfs:comment      "Payment by bank transfer after delivery, i.e., the offering gr:BusinessEntity will deliver first, inform the buying party about the due amount and their bank account details, and expect payment shortly after delivery."@en ;
        rdfs:isDefinedBy  <http://purl.org/goodrelations/v1> ;
        rdfs:label        "By invoice (payment method)"@en .

gr:Sell  a                gr:BusinessFunction ;
        rdfs:comment      "This gr:BusinessFunction indicates that the gr:BusinessEntity offers to permanently transfer all property rights on the specified gr:ProductOrService."@en ;
        rdfs:isDefinedBy  <http://purl.org/goodrelations/v1> ;
        rdfs:label        "Sell (business function)"@en .

gr:deliveryLeadTime  a    owl:ObjectProperty ;
        rdfs:comment      "This property can be used to indicate the promised delay between the receipt of the order and the goods leaving the warehouse.\n\nThe duration is specified by attaching an instance of gr:QuantitativeValueInteger. The lower and upper boundaries are specified using the properties gr:hasMinValueInteger and gr:hasMaxValueInteger to that instance. A point value can be modeled with the gr:hasValueInteger property. The unit of measurement is specified using the property gr:hasUnitOfMeasurement with a string holding a UN/CEFACT code suitable for durations, e.g. MON (months), DAY (days), HUR (hours), or MIN (minutes)."@en ;
        rdfs:domain       [ a            owl:Class ;
                            owl:unionOf  ( gr:Offering s:Offer )
                          ] ;
        rdfs:isDefinedBy  <http://purl.org/goodrelations/v1> ;
        rdfs:label        "delivery lead time (0..1)"@en ;
        rdfs:range        gr:QuantitativeValueInteger .

usdl-testing:SystematicTesting
        a                  usdl-testing:TestGenerationStrategy ;
        rdfs:label         "Systematic Testing"@en ;
        skos:altLabel      "Systematic Testing"@en ;
        skos:definition    "<p>A testing method is a systematic testing method.</p>"@en ;
        skos:inScheme      usdl-testing:TestGenerationStrategyClassificationScheme ;
        skos:prefLabel     "Systematic Testing"@en ;
        skos:topConceptOf  usdl-testing:TestGenerationStrategyClassificationScheme .

gr:greaterOrEqual  a      owl:TransitiveProperty , owl:ObjectProperty ;
        rdfs:comment      "This ordering relation for qualitative values indicates that the subject is greater than or equal to the object."@en ;
        rdfs:domain       gr:QualitativeValue ;
        rdfs:isDefinedBy  <http://purl.org/goodrelations/v1> ;
        rdfs:label        "greater or equal (0..*)"@en ;
        rdfs:range        gr:QualitativeValue ;
        owl:inverseOf     gr:lesserOrEqual .

gr:BusinessEntityType
        a                 owl:Class ;
        rdfs:comment      "A business entity type is a conceptual entity representing the legal form, the size, the main line of business, the position in the value chain, or any combination thereof, of a gr:BusinessEntity. From the ontological point of view, business entity types are mostly roles that a business entity has in the market. Business entity types are important for specifying eligible customers, since a gr:Offering is often valid only for business entities of a certain size, legal structure, or role in the value chain. \n\nExamples: Consumers, Retailers, Wholesalers, or Public Institutions"@en ;
        rdfs:isDefinedBy  <http://purl.org/goodrelations/v1> ;
        rdfs:label        "Business entity type"@en ;
        owl:disjointWith  gr:BusinessFunction , gr:PriceSpecification , gr:OpeningHoursSpecification , gr:Brand , gr:WarrantyScope , gr:DeliveryMethod , gr:BusinessEntity , gr:Offering , gr:TypeAndQuantityNode , gr:PaymentMethod , gr:QuantitativeValue , gr:Location , gr:DayOfWeek , gr:WarrantyPromise , gr:ProductOrService .

gr:WarrantyScope  a       owl:Class ;
        rdfs:comment      "The warranty scope represents types of services that will be provided free of charge by the vendor or manufacturer in the case of a defect (e.g. labor and parts, just parts), as part of the warranty included in an gr:Offering. The actual services may be provided by the gr:BusinessEntity making the offering, by the manufacturer of the product, or by a third party. \n\nExamples: Parts and Labor, Parts"@en ;
        rdfs:isDefinedBy  <http://purl.org/goodrelations/v1> ;
        rdfs:label        "Warranty scope"@en ;
        owl:disjointWith  gr:DeliveryMethod , gr:WarrantyPromise , gr:BusinessEntityType , gr:PaymentMethod , gr:Brand , gr:BusinessFunction , gr:Location , gr:BusinessEntity , gr:TypeAndQuantityNode , gr:QuantitativeValue , gr:PriceSpecification , gr:ProductOrService , gr:OpeningHoursSpecification , gr:DayOfWeek , gr:Offering .

<http://www.linked-usdl.org/ns/by-automation>
        a               skos:Collection ;
        skos:member     <http://www.linked-usdl.org/ns/automated> , <http://www.linked-usdl.org/ns/semi-automated> , <http://www.linked-usdl.org/ns/manual> ;
        skos:prefLabel  "<p>Interaction Types by level of Automation"@en .

s:Product  a                 owl:Class ;
        owl:equivalentClass  gr:ProductOrService .

attr:attr-accountability-supply-chain
        a                    usdl-pref:ServiceAttribute ;
        dcterms:created      "2014-07-18T08:10:41Z"^^xsd:dateTime ;
        dcterms:creator      ""^^xsd:string ;
        dcterms:description  "The service provider ensures that any SLAs that must be supported by its suppliers are supported"^^xsd:string ;
        dcterms:identifier   "attr-accountability-supply-chain"^^xsd:string ;
        dcterms:modified     "2014-07-18T08:10:41Z"^^xsd:dateTime ;
        dcterms:title        "Provider Supply Chain"^^xsd:string ;
        skos:broader         attr:attr-accountability .

attr:attr-financial-cost-data-outbound
        a                    usdl-pref:ServiceAttribute ;
        dcterms:created      "2014-05-23T18:32:35Z"^^xsd:dateTime ;
        dcterms:creator      ""^^xsd:string ;
        dcterms:description  ""^^xsd:string ;
        dcterms:identifier   "attr-financial-cost-data-outbound"^^xsd:string ;
        dcterms:modified     "2014-07-18T09:25:36Z"^^xsd:dateTime ;
        dcterms:title        "Data - Outbound"^^xsd:string ;
        skos:broader         attr:attr-financial-cost .

foaf:depiction  a  owl:ObjectProperty .

gr:closes  a              owl:DatatypeProperty ;
        rdfs:comment      "The closing  hour of the gr:Location on the given gr:DayOfWeek.\nIf no time-zone suffix is included, the time is given in the local time valid at the gr:Location.\n\nFor a time in GMT/UTC, simply add a \"Z\" following the time:\n\n09:30:10Z.\n\nAlternatively, you can specify an offset from the UTC time by adding a positive or negative time following the time:\n\n09:30:10-09:00\n\n09:30:10+09:00.\n\nNote 1: Use 00:00:00 for the first second of the respective day and 23:59:59 for the last second of that day.\nNote 2: If a store opens at 17:00 on Saturdays and closes at 03:00:00 a.m. next morning, use two instances of this class, one with 17:00:00 - 23:59:59 for Saturday and another one with 00:00:00 - 03:00:00 for Sunday.\nNote 3: If the shop re-opens on the same day of the week or set of days of the week, you must create a second instance of gr:OpeningHoursSpecification."@en ;
        rdfs:domain       gr:OpeningHoursSpecification ;
        rdfs:isDefinedBy  <http://purl.org/goodrelations/v1> ;
        rdfs:label        "closes (1..1)"@en ;
        rdfs:range        xsd:time .

usdl-pref:refToServiceAttribute
        a                 rdf:Property ;
        rdfs:comment      "<p>Optimization attribute for a preference variable.</p>\r\n" ;
        rdfs:domain       usdl-pref:PreferenceVariable ;
        rdfs:isDefinedBy  <http://www.linked-usdl.org/ns/usdl-pref> ;
        rdfs:label        "ref to optimization attribute" ;
        rdfs:range        usdl-pref:ServiceAttribute .

usdl-testing:hasModel
        a                 rdf:Property ;
        rdfs:comment      "<p>Connects TestingMethod to a resource containing method-specific model for the specification of testing instructions.</p>"@en ;
        rdfs:domain       usdl-testing:TestingMethod ;
        rdfs:isDefinedBy  <http://www.linked-usdl.org/ns/usdl-core/cloud-broker/testing> ;
        rdfs:label        "has model"@en ;
        rdfs:range        rdfs:Resource .

gr:nonEqual  a            owl:SymmetricProperty , owl:ObjectProperty ;
        rdfs:comment      "This ordering relation for gr:QualitativeValue pairs indicates that the subject is not equal to the object."@en ;
        rdfs:domain       gr:QualitativeValue ;
        rdfs:isDefinedBy  <http://purl.org/goodrelations/v1> ;
        rdfs:label        "non equal (0..*)"@en ;
        rdfs:range        gr:QualitativeValue ;
        owl:inverseOf     gr:nonEqual .

gr:SomeItems  a              owl:Class ;
        rdfs:comment         "A placeholder instance for unknown instances of a mass-produced commodity. This is used as a computationally cheap work-around for such instances that are not individually exposed on the Web but just stated to exist (i.e., which are existentially quantified).\n\nExample: An instance of this class can represent an anonymous set of green Siemens1234 phones. It is different from the gr:ProductOrServiceModel Siemens1234, since this refers to the make and model, and it is different from a particular instance of this make and model (e.g. my individual phone) since the latter can be sold only once.\n\nNote: This class is the new, shorter form of the former gr:ProductOrServicesSomeInstancesPlaceholder.\n\t\t\nCompatibility with schema.org: This class is (approximately) a subclass of http://schema.org/Product."@en ;
        rdfs:isDefinedBy     <http://purl.org/goodrelations/v1> ;
        rdfs:label           "Some items"@en ;
        rdfs:subClassOf      s:Product , gr:ProductOrService ;
        owl:disjointWith     gr:ProductOrServiceModel , gr:Individual ;
        owl:equivalentClass  gr:ProductOrServicesSomeInstancesPlaceholder .

attr:attr-reputation-sustainability-carbon-footprint
        a                    usdl-pref:ServiceAttribute ;
        dcterms:created      "2014-07-18T13:35:43Z"^^xsd:dateTime ;
        dcterms:creator      ""^^xsd:string ;
        dcterms:description  ""^^xsd:string ;
        dcterms:identifier   "attr-reputation-sustainability-carbon-footprint"^^xsd:string ;
        dcterms:modified     "2014-07-18T13:35:43Z"^^xsd:dateTime ;
        dcterms:title        "Carbon footprint"^^xsd:string ;
        skos:broader         attr:attr-reputation-sustainability .

gr:hasMakeAndModel  a     owl:ObjectProperty ;
        rdfs:comment      "This states that an actual product instance (gr:Individual) or a placeholder instance for multiple, unidentified such instances (gr:SomeItems) is one occurence of a particular gr:ProductOrServiceModel.\n\nExample: myFordT hasMakeAndModel FordT."@en ;
        rdfs:domain       [ a            owl:Class ;
                            owl:unionOf  ( gr:Individual gr:SomeItems s:Product )
                          ] ;
        rdfs:isDefinedBy  <http://purl.org/goodrelations/v1> ;
        rdfs:label        "has make and model (0..1)"@en ;
        rdfs:range        gr:ProductOrServiceModel .

gr:GoogleCheckout  a      gr:PaymentMethod ;
        rdfs:comment      "Payment via the Google Checkout payment service."@en ;
        rdfs:isDefinedBy  <http://purl.org/goodrelations/v1> ;
        rdfs:label        "Google Checkout (payment method)"@en .

usdl-core:InteractionPoint
        a                 owl:Class , rdfs:Class ;
        rdfs:comment      "<p>An InteractionPoint represents an actual step in accessing and performing operations of the service. On a technical level this could translate into calling a Web Service operation. \r\nOn a professional level, it could mean that consumer and provider meet in person to exchange service parameters or resources involved in the service delivery (e.g. documents that are processed by the provider). \r\nAn InteractionPoint can be initiated by the consumer or the provider. Since InteractionPoints may take time and have an ordering with respect to other InteractionPoints, this is a subclass of TimeSpanningEntity.\r\nOne can therefore express temporal relationships between InteractionPoints such as before or after. For richer expressions the time ontology constructs could be used.</p>"@en ;
        rdfs:isDefinedBy  <http://www.linked-usdl.org/ns/usdl-core> ;
        rdfs:label        "Interaction Point"@en .

gr:weight  a                owl:ObjectProperty ;
        rdfs:comment        "The weight of the gr:ProductOrService.\nTypical unit code(s): GRM for gram, KGM for kilogram, LBR for pound"@en ;
        rdfs:domain         [ a            owl:Class ;
                              owl:unionOf  ( gr:ProductOrService s:Product )
                            ] ;
        rdfs:isDefinedBy    <http://purl.org/goodrelations/v1> ;
        rdfs:label          "weight (0..1)"@en ;
        rdfs:range          gr:QuantitativeValue ;
        rdfs:subPropertyOf  gr:quantitativeProductOrServiceProperty .

usdl-pref:FuzzyVariable
        a                 owl:Class , rdfs:Class ;
        rdfs:comment      "<p> A FuzzyVariable is used to reference a fuzzy value.</p> " ;
        rdfs:isDefinedBy  <http://www.linked-usdl.org/ns/usdl-pref> ;
        rdfs:label        "Fuzzy Variable" ;
        rdfs:subClassOf   usdl-pref:PreferenceVariable .

<http://www.linked-usdl.org/ns/intermediary>
        a                  usdl-core:BusinessRole ;
        rdfs:label         "Intermediary"@en ;
        skos:definition    "<p>An Intermediary is a third party entity that is involved in the actual service delivery chain. This may be a subcontractor, a broker, etc. Tracking this information allows one to know the entities involved in an entire chain.</p>"@en ;
        skos:inScheme      <http://www.linked-usdl.org/ns/usdl-business-roles> ;
        skos:prefLabel     "Intermediary"@en ;
        skos:topConceptOf  <http://www.linked-usdl.org/ns/usdl-business-roles> .

attr:attr-usability-operability
        a                    usdl-pref:ServiceAttribute ;
        dcterms:created      "2014-07-18T16:24:11+03:00"^^xsd:dateTime ;
        dcterms:description  "The ability of a service to be easily operated by users"^^xsd:string ;
        dcterms:identifier   "attr-usability-operability"^^xsd:string ;
        dcterms:modified     "2014-07-18T16:24:11+03:00"^^xsd:dateTime ;
        dcterms:title        "Operability"^^xsd:string ;
        skos:broader         attr:attr-usability .

attr:attr-security  a        usdl-pref:ServiceAttribute ;
        dcterms:created      "2014-05-23T21:21:05+03:00"^^xsd:dateTime ;
        dcterms:description  "It indicates the effectiveness of a cloud service provider's controls on access to services, service data, and the physical facilities from which services are provided"^^xsd:string ;
        dcterms:identifier   "attr-security"^^xsd:string ;
        dcterms:modified     "2014-07-18T15:07:41+03:00"^^xsd:dateTime ;
        dcterms:title        "Security and Privacy"^^xsd:string ;
        skos:broader         attr:attr-root .

usdl-core:ofBusinessEntity
        a                 rdf:Property ;
        rdfs:comment      "<p>Captures the BusinessEntity involved in a particular EntityInvolvement or EntityInteraction. For instance the entity involved could be SAP, IBM, Siemens, etc.</p>"@en ;
        rdfs:domain       [ a            owl:Class ;
                            owl:unionOf  ( usdl-core:EntityInvolvement usdl-core:EntityInteraction )
                          ] ;
        rdfs:isDefinedBy  <http://www.linked-usdl.org/ns/usdl-core> ;
        rdfs:label        "of business entity"@en ;
        rdfs:range        gr:BusinessEntity .

usdl-pref:ipatiniotakis
        a          foaf:Person ;
        foaf:name  "Ioannis Patiniotakis" .

gr:Labor-BringIn  a       gr:WarrantyScope ;
        rdfs:comment      "In case of a defect or malfunction, the buying party has the right to transport the good to a service location determined by the the selling gr:BusinessEntity and will be charged only for parts and materials needed to fix the problem. Labor will be covered by the selling business entity or one of its partnering business entities.\n\nNote: This is just a rough classification for filtering offers. It is up to the buying party to check the exact scope and terms and conditions of the gr:WarrantyPromise."@en ;
        rdfs:isDefinedBy  <http://purl.org/goodrelations/v1> ;
        rdfs:label        "Labor / bring-in (warranty scope)"@en .

gr:hasValue  a              owl:DatatypeProperty ;
        rdfs:comment        "This subproperty specifies that the upper and lower limit of the given gr:QuantitativeValue are identical and have the respective value. It is a shortcut for such cases where a quantitative property is (at least practically) a single point value and not an interval."@en ;
        rdfs:domain         gr:QuantitativeValue ;
        rdfs:isDefinedBy    <http://purl.org/goodrelations/v1> ;
        rdfs:label          "has value (0..1)"@en ;
        rdfs:range          rdfs:Literal ;
        rdfs:subPropertyOf  gr:hasMinValue , gr:hasMaxValue .

gr:isListPrice  a         owl:DatatypeProperty ;
        rdfs:comment      "This boolean attribute indicates whether a gr:UnitPriceSpecification is a list price (usually a vendor recommendation) or not. \"true\"  indicates it is a list price, \"false\" indicates it is not.\nDEPRECATED. Use the gr:priceType property instead."@en ;
        rdfs:domain       gr:UnitPriceSpecification ;
        rdfs:isDefinedBy  <http://purl.org/goodrelations/v1> ;
        rdfs:label        "is list price (DEPRECATED)"@en ;
        rdfs:range        xsd:boolean ;
        owl:deprecated    true .

owl:deprecated  a  owl:AnnotationProperty .

gr:availabilityEnds  a    owl:DatatypeProperty ;
        rdfs:comment      "This property specifies the end of the availability of the gr:ProductOrService included in the gr:Offering.\nThe difference to the properties gr:validFrom and gr:validThrough is that those specify the period of time during which the offer is valid and can be accepted.\n\nExample: I offer to lease my boat for the period of August 1 - August 31, 2010, but you must accept by offer no later than July 15.\n\nA time-zone should be specified. For a time in GMT/UTC, simply add a \"Z\" following the time:\n\n2008-05-30T09:30:10Z.\n\nAlternatively, you can specify an offset from the UTC time by adding a positive or negative time following the time:\n\n2008-05-30T09:30:10-09:00\n\nor\n\n2008-05-30T09:30:10+09:00.\n\nNote: There is another property gr:availableAtOrFrom, which is used to indicate the gr:Location (e.g. store or shop) from which the goods would be available."@en ;
        rdfs:domain       [ a            owl:Class ;
                            owl:unionOf  ( gr:Offering s:Offer )
                          ] ;
        rdfs:isDefinedBy  <http://purl.org/goodrelations/v1> ;
        rdfs:label        "availability ends (0..1)"@en ;
        rdfs:range        xsd:dateTime .

[ a               gr:Offering ;
  gr:category     "42" ;
  gr:description  "VGhlIFNldmVuIE5vYWhpZGUgTGF3cw0KMS4gQmVsaWVmIGluIEctZA0KMi4gUmVzcGVjdCBHLWQgYW5kIHByYWlzZSBoaW0NCjMuIFJlc3BlY3QgaHVtYW4gbGlmZQ0KNC4gUmVzcGVjdCB0aGUgZmFtaWx5DQo1LiBSZXNwZWN0IGh1bWFuIGJlaW5ncw0KNi4gSGF2ZSBhIGp1ZGljaWFsIHN5c3RlbQ0KNy4gUmVzcGVjdCBhbGwgY3JlYXR1cmVz"
] .

usdl-testing:TestingGoal
        a                 owl:Class , rdfs:Class ;
        rdfs:comment      "<p> Testing Goal serves as a root class for a taxonomy providing vocabulary for classification of the testing goal of a testing method. </p>"@en ;
        rdfs:isDefinedBy  <http://www.linked-usdl.org/ns/usdl-core/cloud-broker/testing> ;
        rdfs:label        "Testing Goal"@en ;
        rdfs:subClassOf   skos:Concept .

dc:subject  a   owl:AnnotationProperty .

gr:hasGTIN-8  a             owl:DatatypeProperty ;
        rdfs:comment        "The 8-digit Global Trade Item Number (GTIN-8) of the given gr:ProductOrService or gr:Offering, also known as EAN/UCC-8 (8-digit EAN)."@en ;
        rdfs:domain         [ a            owl:Class ;
                              owl:unionOf  ( gr:Offering gr:ProductOrService s:Product )
                            ] ;
        rdfs:isDefinedBy    <http://purl.org/goodrelations/v1> ;
        rdfs:label          "has GTIN-8 (0..*)"@en ;
        rdfs:range          xsd:string ;
        rdfs:subPropertyOf  s:productID .

gr:DeliveryModeParcelService
        a                 owl:Class ;
        rdfs:comment      "A private parcel service as the delivery mode available for a certain offering.\n\nExamples: UPS, DHL"@en ;
        rdfs:isDefinedBy  <http://purl.org/goodrelations/v1> ;
        rdfs:label        "Delivery mode parcel service"@en ;
        rdfs:subClassOf   gr:DeliveryMethod .

attr:attr-root  a            usdl-pref:ServiceAttribute ;
        dcterms:created      "1900-01-01T01:41:48+01:34"^^xsd:dateTime ;
        dcterms:creator      ""^^xsd:string ;
        dcterms:description  "Broker@Cloud Service Attribute Categorization Root"^^xsd:string ;
        dcterms:identifier   "attr-root"^^xsd:string ;
        dcterms:modified     "2014-10-15T19:09:08.613+03:00"^^xsd:dateTime ;
        dcterms:title        "Service Attributes Root (Extended SMI)"^^xsd:string .

gr:DeliveryModeOwnFleet
        a                 gr:DeliveryMethod ;
        rdfs:comment      "Delivery of the goods by using a fleet of vehicles either owned and operated or subcontracted by the gr:BusinessEntity."@en ;
        rdfs:isDefinedBy  <http://purl.org/goodrelations/v1> ;
        rdfs:label        "Delivery mode own fleet (delivery method)"@en .

gr:lesserOrEqual  a       owl:TransitiveProperty , owl:ObjectProperty ;
        rdfs:comment      "This ordering relation for gr:QualitativeValue pairs indicates that the subject is lesser than or equal to the object."@en ;
        rdfs:domain       gr:QualitativeValue ;
        rdfs:isDefinedBy  <http://purl.org/goodrelations/v1> ;
        rdfs:label        "lesser or equal (0..*)"@en ;
        rdfs:range        gr:QualitativeValue ;
        owl:inverseOf     gr:greaterOrEqual .

attr:attr-performance-capacity-memory-speed
        a                    usdl-pref:ServiceAttribute ;
        dcterms:created      "2014-07-18T11:57:47Z"^^xsd:dateTime ;
        dcterms:creator      ""^^xsd:string ;
        dcterms:description  ""^^xsd:string ;
        dcterms:identifier   "attr-performance-capacity-memory-speed"^^xsd:string ;
        dcterms:modified     "2014-07-18T11:57:47Z"^^xsd:dateTime ;
        dcterms:title        "Memory Speed"^^xsd:string ;
        skos:broader         attr:attr-performance-capacity .

gr:PublicHolidays  a        gr:DayOfWeek ;
        rdfs:comment        "A placeholder for all official public holidays at the gr:Location. This allows specifying the opening hours on public holidays. If a given day is a public holiday, this specification supersedes the opening hours for the respective day of the week."@en ;
        rdfs:isDefinedBy    <http://purl.org/goodrelations/v1> ;
        rdfs:label          "Public holidays (day of week)"@en ;
        gr:displayPosition  8 .

gr:DeliveryModeDirectDownload
        a                 gr:DeliveryMethod ;
        rdfs:comment      "Delivery of the goods via direct download from the Internet, i.e., the offering gr:BusinessEntity provides the buying party with details on how to retrieve the goods online. Connection fees and other costs of using the infrastructure are to be carried by the buying party."@en ;
        rdfs:isDefinedBy  <http://purl.org/goodrelations/v1> ;
        rdfs:label        "Delivery mode direct download (delivery method)"@en .

gr:hasPrevious  a         owl:ObjectProperty ;
        rdfs:comment      "This ordering relation for gr:DayOfWeek indicates that the subject is directly preceeded by the object.\n\nExample: Tuesday hasPrevious Monday\n\nSince days of the week are a cycle, this property is not transitive."@en ;
        rdfs:domain       gr:DayOfWeek ;
        rdfs:isDefinedBy  <http://purl.org/goodrelations/v1> ;
        rdfs:label        "has previous (0..1)"@en ;
        rdfs:range        gr:DayOfWeek ;
        owl:inverseOf     gr:hasNext .

gr:greater  a             owl:TransitiveProperty , owl:ObjectProperty ;
        rdfs:comment      "This ordering relation for qualitative values indicates that the subject is greater than the object."@en ;
        rdfs:domain       gr:QualitativeValue ;
        rdfs:isDefinedBy  <http://purl.org/goodrelations/v1> ;
        rdfs:label        "greater (0..*)"@en ;
        rdfs:range        gr:QualitativeValue ;
        owl:inverseOf     gr:lesser .

gr:owns  a                owl:ObjectProperty ;
        rdfs:comment      "This property indicates that a particular person or business owns a particular product. It can be used to expose the products in one's posession in order to empower recommender systems to suggest matching offers.\n\nNote that the product must be an instance of the class gr:Individual.\n\nThis property can also be safely applied to foaf:Agent instances."@en ;
        rdfs:domain       [ a            owl:Class ;
                            owl:unionOf  ( gr:BusinessEntity s:Organization s:Person )
                          ] ;
        rdfs:isDefinedBy  <http://purl.org/goodrelations/v1> ;
        rdfs:label        "owns (0..*)"@en ;
        rdfs:range        gr:Individual .

gr:availableDeliveryMethods
        a                 owl:ObjectProperty ;
        rdfs:comment      "This specifies the gr:DeliveryMethod or methods available for a given gr:Offering."@en ;
        rdfs:domain       [ a            owl:Class ;
                            owl:unionOf  ( gr:Offering s:Offer )
                          ] ;
        rdfs:isDefinedBy  <http://purl.org/goodrelations/v1> ;
        rdfs:label        "available delivery methods (0..*)"@en ;
        rdfs:range        gr:DeliveryMethod .

<http://www.linked-usdl.org/ns/participant>
        a                  usdl-core:InteractionRole ;
        rdfs:label         "participant"@en ;
        skos:definition    "<p>A Participant is an entity that takes active part within a concrete interaction.</p>"@en ;
        skos:inScheme      <http://www.linked-usdl.org/ns/usdl-interaction-roles> ;
        skos:prefLabel     "participant"@en ;
        skos:topConceptOf  <http://www.linked-usdl.org/ns/usdl-interaction-roles> .

attr:attr-performance-suitability
        a                    usdl-pref:ServiceAttribute ;
        dcterms:created      "2014-07-18T12:02:58Z"^^xsd:dateTime ;
        dcterms:creator      ""^^xsd:string ;
        dcterms:description  "How closely do the capabilities of the service match the needs of the client"^^xsd:string ;
        dcterms:identifier   "attr-performance-suitability"^^xsd:string ;
        dcterms:modified     "2014-07-18T12:02:58Z"^^xsd:dateTime ;
        dcterms:title        "Suitability"^^xsd:string ;
        skos:broader         attr:attr-performance .

attr:attr-performance-capacity-ephemeral-disc
        a                    usdl-pref:ServiceAttribute ;
        dcterms:created      "2015-09-08T10:39:50.943+03:00"^^xsd:dateTime ;
        dcterms:description  "Amount of disc space which is operational only if the VM instance is alive"^^xsd:string ;
        dcterms:identifier   "attr-performance-capacity-ephemeral-disc"^^xsd:string ;
        dcterms:modified     "2015-09-08T10:39:50.943+03:00"^^xsd:dateTime ;
        dcterms:title        "Ephemeral Disc"^^xsd:string ;
        skos:broader         attr:attr-performance-capacity .

gr:PaySwarm  a            gr:PaymentMethod ;
        rdfs:comment      "Payment via the PaySwarm distributed micropayment service."@en ;
        rdfs:isDefinedBy  <http://purl.org/goodrelations/v1> ;
        rdfs:label        "PaySwarm (payment method)"@en .

gr:isConsumableFor  a     owl:ObjectProperty ;
        rdfs:comment      "This states that a particular gr:ProductOrService is a consumable for another product or service."@en ;
        rdfs:domain       [ a            owl:Class ;
                            owl:unionOf  ( gr:ProductOrService s:Product )
                          ] ;
        rdfs:isDefinedBy  <http://purl.org/goodrelations/v1> ;
        rdfs:label        "is consumable for (0..*)"@en ;
        rdfs:range        gr:ProductOrService .

usdl-pref:QuantitativeVariable
        a                 owl:Class , rdfs:Class ;
        rdfs:comment      "<p> A QuantitativeVariable is used to reference a quantitative value.</p> " ;
        rdfs:isDefinedBy  <http://www.linked-usdl.org/ns/usdl-pref> ;
        rdfs:label        "Quantitative Variable" ;
        rdfs:subClassOf   usdl-pref:PreferenceVariable .

gr:PartsAndLabor-PickUp
        a                 gr:WarrantyScope ;
        rdfs:comment      "In case of a defect or malfunction, the buying party has the right to request from the selling gr:Business Entity to pick-up the good from its current location to a suitable service location, where the functionality of the good will be restored. All transportation, labor, parts, and materials needed to fix the problem will be covered by the selling business entity or one of its partnering business entities.\n  \nNote: This is just a rough classification for filtering offers. It is up to the buying party to check the exact scope and terms and conditions of the gr:WarrantyPromise."@en ;
        rdfs:isDefinedBy  <http://purl.org/goodrelations/v1> ;
        rdfs:label        "Parts and labor / pick up (warranty scope)"@en .

usdl-testing:StressTesting
        a                  usdl-testing:TestingGoal ;
        rdfs:label         "Stress Testing"@en ;
        skos:altLabel      "Stress Testing"@en ;
        skos:definition    "<p>A testing method is a stress testing method.</p>"@en ;
        skos:inScheme      usdl-testing:TestingGoalClassificationScheme ;
        skos:prefLabel     "Stress Testing"@en ;
        skos:topConceptOf  usdl-testing:TestingGoalClassificationScheme .

usdl-testing:TestAdequacyCriteriaClassificationScheme
        a                    skos:ConceptScheme ;
        dcterms:description  "<p>This vocabulary provides the concepts to classify test adequacy criteria dimension. </p>"@en ;
        dcterms:title        "Test Adequacy Criteria classification concept scheme" ;
        skos:hasTopConcept   usdl-testing:FaultBasedTesting , usdl-testing:CodeBasedTesting , usdl-testing:ModelBasedTesting ;
        skos:prefLabel       "Test Adequacy Criteria Classification"@en .

gr:DinersClub  a          gr:PaymentMethodCreditCard ;
        rdfs:comment      "Payment by credit or debit cards issued by the Diner's Club network."@en ;
        rdfs:isDefinedBy  <http://purl.org/goodrelations/v1> ;
        rdfs:label        "Diners Club (payment method)"@en .

gr:hasMinCurrencyValue
        a                 owl:DatatypeProperty ;
        rdfs:comment      "This property specifies the LOWER BOUND of the amount of money for a price RANGE per unit, shipping charges, or payment charges. The currency and other relevant details are attached to the respective gr:PriceSpecification etc.\nFor a gr:UnitPriceSpecification, this is the LOWER BOUND for the price for one unit or bundle (as specified in the unit of measurement of the unit price specification) of the respective gr:ProductOrService. For a gr:DeliveryChargeSpecification or a gr:PaymentChargeSpecification, it is the LOWER BOUND of the price per delivery or payment.\n\nUsing gr:hasCurrencyValue sets the upper and lower bounds to the same given value, i.e., x gr:hasCurrencyValue y implies x gr:hasMinCurrencyValue y, x gr:hasMaxCurrencyValue y."@en ;
        rdfs:domain       gr:PriceSpecification ;
        rdfs:isDefinedBy  <http://purl.org/goodrelations/v1> ;
        rdfs:label        "has min currency value (1..1)"@en ;
        rdfs:range        xsd:float .

gr:acceptedPaymentMethods
        a                 owl:ObjectProperty ;
        rdfs:comment      "The gr:PaymentMethod or methods accepted by the gr:BusinessEntity for the given gr:Offering."@en ;
        rdfs:domain       [ a            owl:Class ;
                            owl:unionOf  ( gr:Offering s:Offer )
                          ] ;
        rdfs:isDefinedBy  <http://purl.org/goodrelations/v1> ;
        rdfs:label        "accepted payment methods (0..*)"@en ;
        rdfs:range        gr:PaymentMethod .

dc:creator  a   owl:AnnotationProperty .

gr:Wednesday  a             gr:DayOfWeek ;
        rdfs:comment        "Wednesday as a day of the week."@en ;
        rdfs:isDefinedBy    <http://purl.org/goodrelations/v1> ;
        rdfs:label          "Wednesday (day of week)"@en ;
        gr:displayPosition  3 ;
        gr:hasNext          gr:Thursday ;
        gr:hasPrevious      gr:Tuesday .

gr:hasValueFloat  a         owl:DatatypeProperty ;
        rdfs:comment        "This subproperty specifies that the upper and lower limit of the given gr:QuantitativeValueFloat are identical and have the respective float value. It is a shortcut for such cases where a quantitative property is (at least practically) a single point value and not an interval."@en ;
        rdfs:domain         gr:QuantitativeValueFloat ;
        rdfs:isDefinedBy    <http://purl.org/goodrelations/v1> ;
        rdfs:label          "has value float (0..1)"@en ;
        rdfs:range          xsd:float ;
        rdfs:subPropertyOf  gr:hasMinValueFloat , gr:hasMaxValueFloat .

gr:hasCurrencyValue  a      owl:DatatypeProperty ;
        rdfs:comment        "This property specifies the amount of money for a price per unit, shipping charges, or payment charges. The currency and other relevant details are attached to the respective gr:PriceSpecification etc.\n\nFor a gr:UnitPriceSpecification, this is the price for one unit or bundle (as specified in the unit of measurement of the unit price specification) of the respective gr:ProductOrService. For a gr:DeliveryChargeSpecification or a gr:PaymentChargeSpecification, it is the price per delivery or payment.\n\nGoodRelations also supports giving price information as intervals only. If this is needed, use gr:hasMaxCurrencyValue for the upper bound and gr:hasMinCurrencyValue for the lower bound. \n\nUsing gr:hasCurrencyValue sets the upper and lower bounds to the same given value, i.e., x gr:hasCurrencyValue y implies x gr:hasMinCurrencyValue y, x gr:hasMaxCurrencyValue y."@en ;
        rdfs:domain         gr:PriceSpecification ;
        rdfs:isDefinedBy    <http://purl.org/goodrelations/v1> ;
        rdfs:label          "has currency value (0..1)"@en ;
        rdfs:range          xsd:float ;
        rdfs:subPropertyOf  gr:hasMinCurrencyValue , gr:hasMaxCurrencyValue .

gr:isAccessoryOrSparePartFor
        a                 owl:ObjectProperty ;
        rdfs:comment      "This states that a particular gr:ProductOrService is an accessory or spare part for another product or service."@en ;
        rdfs:domain       [ a            owl:Class ;
                            owl:unionOf  ( gr:ProductOrService s:Product )
                          ] ;
        rdfs:isDefinedBy  <http://purl.org/goodrelations/v1> ;
        rdfs:label        "is accessory or spare part for (0..*)"@en ;
        rdfs:range        gr:ProductOrService .

foaf:homepage  a  owl:AnnotationProperty .

attr:attr-security-management-encrypted-storage
        a                    usdl-pref:ServiceAttribute ;
        dcterms:created      "2014-07-18T15:57:10+03:00"^^xsd:dateTime ;
        dcterms:creator      ""^^xsd:string ;
        dcterms:description  ""^^xsd:string ;
        dcterms:identifier   "attr-security-management-encrypted-storage"^^xsd:string ;
        dcterms:modified     "2014-07-18T15:57:10+03:00"^^xsd:dateTime ;
        dcterms:title        "Encrypted Storage"^^xsd:string ;
        skos:broader         attr:attr-security-management .

usdl-sla-cb:hasMaxSupport
        a                   rdf:Property ;
        rdfs:comment        "<p>Indicates a max support.</p>"@en ;
        rdfs:domain         usdl-sla-cb:FuzzyValue ;
        rdfs:isDefinedBy    usdl-core-cb: ;
        rdfs:label          "has max support"@en ;
        rdfs:range          xsd:float ;
        rdfs:subPropertyOf  gr:hasMaxValueFloat .

attr:attr-financial-structure
        a                    usdl-pref:ServiceAttribute ;
        dcterms:created      "2014-07-18T09:41:49Z"^^xsd:dateTime ;
        dcterms:creator      ""^^xsd:string ;
        dcterms:description  "How responsive to the client's needs are the cloud service provider's pricing and billing components"^^xsd:string ;
        dcterms:identifier   "attr-financial-structure"^^xsd:string ;
        dcterms:modified     "2014-07-18T09:41:49Z"^^xsd:dateTime ;
        dcterms:title        "Financial Structure"^^xsd:string ;
        skos:broader         attr:attr-financial .

gr:lesser  a              owl:TransitiveProperty , owl:ObjectProperty ;
        rdfs:comment      "This ordering relation for gr:QualitativeValue pairs indicates that the subject is lesser than the object."@en ;
        rdfs:domain       gr:QualitativeValue ;
        rdfs:isDefinedBy  <http://purl.org/goodrelations/v1> ;
        rdfs:label        "lesser (0..*)"@en ;
        rdfs:range        gr:QualitativeValue ;
        owl:inverseOf     gr:greater .

attr:attr-performance-capacity-memory
        a                    usdl-pref:ServiceAttribute ;
        dcterms:created      "2014-07-18T11:57:29Z"^^xsd:dateTime ;
        dcterms:creator      ""^^xsd:string ;
        dcterms:description  ""^^xsd:string ;
        dcterms:identifier   "attr-performance-capacity-memory"^^xsd:string ;
        dcterms:modified     "2014-07-18T11:57:29Z"^^xsd:dateTime ;
        dcterms:title        "Memory"^^xsd:string ;
        skos:broader         attr:attr-performance-capacity .

attr:attr-assurance  a       usdl-pref:ServiceAttribute ;
        dcterms:created      "2014-05-23T18:16:36Z"^^xsd:dateTime ;
        dcterms:creator      ""^^xsd:string ;
        dcterms:description  "Indicates how likely it is that the service will be available as specified"^^xsd:string ;
        dcterms:identifier   "attr-assurance"^^xsd:string ;
        dcterms:modified     "2014-07-18T08:47:41Z"^^xsd:dateTime ;
        dcterms:title        "Assurance"^^xsd:string ;
        skos:broader         attr:attr-root .

usdl-pref:hasPreferenceProfile
        a                 rdf:Property ;
        rdfs:comment      "<p>Consumer Preference Profiles. We assume here that Consumer is described as an instance of gr:BusinessEntity.</p>\r\n" ;
        rdfs:domain       gr:BusinessEntity ;
        rdfs:isDefinedBy  <http://www.linked-usdl.org/ns/usdl-pref> ;
        rdfs:label        "has preference profile" ;
        rdfs:range        usdl-pref:ConsumerPreferenceProfile .

gr:Enduser  a             gr:BusinessEntityType ;
        rdfs:comment      "The gr:BusinessEntityType representing such agents that are purchasing the good or service for private consumption, in particular not for resale or for usage within an industrial enterprise. By default, a Business Entity is an Enduser."@en ;
        rdfs:isDefinedBy  <http://purl.org/goodrelations/v1> ;
        rdfs:label        "Enduser (business entity type)"@en .

gr:UPS  a                 gr:DeliveryModeParcelService ;
        rdfs:comment      "Delivery via the parcel service UPS."@en ;
        rdfs:isDefinedBy  <http://purl.org/goodrelations/v1> ;
        rdfs:label        "UPS (delivery method)"@en .

usdl-pref:ServiceAttribute
        a                 owl:Class , rdfs:Class ;
        rdfs:comment      "<p>The ServiceAttribute class forms a classification of cloud service attributes used for optimization. It is a subclass of skos:Concept and uses its properties: skos:broader, skos:narrower to express the hierarchical relation between the attributes. This classification is derived and extends the Service Measurement Index in order to encompass both precise and imprecise attributes. SMI is currently being developed by the Cloud Services Measurement Initiative Consortium</p>"@en ;
        rdfs:isDefinedBy  <http://www.linked-usdl.org/ns/usdl-pref> ;
        rdfs:label        "Service Attribute"@en ;
        rdfs:subClassOf   skos:Concept .

attr:attr-performance-service-response-time-minimum
        a                    usdl-pref:ServiceAttribute ;
        dcterms:created      "2014-07-18T12:05:02Z"^^xsd:dateTime ;
        dcterms:creator      ""^^xsd:string ;
        dcterms:description  ""^^xsd:string ;
        dcterms:identifier   "attr-performance-service-response-time-minimum"^^xsd:string ;
        dcterms:modified     "2014-07-18T12:05:02Z"^^xsd:dateTime ;
        dcterms:title        "Minimum Response time"^^xsd:string ;
        skos:broader         attr:attr-performance-service-response-time .

attr:attr-assurance-service-stability-cpu
        a                    usdl-pref:ServiceAttribute ;
        dcterms:created      "2014-05-23T21:29:16+03:00"^^xsd:dateTime ;
        dcterms:creator      ""^^xsd:string ;
        dcterms:description  ""^^xsd:string ;
        dcterms:identifier   "attr-assurance-service-stability-cpu"^^xsd:string ;
        dcterms:modified     "2014-05-23T21:29:16+03:00"^^xsd:dateTime ;
        dcterms:title        "CPU"^^xsd:string ;
        skos:broader         attr:attr-assurance-service-stability .

gr:predecessorOf  a       owl:TransitiveProperty , owl:ObjectProperty ;
        rdfs:comment      "This property indicates that the subject is a previous, often discontinued variant of the gr:ProductOrServiceModel used as the object.\n\nExample: Golf III predecessorOf Golf IV\n\nThis relation is transitive."@en ;
        rdfs:domain       gr:ProductOrServiceModel ;
        rdfs:isDefinedBy  <http://purl.org/goodrelations/v1> ;
        rdfs:label        "predecessor of (0..*)"@en ;
        rdfs:range        gr:ProductOrServiceModel ;
        owl:inverseOf     gr:successorOf .

gr:FederalExpress  a      gr:DeliveryModeParcelService ;
        rdfs:comment      "Delivery via the parcel service Federal Express."@en ;
        rdfs:isDefinedBy  <http://purl.org/goodrelations/v1> ;
        rdfs:label        "Federal Express (delivery method)"@en .

attr:attr-performance-functionality-quality-of-features
        a                    usdl-pref:ServiceAttribute ;
        dcterms:created      "2014-07-18T12:02:40Z"^^xsd:dateTime ;
        dcterms:creator      ""^^xsd:string ;
        dcterms:description  ""^^xsd:string ;
        dcterms:identifier   "attr-performance-functionality-quality-of-features"^^xsd:string ;
        dcterms:modified     "2014-07-18T12:02:40Z"^^xsd:dateTime ;
        dcterms:title        "Quality of Features"^^xsd:string ;
        skos:broader         attr:attr-performance-functionality .

attr:attr-accountability
        a                    usdl-pref:ServiceAttribute ;
        dcterms:description  "Measures the properties related to the cloud service provider organization"^^xsd:string ;
        dcterms:identifier   "attr-accountability"^^xsd:string ;
        dcterms:modified     "2014-07-18T10:29:44+03:00"^^xsd:dateTime ;
        dcterms:title        "Accountability"^^xsd:string ;
        skos:broader         attr:attr-root .

<http://www.linked-usdl.org/ns/usdl-interaction-types>
        a                              owl:Ontology , skos:ConceptScheme ;
        dcterms:creator                usdl-core:cpedrinaci , usdl-core:jcardoso , usdl-core:tleidig ;
        dcterms:description            "<p>This vocabulary provides the core InteractionTypes contemplated within Linked USDL. It therefore covers different categorisations for the Interactions that can occur in an InteractionPoint. The taxonomy provided here is a minimal reference taxonomy focussed on the level of automation and the locality considerations (e.g., on-site vs remote). Extensions or replacements for this could be defined an used within applications in the very same way by refining InteractionType. </p>"@en ;
        dcterms:modified               "2013-02-11"^^xsd:date , "2014-01-14"^^xsd:date ;
        dcterms:title                  "Linked USDL Basic Interaction Types concept scheme" ;
        vann:preferredNamespacePrefix  "usdl-it" ;
        vann:preferredNamespaceUri     "http://www.linked-usdl.org/ns/usdl-interaction-types#" ;
        skos:hasTopConcept             <http://www.linked-usdl.org/ns/semi-automated> , <http://www.linked-usdl.org/ns/automated> , <http://www.linked-usdl.org/ns/remote> , <http://www.linked-usdl.org/ns/manual> , <http://www.linked-usdl.org/ns/on-site> ;
        skos:prefLabel                 "Interaction Types"@en ;
        foaf:page                      <http://www.linked-usdl.org/ns/usdl-interaction-types.html> .

usdl-testing:SearchBasedTesting
        a                  usdl-testing:TestGenerationStrategy ;
        rdfs:label         "Search-based Testing"@en ;
        skos:altLabel      "Search-based Testing"@en ;
        skos:definition    "<p>A testing method is a search-based testing method.</p>"@en ;
        skos:inScheme      usdl-testing:TestGenerationStrategyClassificationScheme ;
        skos:prefLabel     "Search-based Testing"@en ;
        skos:topConceptOf  usdl-testing:TestGenerationStrategyClassificationScheme .

<http://www.linked-usdl.org/ns/remote>
        a                  usdl-core:InteractionType ;
        rdfs:label         "Remote"@en ;
        skos:altLabel      "Remote Interaction"@en ;
        skos:definition    "<p>The interaction between the two parties can take place entirely remotely, e.g.,  the travel insurance service is provided entirely remotely independently from any location.</p>"@en ;
        skos:inScheme      <http://www.linked-usdl.org/ns/usdl-interaction-types> ;
        skos:prefLabel     "Remote"@en ;
        skos:topConceptOf  <http://www.linked-usdl.org/ns/usdl-interaction-types> .

usdl-pref:hasWeight  a    rdf:Property ;
        rdfs:comment      "<p>The relative weight of a consumer preference within a profile.</p>\r\n" ;
        rdfs:domain       usdl-pref:ConsumerPreference ;
        rdfs:isDefinedBy  <http://www.linked-usdl.org/ns/usdl-pref> ;
        rdfs:label        "has weight" ;
        rdfs:range        usdl-pref:Weight .

usdl-testing:TestGenerationStrategyClassificationScheme
        a                    skos:ConceptScheme ;
        dcterms:description  "<p>This vocabulary provides the concepts to classify test generation strategy dimension. </p>"@en ;
        dcterms:title        "Test Generation Strategy classification concept scheme" ;
        skos:hasTopConcept   usdl-testing:SearchBasedTesting , usdl-testing:SystematicTesting , usdl-testing:RandomTesting , usdl-testing:ManualTesting ;
        skos:prefLabel       "Testing Generation Strategy Classification"@en .

attr:attr-reputation-sustainability-energy-consumption
        a                    usdl-pref:ServiceAttribute ;
        dcterms:created      "2014-07-18T16:35:29+03:00"^^xsd:dateTime ;
        dcterms:description  ""^^xsd:string ;
        dcterms:identifier   "attr-reputation-sustainability-energy-consumption"^^xsd:string ;
        dcterms:modified     "2014-07-18T16:35:29+03:00"^^xsd:dateTime ;
        dcterms:title        "Energy consumption"^^xsd:string ;
        skos:broader         attr:attr-reputation-sustainability .

usdl-testing:focusOn  a   rdf:Property ;
        rdfs:comment      "<p>Connects TestingMethod to TestingFocus classification dimension.</p>"@en ;
        rdfs:domain       usdl-testing:TestingMethod ;
        rdfs:isDefinedBy  <http://www.linked-usdl.org/ns/usdl-core/cloud-broker/testing> ;
        rdfs:label        "focus on"@en ;
        rdfs:range        usdl-testing:TestingFocus .

usdl-testing:hasTestingMethod
        a                 rdf:Property ;
        rdfs:comment      "<p>Connects TestingProcedure to TestingMethod description.</p>"@en ;
        rdfs:domain       usdl-testing:TestingProcedure ;
        rdfs:isDefinedBy  <http://www.linked-usdl.org/ns/usdl-core/cloud-broker/testing> ;
        rdfs:label        "has testing method"@en ;
        rdfs:range        usdl-testing:TestingMethod .

attr:attr-assurance-serviceability
        a                    usdl-pref:ServiceAttribute ;
        dcterms:created      "2014-05-23T18:28:31Z"^^xsd:dateTime ;
        dcterms:creator      ""^^xsd:string ;
        dcterms:description  "The ease and efficiency of performing maintenance and correcting problems with the service"^^xsd:string ;
        dcterms:identifier   "attr-assurance-serviceability"^^xsd:string ;
        dcterms:modified     "2014-07-18T09:13:22Z"^^xsd:dateTime ;
        dcterms:title        "Serviceability"^^xsd:string ;
        skos:broader         attr:attr-assurance .

s:Person  a              owl:Class ;
        rdfs:subClassOf  gr:BusinessEntity .

gr:amountOfThisGood  a    owl:DatatypeProperty ;
        rdfs:comment      "This property specifies the quantity of the goods included in the gr:Offering via this gr:TypeAndQuantityNode. The quantity is given in the unit of measurement attached to the gr:TypeAndQuantityNode."@en ;
        rdfs:domain       gr:TypeAndQuantityNode ;
        rdfs:isDefinedBy  <http://purl.org/goodrelations/v1> ;
        rdfs:label        "amount of this good (1..1)"@en ;
        rdfs:range        xsd:float .

attr:attr-accountability-personnel-requirements-technical-competency-of-support
        a                    usdl-pref:ServiceAttribute ;
        dcterms:created      "2014-07-18T07:36:47Z"^^xsd:dateTime ;
        dcterms:creator      ""^^xsd:string ;
        dcterms:description  ""^^xsd:string ;
        dcterms:identifier   "attr-accountability-personnel-requirements-technical-competency-of-support"^^xsd:string ;
        dcterms:modified     "2014-07-18T07:36:47Z"^^xsd:dateTime ;
        dcterms:title        "Technical competency of the support employees"^^xsd:string ;
        skos:broader         attr:attr-accountability-personnel-requirements .

gr:eligibleCustomerTypes
        a                 owl:ObjectProperty ;
        rdfs:comment      "The types of customers (gr:BusinessEntityType) for which the given gr:Offering is valid."@en ;
        rdfs:domain       [ a            owl:Class ;
                            owl:unionOf  ( gr:Offering s:Offer )
                          ] ;
        rdfs:isDefinedBy  <http://purl.org/goodrelations/v1> ;
        rdfs:label        "eligible customer types (0..*)"@en ;
        rdfs:range        gr:BusinessEntityType .

gr:appliesToDeliveryMethod
        a                 owl:ObjectProperty ;
        rdfs:comment      "This property specifies the gr:DeliveryMethod to which the gr:DeliveryChargeSpecification applies."@en ;
        rdfs:domain       gr:DeliveryChargeSpecification ;
        rdfs:isDefinedBy  <http://purl.org/goodrelations/v1> ;
        rdfs:label        "applies to delivery method (0..*)"@en ;
        rdfs:range        gr:DeliveryMethod .

gr:availabilityStarts
        a                 owl:DatatypeProperty ;
        rdfs:comment      "This property specifies the beginning of the availability of the gr:ProductOrService included in the gr:Offering.\nThe difference to the properties gr:validFrom and gr:validThrough is that those specify the period of time during which the offer is valid and can be accepted.\n\nExample: I offer to lease my boat for the period of August 1 - August 31, 2010, but you must accept by offer no later than July 15.\n\nA time-zone should be specified. For a time in GMT/UTC, simply add a \"Z\" following the time:\n\n2008-05-30T09:30:10Z.\n\nAlternatively, you can specify an offset from the UTC time by adding a positive or negative time following the time:\n\n2008-05-30T09:30:10-09:00\n\nor\n\n2008-05-30T09:30:10+09:00.\n\nNote: There is another property gr:availableAtOrFrom, which is used to indicate the gr:Location (e.g. store or shop) from which the goods would be available."@en ;
        rdfs:domain       [ a            owl:Class ;
                            owl:unionOf  ( gr:Offering s:Offer )
                          ] ;
        rdfs:isDefinedBy  <http://purl.org/goodrelations/v1> ;
        rdfs:label        "availability starts (0..1)"@en ;
        rdfs:range        xsd:dateTime .

usdl-sla-cb:hasDefaultQualitativeProperty
        a                 rdf:Property ;
        rdfs:comment      "<p>The default qualitative value of the variable.</p>\r\n" ;
        rdfs:domain       usdl-sla:Variable ;
        rdfs:isDefinedBy  <http://linked-usdl.org/ns/usdl-sla/cloud-broker> ;
        rdfs:label        "has default qualitative property" ;
        rdfs:range        gr:QualitativeValue .

gr:PriceSpecification
        a                 owl:Class ;
        rdfs:comment      "The superclass of all price specifications."@en ;
        rdfs:isDefinedBy  <http://purl.org/goodrelations/v1> ;
        rdfs:label        "Price specification"@en ;
        owl:disjointWith  gr:Location , gr:DayOfWeek , gr:PaymentMethod , gr:BusinessEntity , gr:Brand , gr:ProductOrService , gr:BusinessFunction , gr:TypeAndQuantityNode , gr:BusinessEntityType , gr:DeliveryMethod , gr:WarrantyPromise , gr:QuantitativeValue , gr:WarrantyScope , gr:OpeningHoursSpecification , gr:Offering .

usdl-testing:hasTestingInstructions
        a                 rdf:Property ;
        rdfs:comment      "<p>Connects TestingProcedure to a resource containing testing instructions.</p>"@en ;
        rdfs:domain       usdl-testing:TestingProcedure ;
        rdfs:isDefinedBy  <http://www.linked-usdl.org/ns/usdl-core/cloud-broker/testing> ;
        rdfs:label        "has testing instructions"@en ;
        rdfs:range        rdfs:Resource .

usdl-testing:RegressionTesting
        a                  usdl-testing:TestingGoal ;
        rdfs:label         "Regression Testing"@en ;
        skos:altLabel      "Regression Testing"@en ;
        skos:definition    "<p>A testing method is a regression testing method.</p>"@en ;
        skos:inScheme      usdl-testing:TestingGoalClassificationScheme ;
        skos:prefLabel     "Regression Testing"@en ;
        skos:topConceptOf  usdl-testing:TestingGoalClassificationScheme .

gr:COD  a                 gr:PaymentMethod ;
        rdfs:comment      "Collect on delivery / Cash on delivery - A payment method where the recipient of goods pays at the time of delivery. Usually, the amount of money is collected by the transportation company handling the goods."@en ;
        rdfs:isDefinedBy  <http://purl.org/goodrelations/v1> ;
        rdfs:label        "COD (payment method)"@en .

gr:hasISICv4  a           owl:DatatypeProperty ;
        rdfs:comment      "The International Standard of Industrial Classification of All Economic Activities (ISIC), Revision 4 code for a particular gr:BusinessEntity or gr:Location. See http://unstats.un.org/unsd/cr/registry/isic-4.asp for more information.\n\nNote: While ISIC codes are sometimes misused for classifying products or services, they are designed and suited only for classifying business establishments."@en ;
        rdfs:domain       [ a            owl:Class ;
                            owl:unionOf  ( gr:BusinessEntity gr:Location s:Organization s:Place )
                          ] ;
        rdfs:isDefinedBy  <http://purl.org/goodrelations/v1> ;
        rdfs:label        "has ISIC v4 (0..*)"@en ;
        rdfs:range        xsd:int .

attr:attr-security-data-privacy-loss-audit-trailing
        a                    usdl-pref:ServiceAttribute ;
        dcterms:created      "2014-07-18T15:54:00+03:00"^^xsd:dateTime ;
        dcterms:description  ""^^xsd:string ;
        dcterms:identifier   "attr-security-data-privacy-loss-audit-trailing"^^xsd:string ;
        dcterms:modified     "2014-07-18T15:54:00+03:00"^^xsd:dateTime ;
        dcterms:title        "Audit Trailing"^^xsd:string ;
        skos:broader         attr:attr-security-data-privacy-loss .

attr:attr-usability  a       usdl-pref:ServiceAttribute ;
        dcterms:created      "2014-07-18T15:58:49+03:00"^^xsd:dateTime ;
        dcterms:description  "It is related to the ease with which a service can be used"^^xsd:string ;
        dcterms:identifier   "attr-usability"^^xsd:string ;
        dcterms:modified     "2014-07-18T15:58:49+03:00"^^xsd:dateTime ;
        dcterms:title        "Usability"^^xsd:string ;
        skos:broader         attr:attr-root .

usdl-testing:IntegrationTesting
        a                  usdl-testing:TestingScale ;
        rdfs:label         "Integration Testing"@en ;
        skos:altLabel      "Integration Testing"@en ;
        skos:definition    "<p>A testing method is an integration testing method.</p>"@en ;
        skos:inScheme      usdl-testing:TestingScaleClassificationScheme ;
        skos:prefLabel     "Integration Testing"@en ;
        skos:topConceptOf  usdl-testing:TestingScaleClassificationScheme .

usdl-sla-cb:dependsOn
        a                 rdf:Property ;
        rdfs:comment      "<p>Indicates if a service depends on an other service. </p>"@en ;
        rdfs:domain       usdl-core:Service ;
        rdfs:isDefinedBy  usdl-core-cb: ;
        rdfs:label        "depends on"@en ;
        rdfs:range        usdl-core:Service .

usdl-core:ServiceIndividual
        a                 owl:Class , rdfs:Class ;
        rdfs:comment      "<p>Instances of ServiceIndividual are actual services that are creating value to a network of business entities. For instance, your concrete life insurance provided by AXA is a ServiceIndividual which is providing value to yourself and AXA.</p>"@en ;
        rdfs:isDefinedBy  <http://www.linked-usdl.org/ns/usdl-core> ;
        rdfs:label        "Service Individual"@en ;
        rdfs:subClassOf   gr:Individual , usdl-core:Service .

attr:attr-usability-transparency
        a                    usdl-pref:ServiceAttribute ;
        dcterms:created      "2014-07-18T16:24:46+03:00"^^xsd:dateTime ;
        dcterms:description  "The extent to which users are able to determine when changes in a feature or component of the service occur and whether these changes impact usability"^^xsd:string ;
        dcterms:identifier   "attr-usability-transparency"^^xsd:string ;
        dcterms:modified     "2014-07-18T16:24:46+03:00"^^xsd:dateTime ;
        dcterms:title        "Transparency"^^xsd:string ;
        skos:broader         attr:attr-usability .

attr:attr-assurance-service-stability
        a                    usdl-pref:ServiceAttribute ;
        dcterms:created      "2014-05-23T18:28:13Z"^^xsd:dateTime ;
        dcterms:creator      ""^^xsd:string ;
        dcterms:description  "The degree to which the service is resistant to change, deterioration, or displacement"^^xsd:string ;
        dcterms:identifier   "attr-assurance-service-stability"^^xsd:string ;
        dcterms:modified     "2014-07-18T08:54:41Z"^^xsd:dateTime ;
        dcterms:title        "Service Stability"^^xsd:string ;
        skos:broader         attr:attr-assurance .

gr:Business  a            gr:BusinessEntityType ;
        rdfs:comment      "The gr:BusinessEntityType representing such agents that are themselves offering commercial services or products on the market. Usually, businesses are characterized by the fact that they are officially registered with the public administration and strive for profits by their activities."@en ;
        rdfs:isDefinedBy  <http://purl.org/goodrelations/v1> ;
        rdfs:label        "Business (business entity type)"@en .

gr:validThrough  a        owl:DatatypeProperty ;
        rdfs:comment      "This property specifies the end of the validity of the gr:Offering, gr:PriceSpecification, gr:License, or gr:OpeningHoursSpecification.\nA time-zone should be specified. For a time in GMT/UTC, simply add a \"Z\" following the time:\n\n2008-05-30T09:30:10Z.\n\nAlternatively, you can specify an offset from the UTC time by adding a positive or negative time following the time:\n\n2008-05-30T09:30:10-09:00\n\nor\n2008-05-30T09:30:10+09:00.\n\nNote 1: If multiple contradicting instances of a gr:Offering, gr:PriceSpecification, or gr:OpeningHoursSpecification exist, it is a good heuristics to assume that\n1. Information with validity information for the respective period of time ranks higher than information without validity information.\n2. Among conflicting nodes both having validity information, the one with the shorter validity span ranks higher.\nNote 2: For Google, attaching a gr:validThrough statement to a gr:UnitPriceSpecification is mandatory. \n"@en ;
        rdfs:domain       [ a            owl:Class ;
                            owl:unionOf  ( gr:Offering gr:OpeningHoursSpecification gr:PriceSpecification gr:License s:Offer )
                          ] ;
        rdfs:isDefinedBy  <http://purl.org/goodrelations/v1> ;
        rdfs:label        "valid through (0..1)"@en ;
        rdfs:range        xsd:dateTime .

usdl-pref:hasDefaultQuantitativeValue
        a                 rdf:Property ;
        rdfs:comment      "<p>The quantitative value of a preference variable.</p>\r\n" ;
        rdfs:domain       usdl-pref:QuantitativeVariable ;
        rdfs:isDefinedBy  <http://www.linked-usdl.org/ns/usdl-pref> ;
        rdfs:label        "has default quantitative value" ;
        rdfs:range        gr:QuantitativeValue .

usdl-testing:hasTestingProcedure
        a                 rdf:Property ;
        rdfs:comment      "<p>Connects Service Interaction Point to a TestingProcedure.</p>"@en ;
        rdfs:domain       usdl-core:InteractionPoint ;
        rdfs:isDefinedBy  <http://www.linked-usdl.org/ns/usdl-core/cloud-broker/testing> ;
        rdfs:label        "has testing procedure"@en ;
        rdfs:range        usdl-testing:TestingProcedure .

usdl-sla-cb:hasClassificationDimension
        a                   rdf:Property ;
        rdfs:comment        "<p>Indicates a classification dimension of a Service restricted to the taxonomies sub-classified under the usdl-core-cb:ClassificationDimension class.</p>"@en ;
        rdfs:domain         usdl-core:Service ;
        rdfs:isDefinedBy    usdl-core-cb: ;
        rdfs:label          "has classification dimension"@en ;
        rdfs:range          usdl-sla-cb:ClassificationDimension ;
        rdfs:subPropertyOf  usdl-core:hasClassification .

gr:width  a                 owl:ObjectProperty ;
        rdfs:comment        "The width of the gr:ProductOrService.\nTypical unit code(s): CMT for centimeters, INH for inches"@en ;
        rdfs:domain         [ a            owl:Class ;
                              owl:unionOf  ( gr:ProductOrService s:Product )
                            ] ;
        rdfs:isDefinedBy    <http://purl.org/goodrelations/v1> ;
        rdfs:label          "width (0..1)"@en ;
        rdfs:range          gr:QuantitativeValue ;
        rdfs:subPropertyOf  gr:quantitativeProductOrServiceProperty .

dc:contributor  a  owl:AnnotationProperty .

gr:relatedWebService  a   owl:AnnotationProperty ;
        rdfs:comment      "The URI of a SOAP or REST Web Service from which additional information about the gr:BusinessEntity, gr:Offering, gr:PriceSpecification, or gr:ProductOrService, or any other element,  can be obtained. The recommended range is xsd:anyURI i.e., the URI of a SOAP or REST Web Service.\n\nIn principle, any existing or upcoming vocabulary for Web Services can be used in combination with GoodRelations, because the association between (a) the service description and (b) the GoodRelations description can be found via the Web Service URI value used with this gr:relatedWebService property."@en ;
        rdfs:isDefinedBy  <http://purl.org/goodrelations/v1> ;
        rdfs:label        "related Web Service (0..*)"@en .

usdl-testing:SystemTesting
        a                  usdl-testing:TestingScale ;
        rdfs:label         "System Testing"@en ;
        skos:altLabel      "System Testing"@en ;
        skos:definition    "<p>A testing method is a system testing method.</p>"@en ;
        skos:inScheme      usdl-testing:TestingScaleClassificationScheme ;
        skos:prefLabel     "System Testing"@en ;
        skos:topConceptOf  usdl-testing:TestingScaleClassificationScheme .

<http://purl.org/goodrelations/v1>
        a                owl:Ontology ;
        rdfs:comment     "The GoodRelations ontology provides the vocabulary for annotating e-commerce offerings (1) to sell, lease, repair, dispose, or maintain commodity products and (2) to provide commodity services.\n\nGoodRelations allows describing the relationship between (1) Web resources, (2) offerings made by those Web resources, (3) legal entities, (4) prices, (5) terms and conditions, and the aforementioned ontologies for products and services (6).\n \nFor more information, see http://purl.org/goodrelations/\n\nNote: The base URI of GoodRelations is http://purl.org/goodrelations/v1. Please make sure you are only using element identifiers in this namespace, e.g. http://purl.org/goodrelations/v1#BusinessEntity. There may be copies of the ontology file on the Web which can be retrieved from other locations, BUT THOSE LOCATIONS MUST NOT BE USED AS THE BASIS OF IDENTIFIERS.\n\nIf you use GoodRelations for scientific purposes, please cite our paper:\n\nHepp, Martin: GoodRelations: An Ontology for Describing Products and Services Offers on the Web, Proceedings of the 16th International Conference on Knowledge Engineering and Knowledge Management (EKAW2008), September 29 - October 3, 2008, Acitrezza, Italy, Springer LNCS, Vol. 5268, pp. 332-347.\n\nPDF at http://www.heppnetz.de/publications/"@en ;
        rdfs:label       "GoodRelations Ontology"@en ;
        dc:contributor   "Work on the GoodRelations ontology and related research and development has been partly supported by the Austrian BMVIT/FFG under the FIT-IT Semantic Systems project myOntology (grant no. 812515/9284), by a Young Researcher's Grant (Nachwuchsfoerderung 2005-2006) from the Leopold-Franzens-Universitaet Innsbruck, by the European Commission under the project SUPER (FP6-026850), and by the German Federal Ministry of Research (BMBF) by a grant under the KMU Innovativ program as part of the Intelligent Match project (FKZ 01IS10022B). The"@en ;
        dc:creator       "Martin Hepp"@en ;
        dc:rights        "The GoodRelations ontology is available under the Creative Commons Attribution 3.0 Unported license; see http://creativecommons.org/licenses/by/3.0/. In a nutshell, you are free to copy, distribute and transmit the work; to remix/adapt the work (e.g. to import the ontology and create specializations of its elements), as long as you attribute the work in the manner specified by the author or licensor (but not in any way that suggests that they endorse you or your use of the work). Proper Attribution: Simply include the statement \"This work is based on the GoodRelations ontology, developed by Martin Hepp\" and link back to http://purl.org/goodrelations/"@en ;
        dc:subject       "E-Commerce, E-Business, GoodRelations, Microdata, Ontology, Semantic SEO, RDFa, Linked Data, RDF, Semantic Web, Recommender Systems"@en ;
        dc:title         "The GoodRelations Vocabulary for Semantic Web-based E-Commerce"@en ;
        dcterms:license  <http://creativecommons.org/licenses/by/3.0/> ;
        owl:versionInfo  "V 1.0, Release 2011-10-01"@en ;
        foaf:homepage    <http://purl.org/goodrelations/> .

gr:hasWarrantyPromise
        a                 owl:ObjectProperty ;
        rdfs:comment      "This specifies the gr:WarrantyPromise made by the gr:BusinessEntity for the given gr:Offering."@en ;
        rdfs:domain       [ a            owl:Class ;
                            owl:unionOf  ( gr:Offering s:Offer )
                          ] ;
        rdfs:isDefinedBy  <http://purl.org/goodrelations/v1> ;
        rdfs:label        "has warranty promise (0..*)"@en ;
        rdfs:range        gr:WarrantyPromise .

gr:DayOfWeek  a           owl:Class ;
        rdfs:comment      "The day of the week, used to specify  to which day the opening hours of a gr:OpeningHoursSpecification refer.\n\nExamples: Monday, Tuesday, Wednesday,..."@en ;
        rdfs:isDefinedBy  <http://purl.org/goodrelations/v1> ;
        rdfs:label        "Day of week"@en ;
        owl:disjointWith  gr:PaymentMethod , gr:Brand , gr:OpeningHoursSpecification , gr:Offering , gr:PriceSpecification , gr:Location , gr:DeliveryMethod , gr:WarrantyScope , gr:ProductOrService , gr:TypeAndQuantityNode , gr:WarrantyPromise , gr:BusinessEntityType , gr:BusinessFunction , gr:BusinessEntity , gr:QuantitativeValue .

gr:PaymentChargeSpecification
        a                 owl:Class ;
        rdfs:comment      "A payment charge specification is a conceptual entity that specifies the additional costs asked for settling the payment after accepting a given gr:Offering using a particular gr:PaymentMethod. A payment charge specification is characterized by (1) a monetary amount per order specified as a literal value of type float in combination with a Currency, (2) the payment method, and (3) a whether this charge includes local sales taxes, namely VAT.\nA gr:Offering may be linked to multiple payment charge specifications that specify alternative charges for various payment methods.\n\nExamples: Payment by VISA or Mastercard costs a fee of 3 Euros including VAT, payment by bank transfer in advance is free of charge.\n\nThe total amount of this surcharge is specified as a float value of the gr:hasCurrencyValue property. The currency is specified via the gr:hasCurrency datatype property. Whether the price includes VAT or not is indicated by the gr:valueAddedTaxIncluded datatype property. The gr:PaymentMethod to which this charge applies is specified using the gr:appliesToPaymentMethod object property.\n\nIf the price can only be given as a range, use gr:hasMaxCurrencyValue and gr:hasMinCurrencyValue for the upper and lower bounds.\n\nImportant: When querying for the price, always use gr:hasMaxCurrencyValue and gr:hasMinCurrencyValue."@en ;
        rdfs:isDefinedBy  <http://purl.org/goodrelations/v1> ;
        rdfs:label        "Payment charge specification"@en ;
        rdfs:subClassOf   gr:PriceSpecification ;
        owl:disjointWith  gr:UnitPriceSpecification , gr:DeliveryChargeSpecification .

<http://www.linked-usdl.org/ns/observer>
        a                  usdl-core:InteractionRole ;
        rdfs:label         "Observer"@en ;
        skos:definition    "<p>An Observer within an Interaction is a third party entity that does not take any active role within the interaction. Observers are typically monitoring the actual activities in order to ensure that best practices or regulations are followed (e.g., Regulators, Quality Assurance Departments).</p>"@en ;
        skos:inScheme      <http://www.linked-usdl.org/ns/usdl-interaction-roles> ;
        skos:narrower      <http://www.linked-usdl.org/ns/receiver> , <http://www.linked-usdl.org/ns/mediator> , <http://www.linked-usdl.org/ns/initiator> ;
        skos:prefLabel     "Observer"@en ;
        skos:topConceptOf  <http://www.linked-usdl.org/ns/usdl-interaction-roles> .

gr:N-Ary-Relations  a     owl:Class ;
        rdfs:comment      "This is the superclass for all classes that are placeholders for n-ary relations, which OWL cannot represent.\nDEPRECATED. Do not use this class in data or queries."@en ;
        rdfs:isDefinedBy  <http://purl.org/goodrelations/v1> ;
        rdfs:label        "N-ary relations (DEPRECATED)"@en ;
        owl:deprecated    true .

gr:vatID  a               owl:DatatypeProperty ;
        rdfs:comment      "The Value-added Tax ID of the gr:BusinessEntity. See http://en.wikipedia.org/wiki/Value_added_tax_identification_number for details."@en ;
        rdfs:domain       [ a            owl:Class ;
                            owl:unionOf  ( gr:BusinessEntity s:Organization s:Person )
                          ] ;
        rdfs:isDefinedBy  <http://purl.org/goodrelations/v1> ;
        rdfs:label        "VAT ID (0..1)"@en ;
        rdfs:range        xsd:string .

usdl-core:hasClassification
        a                   rdf:Property ;
        rdfs:comment        "<p>Indicates a classification of a Service.</p>"@en ;
        rdfs:domain         usdl-core:Service ;
        rdfs:isDefinedBy    <http://www.linked-usdl.org/ns/usdl-core> ;
        rdfs:label          "has classification"@en ;
        rdfs:range          skos:Concept ;
        rdfs:subPropertyOf  dcterms:subject .

attr:attr-financial-agility
        a                    usdl-pref:ServiceAttribute ;
        dcterms:created      "2014-07-18T09:41:28Z"^^xsd:dateTime ;
        dcterms:creator      ""^^xsd:string ;
        dcterms:description  "The flexibility and elasticity of the financial aspects of the CSP's services"^^xsd:string ;
        dcterms:identifier   "attr-financial-agility"^^xsd:string ;
        dcterms:modified     "2014-07-18T09:41:28Z"^^xsd:dateTime ;
        dcterms:title        "Financial Agility"^^xsd:string ;
        skos:broader         attr:attr-financial .

usdl-pref:hasPrefVariable
        a                 rdf:Property ;
        rdfs:comment      "<p>Preference variables for a consumer preference expression.</p>\r\n" ;
        rdfs:domain       usdl-pref:ConsumerPreferenceExpression ;
        rdfs:isDefinedBy  <http://www.linked-usdl.org/ns/usdl-pref> ;
        rdfs:label        "has preference variable" ;
        rdfs:range        usdl-pref:PreferenceVariable .

gr:taxID  a               owl:DatatypeProperty ;
        rdfs:comment      "The Tax / Fiscal ID of the gr:BusinessEntity, e.g. the TIN in the US or the CIF/NIF in Spain. It is usually assigned by the country of residence"@en ;
        rdfs:domain       [ a            owl:Class ;
                            owl:unionOf  ( gr:BusinessEntity s:Organization s:Person )
                          ] ;
        rdfs:isDefinedBy  <http://purl.org/goodrelations/v1> ;
        rdfs:label        "Tax ID (0..1)"@en ;
        rdfs:range        xsd:string .

attr:attr-accountability-governance
        a                    usdl-pref:ServiceAttribute ;
        dcterms:created      "2014-07-18T07:31:58Z"^^xsd:dateTime ;
        dcterms:creator      ""^^xsd:string ;
        dcterms:description  "The processes used by the service provider to manage client expectations, issues and service performance"^^xsd:string ;
        dcterms:identifier   "attr-accountability-governance"^^xsd:string ;
        dcterms:modified     "2014-07-18T07:31:58Z"^^xsd:dateTime ;
        dcterms:title        "Governance"^^xsd:string ;
        skos:broader         attr:attr-accountability .

usdl-core:InteractionRole
        a                 owl:Class , rdfs:Class ;
        rdfs:comment      "<p>The InteractionRoles that an entity may play within a service delivery chain (e.g., Initiator). One may define as many roles as necessary by defining subclasses of InteractionRole or by creating SKOS concept schemes. For completeness Linked USDL Core provides a basic concept scheme for these roles that can be used out of the box or as reference for specific extensions. See Linked USDL Interaction Roles Module.</p>"@en ;
        rdfs:isDefinedBy  <http://www.linked-usdl.org/ns/usdl-core> ;
        rdfs:label        "Interaction Role"@en ;
        rdfs:subClassOf   usdl-core:Role .

usdl-testing:NonFunctionalTesting
        a                  usdl-testing:TestingFocus ;
        rdfs:label         "Non-Functional Testing"@en ;
        skos:altLabel      "Non-Functional Testing"@en ;
        skos:definition    "<p>A testing method is a non-functional testing method.</p>"@en ;
        skos:inScheme      usdl-testing:TestingFocusClassificationScheme ;
        skos:prefLabel     "Non-Functional Testing"@en ;
        skos:topConceptOf  usdl-testing:TestingFocusClassificationScheme .

usdl-testing:TestingScale
        a                 owl:Class , rdfs:Class ;
        rdfs:comment      "<p> Testing Scale serves as a root class for a taxonomy providing vocabulary for classification of the testing scale of a testing method. </p>"@en ;
        rdfs:isDefinedBy  <http://www.linked-usdl.org/ns/usdl-core/cloud-broker/testing> ;
        rdfs:label        "Testing Scale"@en ;
        rdfs:subClassOf   skos:Concept .

usdl-testing:FaultBasedTesting
        a                  usdl-testing:TestAdequacyCriteria ;
        rdfs:label         "Fault-based Testing"@en ;
        skos:altLabel      "Fault-based Testing"@en ;
        skos:definition    "<p>A testing method is a fault-based testing method.</p>"@en ;
        skos:inScheme      usdl-testing:TestAdequacyCriteriaClassificationScheme ;
        skos:prefLabel     "Fault-based Testing"@en ;
        skos:topConceptOf  usdl-testing:TestAdequacyCriteriaClassificationScheme .

gr:UnitPriceSpecification
        a                 owl:Class ;
        rdfs:comment      "A unit price specification is a conceptual entity that specifies the price asked for a given gr:Offering by the respective gr:Business Entity. An offering may be linked to multiple unit price specifications that specify alternative prices for non-overlapping sets of conditions (e.g. quantities or sales regions) or with differing validity periods. \n\nA unit price specification is characterized by (1) the lower and upper limits and the unit of measurement of the eligible quantity, (2) by a monetary amount per unit of the product or service, and (3)  whether this prices includes local sales taxes, namely VAT.\n\t\nExample: The price, including VAT, for 1 kg of a given material is 5 Euros per kg for 0 - 5 kg and 4 Euros for quantities above 5 kg.\n\nThe eligible quantity interval for a given price is specified using the object property gr:hasEligibleQuantity, which points to an instance of gr:QuantitativeValue. The currency is specified using the gr:hasCurrency property, which points to an ISO 4217 currency code. The unit of measurement for the eligible quantity is specified using the gr:hasUnitOfMeasurement datatype property, which points to an UN/CEFACT Common Code (3 characters).\n\t\nIn most cases, the appropriate unit of measurement is the UN/CEFACT Common Code \"C62\" for \"Unit or piece\", since a gr:Offering is defined by the quantity and unit of measurement of all items included (e.g. \"1 kg of bananas plus a 2 kg of apples\"). As long at the offering consists of only one item, it is also possible to use an unit of measurement of choice for specifying the price per unit. For bundles, however, only  \"C62\" for \"Unit or piece\" is a valid unit of measurement.\n\nYou can assume that the price is given per unit or piece if there is no gr:hasUnitOfMeasurement property attached to the price.\n\t\nWhether VAT and sales taxes are included in this price is specified using the property gr:valueAddedTaxIncluded (xsd:boolean).\n\t\nThe price per unit of measurement is specified as a float value of the gr:hasCurrencyValue property. The currency is specified via the gr:hasCurrency datatype property. Whether the price includes VAT or not is indicated by the gr:valueAddedTaxIncluded datatype property.\n\nThe property priceType can be used to indicate that the price is a retail price recommendation only (i.e. a list price). \n\nIf the price can only be given as a range, use gr:hasMaxCurrencyValue and gr:hasMinCurrencyValue for the upper and lower bounds.\n\nImportant: When querying for the price, always use gr:hasMaxCurrencyValue and gr:hasMinCurrencyValue.\n\nNote 1: Due to the complexity of pricing scenarios in various industries, it may be necessary to create extensions of this fundamental model of price specifications. Such can be done easily by importing and refining the GoodRelations ontology.\n\nNote 2: For Google, attaching a gr:validThrough statement to a gr:UnitPriceSpecification is mandatory. \n"@en ;
        rdfs:isDefinedBy  <http://purl.org/goodrelations/v1> ;
        rdfs:label        "Unit price specification"@en ;
        rdfs:subClassOf   gr:PriceSpecification ;
        owl:disjointWith  gr:PaymentChargeSpecification , gr:DeliveryChargeSpecification .

usdl-testing:withGoal
        a                 rdf:Property ;
        rdfs:comment      "<p>Connects TestingMethod to TestingGoal classification dimension.</p>"@en ;
        rdfs:domain       usdl-testing:TestingMethod ;
        rdfs:isDefinedBy  <http://www.linked-usdl.org/ns/usdl-core/cloud-broker/testing> ;
        rdfs:label        "with goal"@en ;
        rdfs:range        usdl-testing:TestingGoal .

gr:Friday  a                gr:DayOfWeek ;
        rdfs:comment        "Friday as a day of the week."@en ;
        rdfs:isDefinedBy    <http://purl.org/goodrelations/v1> ;
        rdfs:label          "Friday (day of week)"@en ;
        gr:displayPosition  5 ;
        gr:hasNext          gr:Saturday ;
        gr:hasPrevious      gr:Thursday .

s:Offer  a               owl:Class ;
        rdfs:subClassOf  gr:Offering .

attr:attr-performance-capacity-storage-capacity
        a                    usdl-pref:ServiceAttribute ;
        dcterms:created      "2014-07-18T11:58:03Z"^^xsd:dateTime ;
        dcterms:creator      ""^^xsd:string ;
        dcterms:description  ""^^xsd:string ;
        dcterms:identifier   "attr-performance-capacity-storage-capacity"^^xsd:string ;
        dcterms:modified     "2014-07-18T11:58:03Z"^^xsd:dateTime ;
        dcterms:title        "Storage Capacity"^^xsd:string ;
        skos:broader         attr:attr-performance-capacity .

usdl-core:withBusinessRole
        a                 rdf:Property ;
        rdfs:comment      "<p>Captures the BusinessRole played by a BusinessEntity in a particular EntityInvolvement or EntityInteraction. For instance the entity involved could be the actual service Deliverer, etc.</p>"@en ;
        rdfs:domain       [ a            owl:Class ;
                            owl:unionOf  ( usdl-core:EntityInvolvement usdl-core:EntityInteraction )
                          ] ;
        rdfs:isDefinedBy  <http://www.linked-usdl.org/ns/usdl-core> ;
        rdfs:label        "with business role"@en ;
        rdfs:range        usdl-core:BusinessRole .

usdl-testing:hasTestingProvider
        a                 rdf:Property ;
        rdfs:comment      "<p>Connects TestingProcedure to a business entity describing the provider of the TestingProcedure.</p>"@en ;
        rdfs:domain       usdl-testing:TestingProcedure ;
        rdfs:isDefinedBy  <http://www.linked-usdl.org/ns/usdl-core/cloud-broker/testing> ;
        rdfs:label        "has testing provider"@en ;
        rdfs:range        gr:BusinessEntity .

dc:rights  a    owl:AnnotationProperty .

gr:quantitativeProductOrServiceProperty
        a                 owl:ObjectProperty ;
        rdfs:comment      "This is the super property of all quantitative  properties for products and services. All properties in product or service ontologies that specify quantitative characteristics, for which an interval is at least theoretically an appropriate value, are subproperties of this property."@en ;
        rdfs:domain       [ a            owl:Class ;
                            owl:unionOf  ( gr:ProductOrService s:Product )
                          ] ;
        rdfs:isDefinedBy  <http://purl.org/goodrelations/v1> ;
        rdfs:label        "quantitative product or service property (0..*)"@en ;
        rdfs:range        gr:QuantitativeValue .

<http://www.linked-usdl.org/ns/usdl-core/cloud-broker/testing>
        a                              owl:Ontology ;
        rdfs:label                     "Linked USDL Cloud Broker Testing"@en ;
        dcterms:created                "2014-11-05"^^xsd:date ;
        dcterms:creator                usdl-testing:afriesen ;
        dcterms:description            "<p>This vocabulary provides a Broker@Cloud extension to the core module of Linked USDL for integration of testing specification into service descriptions. It provides support for classification of testing methods and identification of providers offering testing services. This specification is intended to be quite general in its support for describing testing methods that range from informal to highly formal approaches.</p>"@en ;
        dcterms:issued                 "2014-11-05"^^xsd:date ;
        dcterms:modified               "2014-09-30"^^xsd:date ;
        dcterms:title                  "Linked USDL Cloud Broker Testing"@en ;
        vann:preferredNamespacePrefix  "usdl-testing" ;
        vann:preferredNamespaceUri     "http://www.linked-usdl.org/ns/usdl-core/cloud-broker/testing#" ;
        owl:versionInfo                "1.0" .

attr:attr-usability-client-personnel-requirements
        a                    usdl-pref:ServiceAttribute ;
        dcterms:created      "2014-07-18T16:00:27+03:00"^^xsd:dateTime ;
        dcterms:description  "The minimum number of personnel satisfying roles, skills, experience, education, and certification required of the client to effectively utilize a service"^^xsd:string ;
        dcterms:identifier   "attr-usability-client-personnel-requirements"^^xsd:string ;
        dcterms:modified     "2014-07-18T16:00:27+03:00"^^xsd:dateTime ;
        dcterms:title        "Client Personnel Requirements"^^xsd:string ;
        skos:broader         attr:attr-usability .

gr:Reseller  a            gr:BusinessEntityType ;
        rdfs:comment      "The gr:BusinessEntityType representing such agents that are purchasing the scope of products included in the gr:Offering for resale on the market. Resellers are also businesses, i.e., they are officially registered with the public administration and strive for profits by their activities."@en ;
        rdfs:isDefinedBy  <http://purl.org/goodrelations/v1> ;
        rdfs:label        "Reseller (business entity type)"@en .

gr:eligibleRegions  a     owl:DatatypeProperty ;
        rdfs:comment      "This property specifies the geo-political region or regions for which the gr:Offering, gr:License, or gr:DeliveryChargeSpecification is valid using the two-character version of ISO 3166-1 (ISO 3166-1 alpha-2)  for regions or ISO 3166-2 , which breaks down the countries from ISO 3166-1 into administrative subdivisions.\n\nImportant: Do NOT use 3-letter ISO 3166-1 codes!"@en ;
        rdfs:domain       [ a            owl:Class ;
                            owl:unionOf  ( gr:DeliveryChargeSpecification gr:Offering gr:License s:Offer )
                          ] ;
        rdfs:isDefinedBy  <http://purl.org/goodrelations/v1> ;
        rdfs:label        "eligible regions (0..*)"@en ;
        rdfs:range        xsd:string .

usdl-core:withInteractionRole
        a                 rdf:Property ;
        rdfs:comment      "<p>Captures the InteractionRole played by a BusinessEntity type in a particular InteractionPoint (e.g., Initiator, etc).</p>"@en ;
        rdfs:domain       usdl-core:EntityInteraction ;
        rdfs:isDefinedBy  <http://www.linked-usdl.org/ns/usdl-core> ;
        rdfs:label        "has business role"@en ;
        rdfs:range        usdl-core:InteractionRole .

attr:attr-reputation-provider-ethicality
        a                    usdl-pref:ServiceAttribute ;
        dcterms:created      "2014-07-18T13:33:42Z"^^xsd:dateTime ;
        dcterms:creator      ""^^xsd:string ;
        dcterms:description  "Ethicality refers to the manner in which the service provider conducts business; it includes business practices and ethics outside the scope of regulatory compliance. It also includes fair practices with suppliers, customers, and employees"^^xsd:string ;
        dcterms:identifier   "attr-reputation-provider-ethicality"^^xsd:string ;
        dcterms:modified     "2014-07-18T13:33:42Z"^^xsd:dateTime ;
        dcterms:title        "Provider Ethicality"^^xsd:string ;
        skos:broader         attr:attr-reputation .

gr:hasOpeningHoursDayOfWeek
        a                 owl:ObjectProperty ;
        rdfs:comment      "This specifies the gr:DayOfWeek to which the gr:OpeningHoursSpecification is related.\n\nNote: Use multiple instances of gr:OpeningHoursSpecification for specifying the opening hours for multiple days if the opening hours differ."@en ;
        rdfs:domain       gr:OpeningHoursSpecification ;
        rdfs:isDefinedBy  <http://purl.org/goodrelations/v1> ;
        rdfs:label        "has opening hours day of week (1..*)"@en ;
        rdfs:range        gr:DayOfWeek .

attr:attr-performance-service-response-time-average-value
        a                    usdl-pref:ServiceAttribute ;
        dcterms:created      "2014-05-23T21:34:16+03:00"^^xsd:dateTime ;
        dcterms:description  ""^^xsd:string ;
        dcterms:identifier   "attr-performance-service-response-time-average-value"^^xsd:string ;
        dcterms:modified     "2014-07-18T15:05:21+03:00"^^xsd:dateTime ;
        dcterms:title        "Average Response time"^^xsd:string ;
        skos:broader         attr:attr-performance-service-response-time .

gr:ConstructionInstallation
        a                 gr:BusinessFunction ;
        rdfs:comment      "This gr:BusinessFunction indicates that the gr:BusinessEntity offers (or seeks) the construction and/or installation of the specified gr:ProductOrService at the customer's location."@en ;
        rdfs:isDefinedBy  <http://purl.org/goodrelations/v1> ;
        rdfs:label        "Construction / installation (business function)"@en .

dc:title  a     owl:AnnotationProperty .

gr:Buy  a                 gr:BusinessFunction ;
        rdfs:comment      "This gr:BusinessFunction indicates that the gr:BusinessEntity is in general interested in purchasing the specified gr:ProductOrService.\nDEPRECATED. Use gr:seeks instead."@en ;
        rdfs:isDefinedBy  <http://purl.org/goodrelations/v1> ;
        rdfs:label        "Buy (business function, DEPRECATED)"@en ;
        owl:deprecated    true .

<http://www.linked-usdl.org/ns/manual>
        a                  usdl-core:InteractionType ;
        rdfs:label         "Manual"@en ;
        skos:altLabel      "Manual Interaction"@en ;
        skos:definition    "<p>The interaction between the two parties is entirely manual.</p>"@en ;
        skos:inScheme      <http://www.linked-usdl.org/ns/usdl-interaction-types> ;
        skos:prefLabel     "Manual"@en ;
        skos:topConceptOf  <http://www.linked-usdl.org/ns/usdl-interaction-types> .

attr:attr-security-management-transport-security-guarantees
        a                    usdl-pref:ServiceAttribute ;
        dcterms:created      "2015-09-08T10:42:33.043+03:00"^^xsd:dateTime ;
        dcterms:description  "Defines the level of transport security"^^xsd:string ;
        dcterms:identifier   "attr-security-management-transport-security-guarantees"^^xsd:string ;
        dcterms:modified     "2015-09-08T10:42:33.043+03:00"^^xsd:dateTime ;
        dcterms:title        "Transport Security Guarantees"^^xsd:string ;
        skos:broader         attr:attr-security-management .

usdl-pref:ConsumerPreferenceProfile
        a                 owl:Class , rdfs:Class ;
        rdfs:comment      "<p>A ConsumerPreferenceProfile might reference one or more consumer preferences. ConsumerPreferenceProfile is associated to a FunctionalServiceCategory. </p> " ;
        rdfs:isDefinedBy  <http://www.linked-usdl.org/ns/usdl-pref> ;
        rdfs:label        "Consumer Preference Profile" .

usdl-pref:hasDefaultFuzzyValue
        a                 rdf:Property ;
        rdfs:comment      "<p>The fuzzy value of a preference variable.</p>\r\n" ;
        rdfs:domain       usdl-pref:FuzzyVariable ;
        rdfs:isDefinedBy  <http://www.linked-usdl.org/ns/usdl-pref> ;
        rdfs:label        "has default fuzzy value" ;
        rdfs:range        usdl-sla-cb:FuzzyValue .

attr:attr-financial-cost
        a                    usdl-pref:ServiceAttribute ;
        dcterms:created      "2014-05-23T21:19:47+03:00"^^xsd:dateTime ;
        dcterms:description  ""^^xsd:string ;
        dcterms:identifier   "attr-financial-cost"^^xsd:string ;
        dcterms:modified     "2014-05-23T21:19:47+03:00"^^xsd:dateTime ;
        dcterms:title        "Cost"^^xsd:string ;
        skos:broader         attr:attr-financial .

attr:attr-security-access-control-privilege-management
        a                    usdl-pref:ServiceAttribute ;
        dcterms:created      "2014-07-18T12:50:58Z"^^xsd:dateTime ;
        dcterms:creator      ""^^xsd:string ;
        dcterms:description  "Policies and processes in use by the service provider to ensure that only the provider and client personnel with appropriate status/reasons to make use of or modify data/work products may do so"^^xsd:string ;
        dcterms:identifier   "attr-security-access-control-privilege-management"^^xsd:string ;
        dcterms:modified     "2014-07-18T12:50:58Z"^^xsd:dateTime ;
        dcterms:title        "Access Control & Privilege Management"^^xsd:string ;
        skos:broader         attr:attr-security .

gr:Offering  a            owl:Class ;
        rdfs:comment      "An offering represents the public, not necessarily binding, not necessarily exclusive, announcement by a gr:BusinessEntity to provide (or seek) a certain gr:BusinessFunction for a certain gr:ProductOrService to a specified target audience. An offering is specified by the type of product or service or bundle it refers to, what business function is being offered (sales, rental, ...), and a set of commercial properties. It can either refer to \n(1) a clearly specified instance (gr:Individual),\n(2) to a set of anonymous instances of a given type (gr:SomeItems),\n(3) a product model specification (gr:ProductOrServiceModel), see also section 3.3.3 of the GoodRelations Technical Report. \n\nAn offering may be constrained in terms of the eligible type of business partner, countries, quantities, and other commercial properties. The definition of the commercial properties, the type of product offered, and the business function are explained in other parts of this vocabulary in more detail.\n\nExample: Peter Miller offers to repair TV sets made by Siemens, Volkswagen Innsbruck sells a particular instance of a Volkswagen Golf at $10,000.\n\nCompatibility with schema.org: This class is a superclass to http://schema.org/Offer, since gr:Offering can also represent demand."@en ;
        rdfs:isDefinedBy  <http://purl.org/goodrelations/v1> ;
        rdfs:label        "Offering"@en ;
        owl:disjointWith  gr:OpeningHoursSpecification , gr:WarrantyPromise , gr:Brand , gr:QuantitativeValue , gr:BusinessFunction , gr:BusinessEntityType , gr:PriceSpecification , gr:DayOfWeek , gr:TypeAndQuantityNode , gr:BusinessEntity , gr:PaymentMethod , gr:DeliveryMethod , gr:Location , gr:QualitativeValue , gr:ProductOrService , gr:WarrantyScope .

usdl-core:cpedrinaci  a  foaf:Person ;
        foaf:homepage  <http://www.cpedrinaci.net> ;
        foaf:name      "Carlos Pedrinaci" .

<http://www.linked-usdl.org/ns/usdl-interaction-roles>
        a                              owl:Ontology , skos:ConceptScheme ;
        dcterms:creator                usdl-core:tleidig , usdl-core:jcardoso , usdl-core:cpedrinaci ;
        dcterms:description            "<p>This vocabulary provides the core interaction roles contemplated within Linked USDL. The taxonomy provided here is a minimal reference one. Extensions or replacements for this could be defined an used within applications in the very same way by refining InteractionRole or creating further SKOS concept schemes. </p>"@en ;
        dcterms:modified               "2013-02-11"^^xsd:date , "2014-01-14"^^xsd:date ;
        dcterms:title                  "Linked USDL Basic Interaction Roles concept scheme" ;
        vann:preferredNamespacePrefix  "usdl-ir" ;
        vann:preferredNamespaceUri     "http://www.linked-usdl.org/ns/usdl-interaction-roles#" ;
        skos:hasTopConcept             <http://www.linked-usdl.org/ns/participant> , <http://www.linked-usdl.org/ns/observer> ;
        skos:prefLabel                 "Interaction Roles"@en ;
        foaf:page                      <http://www.linked-usdl.org/ns/usdl-interaction-roles.html> .

usdl-pref:hasPreferenceExpression
        a                 rdf:Property ;
        rdfs:comment      "<p>Consumer preference expressions.</p>\r\n" ;
        rdfs:domain       usdl-pref:ConsumerPreference ;
        rdfs:isDefinedBy  <http://www.linked-usdl.org/ns/usdl-pref> ;
        rdfs:label        "has preference expression" ;
        rdfs:range        usdl-pref:ConsumerPreferenceExpression .

usdl-sla-cb:isRange  a    rdf:Property ;
        rdfs:comment      "<p>Indicates if an instance of a value class is a numeric or fuzzy range rather than a single value if the value is true. If the value is false only single values have to be provided in the service description. </p>"@en ;
        rdfs:domain       gr:QuantitativeValue ;
        rdfs:isDefinedBy  usdl-core-cb: ;
        rdfs:label        "instance of a value class is a range rather than a single value"@en ;
        rdfs:range        xsd:boolean .

usdl-sla-cb:hasServiceModel
        a                 rdf:Property ;
        rdfs:comment      "<p>Connects Service to a ServiceModel.</p>"@en ;
        rdfs:domain       usdl-core:Service ;
        rdfs:isDefinedBy  usdl-core-cb: ;
        rdfs:label        "has classification dimension"@en ;
        rdfs:range        usdl-core:ServiceModel .

usdl-core:hasEntityInteraction
        a                 rdf:Property ;
        rdfs:comment      "<p>Captures the involvement of BusinessEntities within a particular Interaction.</p>"@en ;
        rdfs:domain       usdl-core:InteractionPoint ;
        rdfs:isDefinedBy  <http://www.linked-usdl.org/ns/usdl-core> ;
        rdfs:label        "has entity interaction"@en ;
        rdfs:range        usdl-core:EntityInteraction .

gr:eligibleDuration  a    owl:ObjectProperty ;
        rdfs:comment      "The minimal and maximal duration for which the given gr:Offering or gr:License is valid. This is mostly used for offers regarding accommodation, the rental of objects, or software licenses. The duration is specified by attaching an instance of gr:QuantitativeValue. The lower and upper boundaries are specified using the properties gr:hasMinValue and gr:hasMaxValue to that instance. If they are the same, use the gr:hasValue property. The unit of measurement is specified using the property gr:hasUnitOfMeasurement with a string holding a UN/CEFACT code suitable for durations, e.g. MON (months), DAY (days), HUR (hours), or MIN (minutes).\n\nThe difference to the gr:validFrom and gr:validThrough properties is that those specify the absiolute interval during which the gr:Offering or gr:License is valid, while gr:eligibleDuration specifies the acceptable duration of the contract or usage."@en ;
        rdfs:domain       [ a            owl:Class ;
                            owl:unionOf  ( gr:Offering gr:License s:Offer )
                          ] ;
        rdfs:isDefinedBy  <http://purl.org/goodrelations/v1> ;
        rdfs:label        "eligible duration (0..1)"@en ;
        rdfs:range        gr:QuantitativeValue .

gr:isSimilarTo  a         owl:ObjectProperty ;
        rdfs:comment      "This states that a given gr:ProductOrService is similar to another product or service. Of course, this is a subjective statement; when interpreting it, the trust in the origin of the statement should be taken into account."@en ;
        rdfs:domain       [ a            owl:Class ;
                            owl:unionOf  ( gr:ProductOrService s:Product )
                          ] ;
        rdfs:isDefinedBy  <http://purl.org/goodrelations/v1> ;
        rdfs:label        "is similar to (0..*)"@en ;
        rdfs:range        gr:ProductOrService .

usdl-core:hasCommunicationChannel
        a                 rdf:Property ;
        rdfs:comment      "<p>InteractionPoints can have several CommunicationChannels, i.e., ways for interacting like the phone, email, etc. </p>"@en ;
        rdfs:domain       usdl-core:InteractionPoint ;
        rdfs:isDefinedBy  <http://www.linked-usdl.org/ns/usdl-core> ;
        rdfs:label        "has communication channel"@en ;
        rdfs:range        usdl-core:CommunicationChannel .

attr:attr-financial-cost-data-inbound
        a                    usdl-pref:ServiceAttribute ;
        dcterms:created      "2014-05-23T18:32:20Z"^^xsd:dateTime ;
        dcterms:creator      ""^^xsd:string ;
        dcterms:description  ""^^xsd:string ;
        dcterms:identifier   "attr-financial-cost-data-inbound"^^xsd:string ;
        dcterms:modified     "2014-07-18T09:25:29Z"^^xsd:dateTime ;
        dcterms:title        "Data - Inbound"^^xsd:string ;
        skos:broader         attr:attr-financial-cost .

gr:LocationOfSalesOrServiceProvisioning
        a                    owl:Class ;
        rdfs:comment         "DEPRECATED - This class is superseded by gr:Location. Replace all occurrences of gr:LocationOfSalesOrServiceProvisioning by gr:Location, if possible."@en ;
        rdfs:isDefinedBy     <http://purl.org/goodrelations/v1> ;
        rdfs:label           "Location of sales or service provisioning (DEPRECATED)"@en ;
        owl:deprecated       true ;
        owl:equivalentClass  gr:Location .

usdl-core:spansInterval
        a                 rdf:Property ;
        rdfs:comment      "<p>Captures the fact that an Interaction Point spans an interval of time.</p>"@en ;
        rdfs:domain       usdl-core:InteractionPoint ;
        rdfs:isDefinedBy  <http://www.linked-usdl.org/ns/usdl-core> ;
        rdfs:label        "spans interval"@en ;
        rdfs:range        time:Interval .

gr:hasValueInteger  a       owl:DatatypeProperty ;
        rdfs:comment        "This subproperty specifies that the upper and lower limit of the given gr:QuantitativeValueInteger are identical and have the respective integer value. It is a shortcut for such cases where a quantitative property is (at least practically) a single point value and not an interval."@en ;
        rdfs:domain         gr:QuantitativeValueInteger ;
        rdfs:isDefinedBy    <http://purl.org/goodrelations/v1> ;
        rdfs:label          "has value integer (0..1)"@en ;
        rdfs:range          xsd:int ;
        rdfs:subPropertyOf  gr:hasMinValueInteger , gr:hasMaxValueInteger .

gr:PartsAndLabor-BringIn
        a                 gr:WarrantyScope ;
        rdfs:comment      "In case of a defect or malfunction, the buying party has the right to transport the good to a service location determined by the the selling gr:BusinessEntity and will not be be charged for labor, parts, and materials needed to fix the problem. All those costs will be covered by the selling business entity or one of its partnering business entities.\n\nNote: This is just a rough classification for filtering offers. It is up to the buying party to check the exact scope and terms and conditions of the gr:WarrantyPromise."@en ;
        rdfs:isDefinedBy  <http://purl.org/goodrelations/v1> ;
        rdfs:label        "Parts and labor / bring-in (warranty scope)"@en .

attr:attr-performance-capacity-concurrent-vm-instances
        a                    usdl-pref:ServiceAttribute ;
        dcterms:created      "2015-09-08T10:38:08.505+03:00"^^xsd:dateTime ;
        dcterms:description  "Amount of working containers able to handle execution load of the service"^^xsd:string ;
        dcterms:identifier   "attr-performance-capacity-concurrent-vm-instances"^^xsd:string ;
        dcterms:modified     "2015-09-08T10:38:08.505+03:00"^^xsd:dateTime ;
        dcterms:title        "Amount of Concurrent VM Instances"^^xsd:string ;
        skos:broader         attr:attr-performance-capacity .

usdl-pref:jverginadis
        a          foaf:Person ;
        foaf:name  "Yiannis Verginadis" .

attr:attr-usability-reusability
        a                    usdl-pref:ServiceAttribute ;
        dcterms:created      "2014-07-18T16:25:27+03:00"^^xsd:dateTime ;
        dcterms:description  "How generic the service is and how easy it is to be used in different cloud applications"^^xsd:string ;
        dcterms:identifier   "attr-usability-reusability"^^xsd:string ;
        dcterms:modified     "2014-07-18T16:25:27+03:00"^^xsd:dateTime ;
        dcterms:title        "Reusability"^^xsd:string ;
        skos:broader         attr:attr-usability .

<http://www.linked-usdl.org/ns/regulator>
        a                  usdl-core:BusinessRole ;
        rdfs:label         "Regulator"@en ;
        skos:altLabel      "Regulation Body"@en ;
        skos:definition    "<p>A Regulator is a third party entity, often governmental, that is in charge of ensuring the adequate application of regulations and best practices. Tracking this information allows one to know the entity one can revolve to in order to deal with concrete problems or simply to have an added garanty that proper control is exercised over a given business activity.</p>"@en ;
        skos:inScheme      <http://www.linked-usdl.org/ns/usdl-business-roles> ;
        skos:prefLabel     "Regulator"@en ;
        skos:topConceptOf  <http://www.linked-usdl.org/ns/usdl-business-roles> .

gr:hasGlobalLocationNumber
        a                 owl:DatatypeProperty ;
        rdfs:comment      "The Global Location Number (GLN, sometimes also referred to as International Location Number or ILN) of the respective gr:BusinessEntity or gr:Location.\nThe Global Location Number is a thirteen-digit number used to identify parties and physical locations."@en ;
        rdfs:domain       [ a            owl:Class ;
                            owl:unionOf  ( gr:BusinessEntity gr:Location s:Place s:Organization )
                          ] ;
        rdfs:isDefinedBy  <http://purl.org/goodrelations/v1> ;
        rdfs:label        "has Global Location Number (0..1)"@en ;
        rdfs:range        xsd:string .

usdl-testing:ModelBasedTesting
        a                  usdl-testing:TestAdequacyCriteria ;
        rdfs:label         "Model-based Testing"@en ;
        skos:altLabel      "Model-based Testing"@en ;
        skos:definition    "<p>A testing method is a model-based testing method.</p>"@en ;
        skos:inScheme      usdl-testing:TestAdequacyCriteriaClassificationScheme ;
        skos:prefLabel     "Model-based Testing"@en ;
        skos:topConceptOf  usdl-testing:TestAdequacyCriteriaClassificationScheme .

gr:LeaseOut  a            gr:BusinessFunction ;
        rdfs:comment      "This gr:BusinessFunction indicates that the gr:BusinessEntity offers (or seeks) the temporary right to use the specified gr:ProductOrService."@en ;
        rdfs:isDefinedBy  <http://purl.org/goodrelations/v1> ;
        rdfs:label        "Lease Out (business function)"@en .

gr:AmericanExpress  a     gr:PaymentMethodCreditCard ;
        rdfs:comment      "Payment by credit or debit cards issued by the American Express network."@en ;
        rdfs:isDefinedBy  <http://purl.org/goodrelations/v1> ;
        rdfs:label        "American Express (payment method)"@en .

attr:attr-accountability-compliance
        a                    usdl-pref:ServiceAttribute ;
        dcterms:created      "2014-07-18T07:30:22Z"^^xsd:dateTime ;
        dcterms:creator      ""^^xsd:string ;
        dcterms:description  "It examines whether or not, standards, processes, and policies committed to by the service provider, are followed"^^xsd:string ;
        dcterms:identifier   "attr-accountability-compliance"^^xsd:string ;
        dcterms:modified     "2014-07-18T07:30:22Z"^^xsd:dateTime ;
        dcterms:title        "Compliance"^^xsd:string ;
        skos:broader         attr:attr-accountability .

usdl-core:CISUC  a     foaf:Organization ;
        foaf:homepage  <http://www.dei.uc.pt> ;
        foaf:member    usdl-core:jcardoso ;
        foaf:name      "CISUC/DEI, University of Coimbra" .

gr:valueReference  a      owl:ObjectProperty ;
        rdfs:comment      "The superclass of properties that link a gr:QuantitativeValue or a gr:QualitativeValue to a second gr:QuantitativeValue or a gr:QualitativeValue that provides additional information on the original value. A good modeling practice is to define specializations of this property (e.g. foo:referenceTemperature) for your particular domain."@en ;
        rdfs:domain       [ a            owl:Class ;
                            owl:unionOf  ( gr:QualitativeValue gr:QuantitativeValue )
                          ] ;
        rdfs:isDefinedBy  <http://purl.org/goodrelations/v1> ;
        rdfs:label        "value reference (0..*)"@en ;
        rdfs:range        [ a            owl:Class ;
                            owl:unionOf  ( gr:QualitativeValue gr:QuantitativeValue )
                          ] .

attr:attr-performance-service-response-time
        a                    usdl-pref:ServiceAttribute ;
        dcterms:created      "2014-05-23T18:33:18Z"^^xsd:dateTime ;
        dcterms:creator      ""^^xsd:string ;
        dcterms:description  "An indicator of the time between when a service is requested and when the response is available"^^xsd:string ;
        dcterms:identifier   "attr-performance-service-response-time"^^xsd:string ;
        dcterms:modified     "2014-07-18T12:04:24Z"^^xsd:dateTime ;
        dcterms:title        "Service Response Time"^^xsd:string ;
        skos:broader         attr:attr-performance .

<http://www.linked-usdl.org/ns/consumer>
        a                  usdl-core:BusinessRole ;
        rdfs:label         "Consumer"@en ;
        owl:sameAs         gr:EndUser ;
        skos:altLabel      "End-user"@en ;
        skos:definition    "<p>A Consumer is the actual end-user benefiting from a Service. In many cases this will coincide with the Customer (i.e., the entity that contracted the service), but this is not necessarily the case. For instance, travel insurances for workers are typically contracted by the company but it is the actual workers that benefit from it. Similarly a car insurance may be contracted by a member of a family and used by all the drivers in the family.</p>"@en ;
        skos:inScheme      <http://www.linked-usdl.org/ns/usdl-business-roles> ;
        skos:prefLabel     "Consumer"@en ;
        skos:topConceptOf  <http://www.linked-usdl.org/ns/usdl-business-roles> .

s:productID  a  owl:DatatypeProperty .

<http://www.linked-usdl.org/ns/usdl-core>
        a                              owl:Ontology ;
        rdfs:label                     "Linked USDL Core"@en ;
        dcterms:created                "2012-09-20"^^xsd:date ;
        dcterms:creator                usdl-core:cpedrinaci , usdl-core:jcardoso , usdl-core:tleidig ;
        dcterms:description            "<p>This vocabulary provides the core module of Linked USDL. It therefore covers the main concepts and properties characterising services, leaving more specific aspects regarding some particular dimensions such as technical interfaces, licensing or security aside. These aspects will be covered in additional modules, or &nbsp;in some cases, like the technical interfaces, by existing vocabularies.</p>\r\n<p>This first draft includes most of the original USDL specification with some useful simplifications. </p>"@en ;
        dcterms:issued                 "2014-01-14"^^xsd:date ;
        dcterms:modified               "2013-03-08"^^xsd:date , "2013-03-07"^^xsd:date , "2012-09-20"^^xsd:date , "2013-12-10"^^xsd:date , "2013-08-29"^^xsd:date , "2014-01-14"^^xsd:date , "2013-03-06"^^xsd:date ;
        dcterms:title                  "Linked USDL Core"@en ;
        vann:preferredNamespacePrefix  "usdl" ;
        vann:preferredNamespaceUri     "http://www.linked-usdl.org/ns/usdl-core#" ;
        owl:versionInfo                "1.0" ;
        foaf:page                      <http://www.linked-usdl.org/ns/usdl-core.html> .

gr:isVariantOf  a         owl:ObjectProperty ;
        rdfs:comment      "This states that a particular gr:ProductOrServiceModel is a variant of another product or service model. It is pretty safe to infer that the variant inherits all gr:quantitativeProductOrServiceProperty, gr:qualitativeProductOrServiceProperty, and gr:datatypeProductOrServiceProperty values that are defined for the first gr:ProductOrServiceModel.\n\nExample:\nfoo:Red_Ford_T_Model gr:isVariantOf foo:Ford_T_Model"@en ;
        rdfs:domain       gr:ProductOrServiceModel ;
        rdfs:isDefinedBy  <http://purl.org/goodrelations/v1> ;
        rdfs:label        "is variant of (0..1)"@en ;
        rdfs:range        gr:ProductOrServiceModel .

attr:attr-agility-extensibility
        a                    usdl-pref:ServiceAttribute ;
        dcterms:created      "2014-07-18T08:13:55Z"^^xsd:dateTime ;
        dcterms:creator      ""^^xsd:string ;
        dcterms:description  "The ability to add new features or services to existing services"^^xsd:string ;
        dcterms:identifier   "attr-agility-extensibility"^^xsd:string ;
        dcterms:modified     "2014-07-18T08:13:55Z"^^xsd:dateTime ;
        dcterms:title        "Extensibility"^^xsd:string ;
        skos:broader         attr:attr-agility .

gr:BusinessEntity  a         owl:Class ;
        rdfs:comment         "An instance of this class represents the legal agent making (or seeking) a particular offering. This can be a legal body or a person. A business entity has at least a primary mailing address and contact details. For this, typical address standards (vCard) and location data (geo, WGS84) can be attached. Note that the location of the business entity is not necessarily the location from which the product or service is being available (e.g. the branch or store). Use gr:Location for stores and branches.\n\t\t\nExample: Siemens Austria AG, Volkswagen Ltd., Peter Miller's Cell phone Shop LLC\n\nCompatibility with schema.org: This class is equivalent to the union of http://schema.org/Person and http://schema.org/Organization.\t\t\n"@en ;
        rdfs:isDefinedBy     <http://purl.org/goodrelations/v1> ;
        rdfs:label           "Business entity"@en ;
        rdfs:subClassOf      vcard:Kind ;
        owl:disjointWith     gr:Offering , gr:WarrantyPromise , gr:PriceSpecification , gr:TypeAndQuantityNode , gr:Location , gr:WarrantyScope , gr:BusinessFunction , gr:OpeningHoursSpecification , gr:DeliveryMethod , gr:QuantitativeValue , gr:BusinessEntityType , gr:Brand , gr:PaymentMethod , gr:DayOfWeek ;
        owl:equivalentClass  [ a            owl:Class ;
                               owl:unionOf  ( s:Person s:Organization )
                             ] .

attr:attr-reputation-provider-business-stability
        a                    usdl-pref:ServiceAttribute ;
        dcterms:created      "2014-07-18T16:33:22+03:00"^^xsd:dateTime ;
        dcterms:description  "The likelihood that the service provider will continue to exist throughout the contracted term"^^xsd:string ;
        dcterms:identifier   "attr-reputation-provider-business-stability"^^xsd:string ;
        dcterms:modified     "2014-07-18T16:33:22+03:00"^^xsd:dateTime ;
        dcterms:title        "Provider business stability"^^xsd:string ;
        skos:broader         attr:attr-reputation .

attr:attr-assurance-serviceability-type-of-support
        a                    usdl-pref:ServiceAttribute ;
        dcterms:created      "2014-05-23T21:30:19+03:00"^^xsd:dateTime ;
        dcterms:description  ""^^xsd:string ;
        dcterms:identifier   "attr-assurance-serviceability-type-of-support"^^xsd:string ;
        dcterms:modified     "2014-05-23T21:30:19+03:00"^^xsd:dateTime ;
        dcterms:title        "Type of Support"^^xsd:string ;
        skos:broader         attr:attr-assurance-serviceability .

attr:attr-security-physical-environmental-security
        a                    usdl-pref:ServiceAttribute ;
        dcterms:created      "2014-07-18T15:54:37+03:00"^^xsd:dateTime ;
        dcterms:creator      ""^^xsd:string ;
        dcterms:description  "Policies and processes in use by the service provider to protect the provider facilities from unauthorized access, damage or interference"^^xsd:string ;
        dcterms:identifier   "attr-security-physical-environmental-security"^^xsd:string ;
        dcterms:modified     "2014-07-18T15:54:37+03:00"^^xsd:dateTime ;
        dcterms:title        "Physical & Environmental Security"^^xsd:string ;
        skos:broader         attr:attr-security .

usdl-pref:hasDefaultQualitativeValue
        a                 rdf:Property ;
        rdfs:comment      "<p>The qualitative value of a preference variable.</p>\r\n" ;
        rdfs:domain       usdl-pref:QualitativeVariable ;
        rdfs:isDefinedBy  <http://www.linked-usdl.org/ns/usdl-pref> ;
        rdfs:label        "has default qualitative value" ;
        rdfs:range        gr:QualitativeValue .

gr:category  a            owl:DatatypeProperty ;
        rdfs:comment      "The name of a category to which this gr:ProductOrService, gr:Offering, gr:BusinessEntity, or gr:Location belongs.\n\t\nNote 1: For products, it is better to add an rdf:type statement referring to a GoodRelations-compliant ontology for vertical industries instead, but if you just have a short text label, gr:category is simpler.\nNote 2: You can use greater signs or slashes to informally indicate a category hierarchy, e.g. \"restaurants/asian_restaurants\" or \"cables > usb_cables\"\n"@en ;
        rdfs:domain       [ a            owl:Class ;
                            owl:unionOf  ( gr:ProductOrService gr:Offering gr:Location gr:BusinessEntity s:Offer s:Product s:Place s:Organization )
                          ] ;
        rdfs:isDefinedBy  <http://purl.org/goodrelations/v1> ;
        rdfs:label        "category (0..*)"@en ;
        rdfs:range        rdfs:Literal .

usdl-pref:hasDefaultDatatypeValue
        a                 rdf:Property ;
        rdfs:comment      "<p>The datatype value of a preference variable.</p>\r\n" ;
        rdfs:domain       usdl-pref:DatatypeVariable ;
        rdfs:isDefinedBy  <http://www.linked-usdl.org/ns/usdl-pref> ;
        rdfs:label        "has default datatype value" ;
        rdfs:range        rdfs:Datatype .

gr:DHL  a                 gr:DeliveryModeParcelService ;
        rdfs:comment      "Delivery via the parcel service DHL."@en ;
        rdfs:isDefinedBy  <http://purl.org/goodrelations/v1> ;
        rdfs:label        "DHL (delivery method)"@en .

attr:attr-agility-scalability
        a                    usdl-pref:ServiceAttribute ;
        dcterms:created      "2014-07-18T08:16:59Z"^^xsd:dateTime ;
        dcterms:creator      ""^^xsd:string ;
        dcterms:description  "The ability of a service provider to increase or decrease the amount of service available to meet client requirements"^^xsd:string ;
        dcterms:identifier   "attr-agility-scalability"^^xsd:string ;
        dcterms:modified     "2014-07-18T08:16:59Z"^^xsd:dateTime ;
        dcterms:title        "Scalability"^^xsd:string ;
        skos:broader         attr:attr-agility .

gr:ByBankTransferInAdvance
        a                 gr:PaymentMethod ;
        rdfs:comment      "Payment by bank transfer in advance, i.e., the offering gr:BusinessEntity will inform the buying party about their bank account details and will deliver the goods upon receipt of the due amount.\nThis is equivalent to payment by wire transfer."@en ;
        rdfs:isDefinedBy  <http://purl.org/goodrelations/v1> ;
        rdfs:label        "By bank transfer in advance (payment method)"@en .

attr:attr-reputation-sustainability
        a                    usdl-pref:ServiceAttribute ;
        dcterms:created      "2014-07-18T16:34:01+03:00"^^xsd:dateTime ;
        dcterms:description  "The impact on the economy, society and the environment of the service provider"^^xsd:string ;
        dcterms:identifier   "attr-reputation-sustainability"^^xsd:string ;
        dcterms:modified     "2014-07-18T16:34:01+03:00"^^xsd:dateTime ;
        dcterms:title        "Sustainability"^^xsd:string ;
        skos:broader         attr:attr-reputation .

attr:attr-usability-accessibility
        a                    usdl-pref:ServiceAttribute ;
        dcterms:created      "2014-07-18T15:59:26+03:00"^^xsd:dateTime ;
        dcterms:description  "The degree to which a service is operable by users with disabilities"^^xsd:string ;
        dcterms:identifier   "attr-usability-accessibility"^^xsd:string ;
        dcterms:modified     "2014-07-18T15:59:26+03:00"^^xsd:dateTime ;
        dcterms:title        "Accessibility"^^xsd:string ;
        skos:broader         attr:attr-usability .

s:description  a                owl:DatatypeProperty ;
        owl:equivalentProperty  gr:description .

usdl-testing:withScale
        a                 rdf:Property ;
        rdfs:comment      "<p>Connects TestingMethod to TestingScale classification dimension.</p>"@en ;
        rdfs:domain       usdl-testing:TestingMethod ;
        rdfs:isDefinedBy  <http://www.linked-usdl.org/ns/usdl-core/cloud-broker/testing> ;
        rdfs:label        "with scale"@en ;
        rdfs:range        usdl-testing:TestingScale .

usdl-pref:ICCS  a      foaf:Organization ;
        foaf:homepage  <http://www.iccs.gr/eng/> ;
        foaf:member    usdl-pref:yverginadis , usdl-pref:jverginadis ;
        foaf:name      "ICCS" .

attr:attr-agility  a         usdl-pref:ServiceAttribute ;
        dcterms:created      "2014-05-23T21:20:44+03:00"^^xsd:dateTime ;
        dcterms:description  "Indicates the impact of a service upon a client's ability to change direction, strategy, or tactics quickly and with minimal disruption"^^xsd:string ;
        dcterms:identifier   "attr-agility"^^xsd:string ;
        dcterms:modified     "2014-07-18T11:11:30+03:00"^^xsd:dateTime ;
        dcterms:title        "Agility"^^xsd:string ;
        skos:broader         attr:attr-root .

gr:DirectDebit  a         gr:PaymentMethod ;
        rdfs:comment      "Payment by direct debit, i.e., the buying party will inform the offering gr:BusinessEntity about its bank account details and authorizes the gr:BusinessEntity to collect the agreed amount directly from that account."@en ;
        rdfs:isDefinedBy  <http://purl.org/goodrelations/v1> ;
        rdfs:label        "Direct debit (payment method)"@en .

<http://www.linked-usdl.org/ns/human-to-machine>
        a                usdl-core:InteractionType ;
        rdfs:label       "Human to Machine"@en ;
        skos:altLabel    "Human to Machine Interaction"@en ;
        skos:broader     <http://www.linked-usdl.org/ns/semi-automated> ;
        skos:definition  "<p>The interaction between the two parties is semi-automated. It is triggered by a human and processed automatically.</p>"@en ;
        skos:inScheme    <http://www.linked-usdl.org/ns/usdl-interaction-types> ;
        skos:prefLabel   "Human to Machine"@en .

usdl-core:includes  a       rdf:Property ;
        rdfs:comment        "<p>The includes property enables to add various services to a ServiceOffering. While a service offering does not enable to capture composite services, it allows creating bundles of services traded as one entity.</p>"@en ;
        rdfs:domain         usdl-core:ServiceOffering ;
        rdfs:isDefinedBy    <http://www.linked-usdl.org/ns/usdl-core> ;
        rdfs:label          "includes"@en ;
        rdfs:range          usdl-core:Service ;
        rdfs:subPropertyOf  gr:includes .

gr:hasNext  a             owl:ObjectProperty ;
        rdfs:comment      "This ordering relation for gr:DayOfWeek indicates that the subject is directly followed by the object.\n\nExample: Monday hasNext Tuesday\n\nSince days of the week are a cycle, this property is not transitive."@en ;
        rdfs:domain       gr:DayOfWeek ;
        rdfs:isDefinedBy  <http://purl.org/goodrelations/v1> ;
        rdfs:label        "has next (0..1)"@en ;
        rdfs:range        gr:DayOfWeek ;
        owl:inverseOf     gr:hasPrevious .

usdl-pref:hasClassificationCategory
        a                 rdf:Property ;
        rdfs:comment      "<p>This property is used in order to associate the Consumer Preference profile with at least one service dimension. </p>\r\n" ;
        rdfs:domain       usdl-pref:ConsumerPreferenceProfile ;
        rdfs:isDefinedBy  <http://www.linked-usdl.org/ns/usdl-pref> ;
        rdfs:label        "has classification category" ;
        rdfs:range        usdl-sla-cb:ClassificationDimension .

gr:TypeAndQuantityNode
        a                 owl:Class ;
        rdfs:comment      "This class collates all the information about a gr:ProductOrService included in a bundle. If a gr:Offering contains just one item, you can directly link from the gr:Offering to the gr:ProductOrService using gr:includes. If the offering contains multiple items, use an instance of this class for each component to indicate the quantity, unit of measurement, and type of product, and link from the gr:Offering via gr:includesObject.\n\nExample: An offering may include of 100g of Butter and 1 kg of potatoes, or 1 cell phone and 2 headsets."@en ;
        rdfs:isDefinedBy  <http://purl.org/goodrelations/v1> ;
        rdfs:label        "Type and quantity node"@en ;
        owl:disjointWith  gr:DayOfWeek , gr:Location , gr:WarrantyScope , gr:ProductOrService , gr:Brand , gr:QuantitativeValue , gr:BusinessFunction , gr:PaymentMethod , gr:QualitativeValue , gr:DeliveryMethod , gr:WarrantyPromise , gr:BusinessEntityType , gr:PriceSpecification , gr:OpeningHoursSpecification , gr:Offering , gr:BusinessEntity .

gr:durationOfWarrantyInMonths
        a                 owl:DatatypeProperty ;
        rdfs:comment      "This property specifies the duration of the gr:WarrantyPromise in months."@en ;
        rdfs:domain       gr:WarrantyPromise ;
        rdfs:isDefinedBy  <http://purl.org/goodrelations/v1> ;
        rdfs:label        "duration of warranty in months (0..1)"@en ;
        rdfs:range        xsd:int .

gr:hasMinValueInteger
        a                   owl:DatatypeProperty ;
        rdfs:comment        "This property captures the lower limit of a gr:QuantitativeValueInteger instance."@en ;
        rdfs:domain         gr:QuantitativeValueInteger ;
        rdfs:isDefinedBy    <http://purl.org/goodrelations/v1> ;
        rdfs:label          "has min value integer (1..1)"@en ;
        rdfs:range          xsd:int ;
        rdfs:subPropertyOf  gr:hasMinValue .

usdl-core:hasEntityInvolvement
        a                 rdf:Property ;
        rdfs:comment      "<p>Captures the involvements of BusinessEntities within a given Service. By means of EntityInvolvement we can capture who is the service provider, what other entities are involved, etc.</p>"@en ;
        rdfs:domain       usdl-core:Service ;
        rdfs:isDefinedBy  <http://www.linked-usdl.org/ns/usdl-core> ;
        rdfs:label        "has entity involvement"@en ;
        rdfs:range        usdl-core:EntityInvolvement .

usdl-pref:Weight  a       owl:Class , rdfs:Class ;
        rdfs:comment      "<p> It is used to weight a consumer preference.</p> " ;
        rdfs:isDefinedBy  <http://www.linked-usdl.org/ns/usdl-pref> ;
        rdfs:label        "Weight" ;
        rdfs:subClassOf   gr:QuantitativeValueFloat .

gr:Maintain  a            gr:BusinessFunction ;
        rdfs:comment      "This gr:BusinessFunction indicates that the gr:BusinessEntity offers (or seeks) typical maintenance tasks for the specified gr:ProductOrService. Maintenance tasks are actions that undo or compensate for wear or other deterioriation caused by regular usage, in order to restore the originally intended function of the product, or to prevent outage or malfunction."@en ;
        rdfs:isDefinedBy  <http://purl.org/goodrelations/v1> ;
        rdfs:label        "Maintain (business function)"@en .

gr:includes  a            owl:ObjectProperty ;
        rdfs:comment      "This object property is a shortcut for the original gr:includesObject property for the common case of having exactly one single gr:ProductOrService instance included in an Offering. \n\nWhen linking to an instance of gr:SomeItems or gr:Individual, it is equivalent to using a gr:TypeAndQuantityNode with gr:hasUnitOfMeasurement=\"C62\"^^xsd:string and gr:amountOfThisGood=\"1.0\"^^xsd:float for that good.\n\nWhen linking to a gr:ProductOrServiceModel, it is equivalent to \n1. defining an blank node for a gr:SomeItems\n2. linking that blank node via gr:hasMakeAndModel to the gr:ProductOrServiceModel, and\n3. linking from the gr:Offering to that blank node using another blank node of type gr:TypeAndQuantityNode with gr:hasUnitOfMeasurement=\"C62\"^^xsd:string and gr:amountOfThisGood=\"1.0\"^^xsd:float for that good."@en ;
        rdfs:domain       gr:Offering ;
        rdfs:isDefinedBy  <http://purl.org/goodrelations/v1> ;
        rdfs:label        "includes (0..1)"@en ;
        rdfs:range        gr:ProductOrService .

usdl-core:receives  a     rdf:Property ;
        rdfs:comment      "<p>Input required for the InteractionPoint.</p>"@en ;
        rdfs:domain       usdl-core:InteractionPoint ;
        rdfs:isDefinedBy  <http://www.linked-usdl.org/ns/usdl-core> ;
        rdfs:label        "receives"@en ;
        rdfs:range        rdfs:Class .

gr:hasMinValueFloat  a      owl:DatatypeProperty ;
        rdfs:comment        "This property captures the lower limit of a gr:QuantitativeValueFloat instance."@en ;
        rdfs:domain         gr:QuantitativeValueFloat ;
        rdfs:isDefinedBy    <http://purl.org/goodrelations/v1> ;
        rdfs:label          "has min value float (1..1)"@en ;
        rdfs:range          xsd:float ;
        rdfs:subPropertyOf  gr:hasMinValue .

attr:attr-security-access-control-privilege-management-rbac
        a                    usdl-pref:ServiceAttribute ;
        dcterms:created      "2014-07-18T12:51:44Z"^^xsd:dateTime ;
        dcterms:creator      ""^^xsd:string ;
        dcterms:description  ""^^xsd:string ;
        dcterms:identifier   "attr-security-access-control-privilege-management-rbac"^^xsd:string ;
        dcterms:modified     "2014-07-18T12:51:44Z"^^xsd:dateTime ;
        dcterms:title        "Role based Access Control (RBAC)"^^xsd:string ;
        skos:broader         attr:attr-security-access-control-privilege-management .

usdl-testing:DefectTesting
        a                  usdl-testing:TestingGoal ;
        rdfs:label         "Defect Testing"@en ;
        skos:altLabel      "Defect Testing"@en ;
        skos:definition    "<p>A testing method is a defect testing method.</p>"@en ;
        skos:inScheme      usdl-testing:TestingGoalClassificationScheme ;
        skos:prefLabel     "Defect Testing"@en ;
        skos:topConceptOf  usdl-testing:TestingGoalClassificationScheme .

usdl-sla-cb:hasMaxMembershipValue
        a                   rdf:Property ;
        rdfs:comment        "<p>Indicates a max membership value.</p>"@en ;
        rdfs:domain         usdl-sla-cb:FuzzyValue ;
        rdfs:isDefinedBy    usdl-core-cb: ;
        rdfs:label          "has max membership value"@en ;
        rdfs:range          xsd:float ;
        rdfs:subPropertyOf  gr:hasValueFloat .

gr:name  a                owl:DatatypeProperty ;
        rdfs:comment      "A short text describing the respective resource.\n\nThis property is semantically equivalent to dcterms:title and rdfs:label and just meant as a handy shortcut for marking up data."@en ;
        rdfs:domain       [ a            owl:Class ;
                            owl:unionOf  ( owl:Thing gr:Brand gr:BusinessEntity gr:BusinessEntityType gr:BusinessFunction gr:DayOfWeek gr:DeliveryChargeSpecification gr:DeliveryMethod gr:DeliveryModeParcelService gr:Individual gr:Location gr:Offering gr:OpeningHoursSpecification gr:PaymentChargeSpecification gr:PaymentMethod gr:PaymentMethodCreditCard gr:PriceSpecification gr:ProductOrService gr:ProductOrServiceModel gr:QualitativeValue gr:QuantitativeValue gr:QuantitativeValueFloat gr:QuantitativeValueInteger gr:SomeItems gr:TypeAndQuantityNode gr:UnitPriceSpecification gr:WarrantyPromise gr:WarrantyScope )
                          ] ;
        rdfs:isDefinedBy  <http://purl.org/goodrelations/v1> ;
        rdfs:label        "name (0..1)"@en ;
        rdfs:range        rdfs:Literal .

<http://www.linked-usdl.org/ns/producer>
        a                  usdl-core:BusinessRole ;
        rdfs:label         "Producer"@en ;
        skos:definition    "<p>A Producer is the entity that actually deliver a given Service. This may often be the Provider, i.e., the entity responsible, but it may in other cases be a subcontracted entity or a named individual. Tracking this allows for example to know who the actual contact point is, or who may be legally liable for a certain error.</p>"@en ;
        skos:inScheme      <http://www.linked-usdl.org/ns/usdl-business-roles> ;
        skos:prefLabel     "Producer"@en ;
        skos:topConceptOf  <http://www.linked-usdl.org/ns/usdl-business-roles> .

gr:hasUnitOfMeasurement
        a                 owl:DatatypeProperty ;
        rdfs:comment      "The unit of measurement for a gr:QuantitativeValue, a gr:UnitPriceSpecification, or a gr:TypeAndQuantityNode given using the UN/CEFACT Common Code (3 characters)."@en ;
        rdfs:domain       [ a            owl:Class ;
                            owl:unionOf  ( gr:QuantitativeValue gr:TypeAndQuantityNode gr:UnitPriceSpecification )
                          ] ;
        rdfs:isDefinedBy  <http://purl.org/goodrelations/v1> ;
        rdfs:label        "has unit of measurement (1..1)"@en ;
        rdfs:range        xsd:string .

<http://www.linked-usdl.org/ns/mediator>
        a                usdl-core:InteractionRole ;
        rdfs:label       "Mediator"@en ;
        skos:broader     <http://www.linked-usdl.org/ns/participant> ;
        skos:definition  "<p>A Mediator is an entity that is involved within a given interaction but is neither the initiator nor the final destination of a given interaction. An interaction reaching a Mediator is not considered to be concluded.</p>"@en ;
        skos:inScheme    <http://www.linked-usdl.org/ns/usdl-interaction-roles> ;
        skos:prefLabel   "Mediator"@en .

usdl-core:ServiceOffering
        a                 owl:Class , rdfs:Class ;
        rdfs:comment      "<p>A ServiceOffering is an offering made by a gr:BusinessEntity of one or more services to customers. An offering usually associates a price, legal terms of use and conditions included in service level agreements with a service. In other words, it makes a service a tradable entity.</p>"@en ;
        rdfs:isDefinedBy  <http://www.linked-usdl.org/ns/usdl-core> ;
        rdfs:label        "Service Offering"@en ;
        rdfs:subClassOf   gr:Offering .

usdl-pref:QualitativeVariable
        a                 owl:Class , rdfs:Class ;
        rdfs:comment      "<p> A QualitativeVariable is used to reference a qualitative value.</p> " ;
        rdfs:isDefinedBy  <http://www.linked-usdl.org/ns/usdl-pref> ;
        rdfs:label        "Qualitative Variable" ;
        rdfs:subClassOf   usdl-pref:PreferenceVariable .

usdl-core:Role  a         owl:Class , rdfs:Class ;
        rdfs:comment      "<p>The Roles that an entity may play. One may define as many Roles as necessary by defining subclasses of Role or by creating SKOS concept schemes. For completeness Linked USDL Core provides both a basic structuring in kinds of Roles to be contemplated (e.g., BusinessRoles, InteractionRoles) as well as a basic concept scheme for these roles that can be used out of the box or as reference for specific extensions. See Linked USDL Business Roles and Interaction Roles Modules.</p>"@en ;
        rdfs:isDefinedBy  <http://www.linked-usdl.org/ns/usdl-core> ;
        rdfs:label        "Role"@en ;
        rdfs:subClassOf   skos:Concept .

gr:PaymentMethodCreditCard
        a                 owl:Class ;
        rdfs:comment      "The subclass of gr:PaymentMethod represents all variants and brands of credit or debit cards as a standardized procedure for transferring the monetary amount for a purchase. It is mostly used for specifying the types of payment accepted by a gr:Business Entity.\n\nExamples: VISA, MasterCard, or American Express."@en ;
        rdfs:isDefinedBy  <http://purl.org/goodrelations/v1> ;
        rdfs:label        "Payment method credit card"@en ;
        rdfs:subClassOf   gr:PaymentMethod .

usdl-pref:ConsumerPreference
        a                 owl:Class , rdfs:Class ;
        rdfs:comment      "<p>A ConsumerPreference specifies a preference on a specific topic. For this purpose it may reference a ConsumerPreferenceExpression.</p> " ;
        rdfs:isDefinedBy  <http://www.linked-usdl.org/ns/usdl-pref> ;
        rdfs:label        "Consumer Preference" .

usdl-core:hasInteractionType
        a                 rdf:Property ;
        rdfs:comment      "<p>The hasInteractionType relationship captures the modes of interaction for a given InteractionPoint through a particular ContactMedium.</p>"@en ;
        rdfs:domain       usdl-core:CommunicationChannel ;
        rdfs:isDefinedBy  <http://www.linked-usdl.org/ns/usdl-core> ;
        rdfs:label        "has interaction type"@en ;
        rdfs:range        usdl-core:InteractionType .

attr:attr-performance-capacity-num-of-cores
        a                    usdl-pref:ServiceAttribute ;
        dcterms:created      "2014-07-18T11:42:21Z"^^xsd:dateTime ;
        dcterms:creator      ""^^xsd:string ;
        dcterms:description  ""^^xsd:string ;
        dcterms:identifier   "attr-performance-capacity-num-of-cores"^^xsd:string ;
        dcterms:modified     "2014-07-18T11:42:21Z"^^xsd:dateTime ;
        dcterms:title        "Number of Cores"^^xsd:string ;
        skos:broader         attr:attr-performance-capacity .

attr:attr-agility-flexibility
        a                    usdl-pref:ServiceAttribute ;
        dcterms:created      "2014-07-18T08:16:15Z"^^xsd:dateTime ;
        dcterms:creator      ""^^xsd:string ;
        dcterms:description  "The ability to add or remove predefined features from a service"^^xsd:string ;
        dcterms:identifier   "attr-agility-flexibility"^^xsd:string ;
        dcterms:modified     "2014-07-18T08:16:15Z"^^xsd:dateTime ;
        dcterms:title        "Flexibility"^^xsd:string ;
        skos:broader         attr:attr-agility .

usdl-sla-cb:hasDefaultQuantitativeProperty
        a                   rdf:Property ;
        rdfs:comment        "<p>The default quantitative value of the variable. Subproperties of this property can be used to refer also to fuzzy values since FuzzyValue is specified as a subclass of gr:QuantitativeValueFloat.</p>" ;
        rdfs:isDefinedBy    <http://linked-usdl.org/ns/usdl-sla/cloud-broker> ;
        rdfs:label          "has default quantitative property" ;
        rdfs:subPropertyOf  usdl-sla:hasDefault .

usdl-sla-cb:afriesen  a  foaf:Person ;
        foaf:name  "Andreas Friesen" .

usdl-testing:ManualTesting
        a                  usdl-testing:TestGenerationStrategy ;
        rdfs:label         "Manual Testing"@en ;
        skos:altLabel      "Manual Testing"@en ;
        skos:definition    "<p>A testing method is a manual testing method.</p>"@en ;
        skos:inScheme      usdl-testing:TestGenerationStrategyClassificationScheme ;
        skos:prefLabel     "Manual Testing"@en ;
        skos:topConceptOf  usdl-testing:TestGenerationStrategyClassificationScheme .

gr:Location  a               owl:Class ;
        rdfs:comment         "A location is a point or area of interest from which a particular product or service is available, e.g. a store, a bus stop, a gas station, or a ticket booth. The difference to gr:BusinessEntity is that the gr:BusinessEntity is the legal entity (e.g. a person or corporation) making the offer, while gr:Location is the store, office, or place. A chain restaurant will e.g. have one legal entity but multiple restaurant locations. Locations are characterized by an address or geographical position and a set of opening hour specifications for various days of the week.\n\t\t\nExample: A rental car company may offer the Business Function Lease Out of cars from two locations, one in Fort Myers, Florida, and one in Boston, Massachussetts. Both stations are open 7:00 - 23:00 Mondays through Saturdays.\n\nNote: Typical address standards (vcard) and location data (geo, WGC84) should be attached to a gr:Location node. Since there already exist established vocabularies for this, the GoodRelations ontology does not provide respective attributes. Instead, the use of respective vocabularies is recommended. However, the gr:hasGlobalLocationNumber property is  provided for linking to public identifiers for business locations.\n\t\t\nCompatibility with schema.org: This class is equivalent to http://schema.org/Place."@en ;
        rdfs:isDefinedBy     <http://purl.org/goodrelations/v1> ;
        rdfs:label           "Location"@en ;
        owl:disjointWith     gr:Brand , gr:BusinessFunction , gr:PriceSpecification , gr:TypeAndQuantityNode , gr:WarrantyPromise , gr:Offering , gr:BusinessEntity , gr:WarrantyScope , gr:OpeningHoursSpecification , gr:DayOfWeek , gr:PaymentMethod , gr:QuantitativeValue , gr:DeliveryMethod , gr:BusinessEntityType ;
        owl:equivalentClass  gr:LocationOfSalesOrServiceProvisioning .

gr:PayPal  a              gr:PaymentMethod ;
        rdfs:comment      "Payment via the PayPal payment service."@en ;
        rdfs:isDefinedBy  <http://purl.org/goodrelations/v1> ;
        rdfs:label        "PayPal (payment method)"@en .

usdl-testing:AcceptanceTesting
        a                  usdl-testing:TestingFocus ;
        rdfs:label         "Acceptance Testing"@en ;
        skos:altLabel      "Acceptance Testing"@en ;
        skos:definition    "<p>A testing method is an acceptance testing method.</p>"@en ;
        skos:inScheme      usdl-testing:TestingFocusClassificationScheme ;
        skos:prefLabel     "Acceptance Testing"@en ;
        skos:topConceptOf  usdl-testing:TestingFocusClassificationScheme .

attr:attr-performance-functionality
        a                    usdl-pref:ServiceAttribute ;
        dcterms:created      "2014-07-18T12:02:07Z"^^xsd:dateTime ;
        dcterms:creator      ""^^xsd:string ;
        dcterms:description  "The specific features provided by a service"^^xsd:string ;
        dcterms:identifier   "attr-performance-functionality"^^xsd:string ;
        dcterms:modified     "2014-07-18T12:02:07Z"^^xsd:dateTime ;
        dcterms:title        "Functionality"^^xsd:string ;
        skos:broader         attr:attr-performance .

attr:attr-security-data-geographic-political
        a                    usdl-pref:ServiceAttribute ;
        dcterms:created      "2014-07-18T12:52:25Z"^^xsd:dateTime ;
        dcterms:creator      ""^^xsd:string ;
        dcterms:description  "The client's constraints on service location based on geography or politics"^^xsd:string ;
        dcterms:identifier   "attr-security-data-geographic-political"^^xsd:string ;
        dcterms:modified     "2014-07-18T12:52:25Z"^^xsd:dateTime ;
        dcterms:title        "Data Geographic/Political"^^xsd:string ;
        skos:broader         attr:attr-security .

gr:availableAtOrFrom  a   owl:ObjectProperty ;
        rdfs:comment      "This states that a particular gr:Offering is available at or from the given gr:Location (e.g. shop or branch)."@en ;
        rdfs:domain       [ a            owl:Class ;
                            owl:unionOf  ( gr:Offering s:Offer )
                          ] ;
        rdfs:isDefinedBy  <http://purl.org/goodrelations/v1> ;
        rdfs:label        "available at or from (0..*)"@en ;
        rdfs:range        gr:Location .

attr:attr-performance
        a                    usdl-pref:ServiceAttribute ;
        dcterms:created      "2014-05-23T21:20:08+03:00"^^xsd:dateTime ;
        dcterms:description  "It covers the features and functions of the provided services"^^xsd:string ;
        dcterms:identifier   "attr-performance"^^xsd:string ;
        dcterms:modified     "2014-07-18T14:41:37+03:00"^^xsd:dateTime ;
        dcterms:title        "Performance"^^xsd:string ;
        skos:broader         attr:attr-root .

gr:VISA  a                gr:PaymentMethodCreditCard ;
        rdfs:comment      "Payment by credit or debit cards issued by the VISA network."@en ;
        rdfs:isDefinedBy  <http://purl.org/goodrelations/v1> ;
        rdfs:label        "VISA (payment method)"@en .

attr:attr-performance-capacity-storage-redundancy
        a                    usdl-pref:ServiceAttribute ;
        dcterms:created      "2014-07-18T11:58:39Z"^^xsd:dateTime ;
        dcterms:creator      ""^^xsd:string ;
        dcterms:description  ""^^xsd:string ;
        dcterms:identifier   "attr-performance-capacity-storage-redundancy"^^xsd:string ;
        dcterms:modified     "2014-07-18T11:58:39Z"^^xsd:dateTime ;
        dcterms:title        "Storage Redundancy"^^xsd:string ;
        skos:broader         attr:attr-performance-capacity .

gr:ProductOrServiceModel
        a                 owl:Class ;
        rdfs:comment      "A product or service model is a intangible entity that specifies some characteristics of a group of similar, usually mass-produced products, in the sense of a prototype. In case of mass-produced products, there exists a relation gr:hasMakeAndModel between the actual product or service (gr:Individual or gr:SomeItems) and the prototype (gr:ProductOrServiceModel). GoodRelations treats product or service models as \"prototypes\" instead of a completely separate kind of entities, because this allows using the same domain-specific properties (e.g. gr:weight) for describing makes and models and for describing actual products.\n\nExamples: Ford T, Volkswagen Golf, Sony Ericsson W123 cell phone\n\nNote: An actual product or service (gr:Individual) by default shares the features of its model (e.g. the weight). However, this requires non-standard reasoning. See http://wiki.goodrelations-vocabulary.org/Axioms for respective rule sets.\n\t\nCompatibility with schema.org: This class is (approximately) a subclass of http://schema.org/Product."@en ;
        rdfs:isDefinedBy  <http://purl.org/goodrelations/v1> ;
        rdfs:label        "Product or service model"@en ;
        rdfs:subClassOf   s:Product , gr:ProductOrService ;
        owl:disjointWith  gr:SomeItems , gr:Brand , gr:BusinessEntity , gr:Individual .

attr:null  a                 usdl-pref:ServiceAttribute ;
        dcterms:created      "1900-01-01T00:00:00+00:00"^^xsd:dateTime ;
        dcterms:creator      ""^^xsd:string ;
        dcterms:description  ""^^xsd:string ;
        dcterms:identifier   "null"^^xsd:string ;
        dcterms:modified     "1900-01-01T00:00:00+00:00"^^xsd:dateTime ;
        dcterms:title        "NO_ATTRIBUTE"^^xsd:string .

usdl-sla-cb:hasDefaultDatatypeProperty
        a                 rdf:Property ;
        rdfs:comment      "<p>The default simple datatype value of the variable.</p>\r\n" ;
        rdfs:domain       usdl-sla:Variable ;
        rdfs:isDefinedBy  <http://linked-usdl.org/ns/usdl-sla/cloud-broker> ;
        rdfs:label        "has default datatype property" ;
        rdfs:range        rdfs:Datatype .

gr:QualitativeValue  a    owl:Class ;
        rdfs:comment      "A qualitative value is a predefined value for a product characteristic. \n\t\nExamples: the color \"green\" or the power cord plug type \"US\"; the garment sizes \"S\", \"M\", \"L\", and \"XL\".\n\t\nNote: Value sets are supported by creating subclasses of this class. Ordinal relations between values (gr:greater, gr:lesser, ...) are provided directly by GoodRelations.\n\nCompatibility with schema.org: This class is equivalent to http://schema.org/Enumeration."@en ;
        rdfs:isDefinedBy  <http://purl.org/goodrelations/v1> ;
        rdfs:label        "Qualitative value"@en ;
        owl:disjointWith  gr:TypeAndQuantityNode , gr:QuantitativeValue , gr:Offering .

attr:attr-performance-monitoring-level
        a                    usdl-pref:ServiceAttribute ;
        dcterms:created      "2014-07-18T12:06:03Z"^^xsd:dateTime ;
        dcterms:creator      ""^^xsd:string ;
        dcterms:description  ""^^xsd:string ;
        dcterms:identifier   "attr-performance-monitoring-level"^^xsd:string ;
        dcterms:modified     "2014-07-18T12:06:03Z"^^xsd:dateTime ;
        dcterms:title        "Monitoring Level"^^xsd:string ;
        skos:broader         attr:attr-performance-monitoring .

gr:Individual  a             owl:Class ;
        rdfs:comment         "A gr:Individual is an actual product or service instance, i.e., a single identifiable object or action that creates some increase in utility (in the economic sense) for the individual possessing or using this very object (product) or for the individual in whose favor this very action is being taken (service). Products or services are types of goods in the economic sense. For an overview of goods and commodities in economics, see Milgate (1987).\n\nExamples: MyThinkpad T60, the pint of beer standing in front of me, my Volkswagen Golf, the haircut that I received or will be receiving at a given date and time.\n\nNote 1: In many cases, product or service instances are not explicitly exposed on the Web but only claimed to exist (i.e. existentially quantified). In this case, use gr:SomeItems.\nNote 2: This class is the new, shorter form of the former gr:ActualProductOrServiceInstance.\n\nCompatibility with schema.org: This class is a subclass of http://schema.org/Product."@en ;
        rdfs:isDefinedBy     <http://purl.org/goodrelations/v1> ;
        rdfs:label           "Individual"@en ;
        rdfs:subClassOf      s:Product , gr:ProductOrService ;
        owl:disjointWith     gr:SomeItems , gr:ProductOrServiceModel ;
        owl:equivalentClass  gr:ActualProductOrServiceInstance .

<http://www.linked-usdl.org/ns/usdl-pref>
        a                              owl:Ontology ;
        dc:creator                     usdl-pref:jverginadis , usdl-pref:afriesen , usdl-pref:ipatiniotakis ;
        dc:description                 "<p>Simple vocabulary for describing consumer preference. This vocabulary is based on the work on Linked USDL in the Broker@Cloud project.</p>\r\n<p>Preferences module of Linked USDL. Consumer preferences are a common way to formally specify consumer preferences on services offered on a cloud service brokerage platform.</p>\r\n" ;
        dc:modified                    "2014-09-08"^^xsd:date ;
        dc:title                       "USDL Preferences" ;
        vann:preferredNamespacePrefix  "usdl-pref" ;
        vann:preferredNamespaceUri     "http://www.linked-usdl.org/ns/usdl-pref#" ;
        foaf:page                      <http://www.linked-usdl.org/ns/usdl-pref.html> .

gr:ProductOrService  a    owl:Class ;
        rdfs:comment      "The superclass of all classes describing products or services types, either by nature or purpose. Examples for such subclasses are \"TV set\", \"vacuum cleaner\", etc. An instance of this class can be either an actual product or service (gr:Individual), a placeholder instance for unknown instances of a mass-produced commodity (gr:SomeItems), or a model / prototype specification (gr:ProductOrServiceModel). When in doubt, use gr:SomeItems.\n\nExamples: \na) MyCellphone123, i.e. my personal, tangible cell phone (gr:Individual)\nb) Siemens1234, i.e. the Siemens cell phone make and model 1234 (gr:ProductOrServiceModel)\nc) dummyCellPhone123 as a placeholder for actual instances of a certain kind of cell phones (gr:SomeItems)\n\t\nNote: Your first choice for specializations of gr:ProductOrService should be http://www.productontology.org.\n\nCompatibility with schema.org: This class is (approximately) equivalent to http://schema.org/Product."@en ;
        rdfs:isDefinedBy  <http://purl.org/goodrelations/v1> ;
        rdfs:label        "Product or service"@en ;
        owl:disjointWith  gr:Brand , gr:QuantitativeValue , gr:WarrantyPromise , gr:DeliveryMethod , gr:OpeningHoursSpecification , gr:Offering , gr:TypeAndQuantityNode , gr:DayOfWeek , gr:WarrantyScope , gr:PriceSpecification , gr:BusinessFunction , gr:BusinessEntityType .

usdl-pref:afriesen  a  foaf:Person ;
        foaf:name  "Andreas Friesen" .

attr:attr-usability-understandability
        a                    usdl-pref:ServiceAttribute ;
        dcterms:created      "2014-07-18T16:25:06+03:00"^^xsd:dateTime ;
        dcterms:description  "The ease with which users can understand the capabilities and operation of the service"^^xsd:string ;
        dcterms:identifier   "attr-usability-understandability"^^xsd:string ;
        dcterms:modified     "2014-07-18T16:25:06+03:00"^^xsd:dateTime ;
        dcterms:title        "Understandability"^^xsd:string ;
        skos:broader         attr:attr-usability .

gr:Repair  a              gr:BusinessFunction ;
        rdfs:comment      "This gr:BusinessFunction indicates that the gr:BusinessEntity offers (or seeks) the evaluation of the chances for repairing, and, if positive, repair of the specified gr:ProductOrService. Repairing means actions that restore the originally intended function of a product that suffers from outage or malfunction."@en ;
        rdfs:isDefinedBy  <http://purl.org/goodrelations/v1> ;
        rdfs:label        "Repair (business function)"@en .

usdl-core:EntityInteraction
        a                 owl:Class , rdfs:Class ;
        rdfs:comment      "<p>EntityInteraction helps captures a ternary relationship between InteractionPoints the types of BusinessEntities involved (based on their role e.g., provider or consumer) and the actual InteractionRole (e.g., initiator or receiver) of that BusinessEntity within a particular InteractionPoint. This enables specifying for instance the fact that an insurance claim should be initiated by the consumer through an interaction with the insurance provider.</p>"@en ;
        rdfs:isDefinedBy  <http://www.linked-usdl.org/ns/usdl-core> ;
        rdfs:label        "Entity Interaction"@en .

gr:WarrantyPromise  a     owl:Class ;
        rdfs:comment      "This is a conceptual entity that holds together all aspects of the n-ary relation gr:hasWarrantyPromise.\n\nA Warranty promise is an entity representing the duration and scope of services that will be provided to a customer free of charge in case of a defect or malfunction of the gr:ProductOrService. A warranty promise is characterized by its temporal duration (usually starting with the date of purchase) and its gr:WarrantyScope. The warranty scope represents the types of services provided (e.g. labor and parts, just parts) of the warranty included in an gr:Offering. The actual services may be provided by the gr:BusinessEntity making the offering, by the manufacturer of the product, or by a third party. There may be multiple warranty promises associated with a particular offering, which differ in duration and scope (e.g. pick-up service during the first 12 months, just parts and labor for 36 months).\n\nExamples: 12 months parts and labor, 36 months parts"@en ;
        rdfs:isDefinedBy  <http://purl.org/goodrelations/v1> ;
        rdfs:label        "Warranty promise"@en ;
        owl:disjointWith  gr:Brand , gr:Location , gr:BusinessFunction , gr:TypeAndQuantityNode , gr:BusinessEntityType , gr:ProductOrService , gr:OpeningHoursSpecification , gr:WarrantyScope , gr:QuantitativeValue , gr:Offering , gr:PriceSpecification , gr:PaymentMethod , gr:DeliveryMethod , gr:DayOfWeek , gr:BusinessEntity .

attr:attr-security-data-privacy-loss
        a                    usdl-pref:ServiceAttribute ;
        dcterms:created      "2014-07-18T12:53:42Z"^^xsd:dateTime ;
        dcterms:creator      ""^^xsd:string ;
        dcterms:description  "Client restrictions on access and use of client data are enforced by the service provider. Any failures of these protections are promptly detected and reported to the client"^^xsd:string ;
        dcterms:identifier   "attr-security-data-privacy-loss"^^xsd:string ;
        dcterms:modified     "2014-07-18T12:53:42Z"^^xsd:dateTime ;
        dcterms:title        "Data Privacy & Data Loss"^^xsd:string ;
        skos:broader         attr:attr-security .

attr:attr-security-proactive-threat-vulnerability-management
        a                    usdl-pref:ServiceAttribute ;
        dcterms:created      "2014-07-18T12:55:12Z"^^xsd:dateTime ;
        dcterms:creator      ""^^xsd:string ;
        dcterms:description  "Mechanisms in place to ensure that the service is protected against known recurring threats as well as new evolving vulnerabilities"^^xsd:string ;
        dcterms:identifier   "attr-security-proactive-threat-vulnerability-management"^^xsd:string ;
        dcterms:modified     "2014-07-18T12:55:12Z"^^xsd:dateTime ;
        dcterms:title        "Proactive Threat & Vulnerability Management"^^xsd:string ;
        skos:broader         attr:attr-security .

<http://www.linked-usdl.org/ns/automated>
        a                  usdl-core:InteractionType ;
        rdfs:label         "Automated"@en ;
        skos:altLabel      "Automated Interaction"@en ;
        skos:definition    "The interaction between the two parties is entirely automated.</p>"@en ;
        skos:inScheme      <http://www.linked-usdl.org/ns/usdl-interaction-types> ;
        skos:prefLabel     "Automated"@en ;
        skos:topConceptOf  <http://www.linked-usdl.org/ns/usdl-interaction-types> .

attr:attr-assurance-recoverability-recovery-time
        a                    usdl-pref:ServiceAttribute ;
        dcterms:created      "2014-07-18T11:53:21+03:00"^^xsd:dateTime ;
        dcterms:description  ""^^xsd:string ;
        dcterms:identifier   "attr-assurance-recoverability-recovery-time"^^xsd:string ;
        dcterms:modified     "2014-07-18T11:53:21+03:00"^^xsd:dateTime ;
        dcterms:title        "Recovery Time"^^xsd:string ;
        skos:broader         attr:attr-assurance-recoverability .

gr:hasStockKeepingUnit
        a                   owl:DatatypeProperty ;
        rdfs:comment        "The Stock Keeping Unit, or SKU is a unique identifier for a product, service, or bundle from the perspective of a particular supplier, i.e. SKUs are mostly assigned and serialized at the merchant level. \nExamples of SKUs are the ordering or parts numbers used by a particular Web shop or catalog.\n\nConsequently, the domain of gr:hasStockKeepingUnit is the union of the classes gr:Offering and gr:ProductOrService. \nIf attached to a gr:Offering, the SKU will usually reflect a merchant-specific identifier, i.e. one valid only for that particular retailer or shop. \nIf attached to a gr:ProductOrServiceModel, the SKU can reflect either the identifier used by the merchant or the part number used by the official manufacturer of that part. For the latter, gr:hasMPN is a better choice.\n\nImportant: Be careful when assuming two products or services instances or offering instances to be identical based on the SKU. Since SKUs are unique only for the same gr:BusinessEntity, this can be assumed only when you are sure that the two SKU values refer to the same business entity. Such can be done by taking into account the provenance of the data. As long as instances of gr:Offering are concerned, you can also check that the offerings are being offered by the same gr:Business Entity.\n\nUsually, the properties gr:hasEAN_UCC-13 and gr:hasGTIN-14 are much more reliable identifiers, because they are globally unique.\n\nSee also http://en.wikipedia.org/wiki/Stock_Keeping_Unit."@en ;
        rdfs:domain         [ a            owl:Class ;
                              owl:unionOf  ( gr:Offering gr:ProductOrService s:Offer s:Product )
                            ] ;
        rdfs:isDefinedBy    <http://purl.org/goodrelations/v1> ;
        rdfs:label          "has Stock Keeping Unit (0..*)"@en ;
        rdfs:range          xsd:string ;
        rdfs:subPropertyOf  s:productID .

gr:hasGTIN-14  a            owl:DatatypeProperty ;
        rdfs:comment        "The Global Trade Item Number (GTIN-14) of the given gr:ProductOrService or gr:Offering."@en ;
        rdfs:domain         [ a            owl:Class ;
                              owl:unionOf  ( gr:Offering gr:ProductOrService s:Product )
                            ] ;
        rdfs:isDefinedBy    <http://purl.org/goodrelations/v1> ;
        rdfs:label          "has GTIN-14 (0..*)"@en ;
        rdfs:range          xsd:string ;
        rdfs:subPropertyOf  s:productID .

usdl-testing:FunctionalTesting
        a                  usdl-testing:TestingFocus ;
        rdfs:label         "Functional Testing"@en ;
        skos:altLabel      "Functional Testing"@en ;
        skos:definition    "<p>A testing method is a functional testing method.</p>"@en ;
        skos:inScheme      usdl-testing:TestingFocusClassificationScheme ;
        skos:prefLabel     "Functional Testing"@en ;
        skos:topConceptOf  usdl-testing:TestingFocusClassificationScheme .

gr:addOn  a               owl:ObjectProperty ;
        rdfs:comment      "This property points from a gr:Offering to additional offerings that can only be obtained in combination with the first offering. This can be used to model supplements and extensions that are available for a surcharge. Any gr:PriceSpecification attached to the secondary offering is to be understood as an additional charge."@en ;
        rdfs:domain       [ a            owl:Class ;
                            owl:unionOf  ( gr:Offering s:Offer )
                          ] ;
        rdfs:isDefinedBy  <http://purl.org/goodrelations/v1> ;
        rdfs:label        "add-on (0..*)"@en ;
        rdfs:range        gr:Offering .

gr:height  a                owl:ObjectProperty ;
        rdfs:comment        "The height of the product.\nTypical unit code(s): CMT for centimeters, INH for inches"@en ;
        rdfs:domain         [ a            owl:Class ;
                              owl:unionOf  ( gr:ProductOrService s:Product )
                            ] ;
        rdfs:isDefinedBy    <http://purl.org/goodrelations/v1> ;
        rdfs:label          "height (0..1)"@en ;
        rdfs:range          gr:QuantitativeValue ;
        rdfs:subPropertyOf  gr:quantitativeProductOrServiceProperty .

gr:Saturday  a              gr:DayOfWeek ;
        rdfs:comment        "Saturday as a day of the week."@en ;
        rdfs:isDefinedBy    <http://purl.org/goodrelations/v1> ;
        rdfs:label          "Saturday (day of week)"@en ;
        gr:displayPosition  6 ;
        gr:hasNext          gr:Sunday ;
        gr:hasPrevious      gr:Friday .

gr:hasMaxValue  a         owl:DatatypeProperty ;
        rdfs:comment      "This property captures the upper limit of a gr:QuantitativeValue instance."@en ;
        rdfs:domain       gr:QuantitativeValue ;
        rdfs:isDefinedBy  <http://purl.org/goodrelations/v1> ;
        rdfs:label        "has max value (0..1)"@en ;
        rdfs:range        rdfs:Literal .

attr:attr-reputation-brand-name
        a                    usdl-pref:ServiceAttribute ;
        dcterms:created      "2014-05-23T21:34:52+03:00"^^xsd:dateTime ;
        dcterms:description  "It is the linguistic expression of the reputation of the cloud service provider as perceived by its consumers"^^xsd:string ;
        dcterms:identifier   "attr-reputation-brand-name"^^xsd:string ;
        dcterms:modified     "2014-07-18T16:26:38+03:00"^^xsd:dateTime ;
        dcterms:title        "Brand Name"^^xsd:string ;
        skos:broader         attr:attr-reputation .

gr:description  a         owl:DatatypeProperty ;
        rdfs:comment      "A short textual description of the resource. \n\nThis property is semantically equivalent to rdfs:comment and just meant as a handy shortcut for marking up data."@en ;
        rdfs:domain       [ a            owl:Class ;
                            owl:unionOf  ( owl:Thing gr:Brand gr:BusinessEntity gr:BusinessEntityType gr:BusinessFunction gr:DayOfWeek gr:DeliveryChargeSpecification gr:DeliveryMethod gr:DeliveryModeParcelService gr:Individual gr:Location gr:Offering gr:OpeningHoursSpecification gr:PaymentChargeSpecification gr:PaymentMethod gr:PaymentMethodCreditCard gr:PriceSpecification gr:ProductOrService gr:ProductOrServiceModel gr:QualitativeValue gr:QuantitativeValue gr:QuantitativeValueFloat gr:QuantitativeValueInteger gr:SomeItems gr:TypeAndQuantityNode gr:UnitPriceSpecification gr:WarrantyPromise gr:WarrantyScope )
                          ] ;
        rdfs:isDefinedBy  <http://purl.org/goodrelations/v1> ;
        rdfs:label        "description (0..1)"@en ;
        rdfs:range        rdfs:Literal .

gr:advanceBookingRequirement
        a                 owl:ObjectProperty ;
        rdfs:comment      "The minimal and maximal amount of time that is required between accepting the gr:Offering and the actual usage of the resource or service. This is mostly relevant for offers regarding hotel rooms, the rental of objects, or the provisioning of services. The duration is specified relatively to the beginning of the usage of the contracted object. It is represented by attaching an instance of the class gr:QuantitativeValueInteger. The lower and upper boundaries are specified using the properties gr:hasMinValueInteger and gr:hasMaxValueInteger to that instance. The unit of measurement is specified using the property gr:hasUnitOfMeasurement with a string holding a UN/CEFACT code suitable for durations, e.g. MON (months), DAY (days), HUR (hours), or MIN (minutes).\n\nThe difference to the gr:validFrom and gr:validThrough properties is that those specify the interval during which the gr:Offering is valid, while gr:advanceBookingRequirement specifies the acceptable relative amount of time between accepting the offer and the fulfilment or usage."@en ;
        rdfs:domain       [ a            owl:Class ;
                            owl:unionOf  ( gr:Offering s:Offer )
                          ] ;
        rdfs:isDefinedBy  <http://purl.org/goodrelations/v1> ;
        rdfs:label        "advance booking requirement (0..1)"@en ;
        rdfs:range        gr:QuantitativeValueInteger .

usdl-testing:ConformanceTestingTesting
        a                  usdl-testing:TestingGoal ;
        rdfs:label         "ConformanceTesting Testing"@en ;
        skos:altLabel      "ConformanceTesting Testing"@en ;
        skos:definition    "<p>A testing method is a conformanceTesting testing method.</p>"@en ;
        skos:inScheme      usdl-testing:TestingGoalClassificationScheme ;
        skos:prefLabel     "ConformanceTesting Testing"@en ;
        skos:topConceptOf  usdl-testing:TestingGoalClassificationScheme .

attr:attr-performance-monitoring-middelware
        a                    usdl-pref:ServiceAttribute ;
        dcterms:created      "2014-07-18T12:06:19Z"^^xsd:dateTime ;
        dcterms:creator      ""^^xsd:string ;
        dcterms:description  ""^^xsd:string ;
        dcterms:identifier   "attr-performance-monitoring-middelware"^^xsd:string ;
        dcterms:modified     "2014-07-18T12:06:19Z"^^xsd:dateTime ;
        dcterms:title        "Monitoring Middelware"^^xsd:string ;
        skos:broader         attr:attr-performance-monitoring .

gr:priceType  a           owl:DatatypeProperty ;
        rdfs:comment      "This attribute can be used to distinguish multiple different price specifications for the same gr:Offering. It supersedes the former gr:isListPrice property. The following values are recommended:\n\nThe absence of this property marks the actual sales price.\n\nSRP: \"suggested retail price\" - applicable for all sorts of a non-binding retail price recommendations, e.g. such published by the manufacturer or the distributor. This value replaces the former gr:isListPrice property.\n\nINVOICE: The invoice price, mostly used in the car industry - this is the price a dealer pays to the manufacturer, excluding rebates and charges."@en ;
        rdfs:domain       gr:UnitPriceSpecification ;
        rdfs:isDefinedBy  <http://purl.org/goodrelations/v1> ;
        rdfs:label        "price type (0..1)"@en ;
        rdfs:range        xsd:string .

attr:attr-reputation-sustainability-societal-impact
        a                    usdl-pref:ServiceAttribute ;
        dcterms:created      "2014-07-18T13:35:01Z"^^xsd:dateTime ;
        dcterms:creator      ""^^xsd:string ;
        dcterms:description  ""^^xsd:string ;
        dcterms:identifier   "attr-reputation-sustainability-societal-impact"^^xsd:string ;
        dcterms:modified     "2014-07-18T13:35:01Z"^^xsd:dateTime ;
        dcterms:title        "Societal impact"^^xsd:string ;
        skos:broader         attr:attr-reputation-sustainability .

attr:attr-performance-monitoring-analytics-framework
        a                    usdl-pref:ServiceAttribute ;
        dcterms:created      "2014-07-18T12:06:31Z"^^xsd:dateTime ;
        dcterms:creator      ""^^xsd:string ;
        dcterms:description  ""^^xsd:string ;
        dcterms:identifier   "attr-performance-monitoring-analytics-framework"^^xsd:string ;
        dcterms:modified     "2014-07-18T12:06:31Z"^^xsd:dateTime ;
        dcterms:title        "Analytics framework"^^xsd:string ;
        skos:broader         attr:attr-performance-monitoring .

attr:attr-reputation-ease-of-doing-business
        a                    usdl-pref:ServiceAttribute ;
        dcterms:created      "2014-07-18T13:32:31Z"^^xsd:dateTime ;
        dcterms:creator      ""^^xsd:string ;
        dcterms:description  "Client satisfaction with the ability to do business with a service provider"^^xsd:string ;
        dcterms:identifier   "attr-reputation-ease-of-doing-business"^^xsd:string ;
        dcterms:modified     "2014-07-18T13:32:31Z"^^xsd:dateTime ;
        dcterms:title        "Ease of doing business"^^xsd:string ;
        skos:broader         attr:attr-reputation .

gr:PublicInstitution  a   gr:BusinessEntityType ;
        rdfs:comment      "The gr:BusinessEntityType representing such agents that are part of the adminstration or owned by the public."@en ;
        rdfs:isDefinedBy  <http://purl.org/goodrelations/v1> ;
        rdfs:label        "Public institution (business entity type)"@en .

usdl-pref:ConsumerPreferenceExpression
        a                 owl:Class , rdfs:Class ;
        rdfs:comment      "<p>A ConsumerPreferenceExpression specifies an expression that is evaluated in the context of a consumer preference. For this purpose it may reference a set of preference variables (quantitative, qualitative or fuzzy variables).</p>\r\n" ;
        rdfs:isDefinedBy  <http://www.linked-usdl.org/ns/usdl-pref> ;
        rdfs:label        "Consumer Preference Expression" .

usdl-core:CommunicationChannel
        a                 owl:Class , rdfs:Class ;
        rdfs:comment      "<p>CommunicationChannel is the class of all different communication channels that business entities could use for communication, e.g., email, phone, etc.</p>"@en ;
        rdfs:isDefinedBy  <http://www.linked-usdl.org/ns/usdl-core> ;
        rdfs:label        "Communication Channel"@en ;
        owl:unionOf       ( msm:Operation vcard:Address vcard:Email vcard:TelephoneType ) .

usdl-testing:TestingGoalClassificationScheme
        a                    skos:ConceptScheme ;
        dcterms:description  "<p>This vocabulary provides the concepts to classify testing goal dimension. </p>"@en ;
        dcterms:title        "Testing Goal classification concept scheme" ;
        skos:hasTopConcept   usdl-testing:StressTesting , usdl-testing:DefectTesting , usdl-testing:RegressionTesting , usdl-testing:ConformanceTesting , usdl-testing:ExploratoryTesting ;
        skos:prefLabel       "Testing Goal Classification"@en .

usdl-testing:TestingMethod
        a                 owl:Class , rdfs:Class ;
        rdfs:comment      "<p>Testing Method allows a multi-dimensional classification of a concrete testing method.</p>"@en ;
        rdfs:isDefinedBy  <http://www.linked-usdl.org/ns/usdl-core/cloud-broker/testing> ;
        rdfs:label        "Testing Method"@en .

<http://www.linked-usdl.org/ns/by-locality>
        a               skos:Collection ;
        skos:member     <http://www.linked-usdl.org/ns/remote> , <http://www.linked-usdl.org/ns/on-site> ;
        skos:prefLabel  "<p>Interaction Types by locality binding"@en .

gr:License  a             owl:Class ;
        rdfs:comment      "A license is the specification of a bundle of rights that determines the type of activity or access offered by the gr:BusinessEntity on the gr:ProductOrService through the gr:Offering.\n\t\nLicenses can be standardized (e.g. LPGL, Creative Commons, ...), vendor-specific, or individually defined for a single offer or product. Whether there is a fee for obtaining the license is specified using the gr:UnitPriceSpecification attached to the gr:Offering. Use foaf:page for linking to a document containing the license, e.g. in PDF or HTML."@en ;
        rdfs:isDefinedBy  <http://purl.org/goodrelations/v1> ;
        rdfs:label        "License"@en ;
        rdfs:subClassOf   gr:BusinessFunction .

attr:attr-performance-interoperability
        a                    usdl-pref:ServiceAttribute ;
        dcterms:created      "2014-07-18T12:03:30Z"^^xsd:dateTime ;
        dcterms:creator      ""^^xsd:string ;
        dcterms:description  "The ability of a service to easily interact with other services (from the same service provider and from other service providers)"^^xsd:string ;
        dcterms:identifier   "attr-performance-interoperability"^^xsd:string ;
        dcterms:modified     "2014-07-18T12:03:30Z"^^xsd:dateTime ;
        dcterms:title        "Interoperability"^^xsd:string ;
        skos:broader         attr:attr-performance .

gr:hasBrand  a            owl:ObjectProperty ;
        rdfs:comment      "This specifies the brand or brands (gr:Brand) associated with a gr:ProductOrService, or the brand or brands maintained by a gr:BusinessEntity."@en ;
        rdfs:domain       [ a            owl:Class ;
                            owl:unionOf  ( gr:BusinessEntity gr:ProductOrService s:Organization s:Product )
                          ] ;
        rdfs:isDefinedBy  <http://purl.org/goodrelations/v1> ;
        rdfs:label        "has brand (0..*)"@en ;
        rdfs:range        gr:Brand .

attr:attr-agility-elasticity-time
        a                    usdl-pref:ServiceAttribute ;
        dcterms:created      "2014-05-23T18:25:30Z"^^xsd:dateTime ;
        dcterms:description  ""^^xsd:string ;
        dcterms:identifier   "attr-agility-elasticity-time"^^xsd:string ;
        dcterms:modified     "2014-05-23T18:25:30Z"^^xsd:dateTime ;
        dcterms:title        "Time"^^xsd:string ;
        skos:broader         attr:attr-agility-elasticity .

<http://www.linked-usdl.org/ns/customer>
        a                  usdl-core:BusinessRole ;
        rdfs:label         "Customer"@en ;
        skos:definition    "<p>A Customer is the entity that contracted a given service from a particular provider. It is often the entity that will pay for the service. It may often coincide with the actual Consumer or end-user but need not be necessarily the case. See Consumer.</p>"@en ;
        skos:inScheme      <http://www.linked-usdl.org/ns/usdl-business-roles> ;
        skos:prefLabel     "Customer"@en ;
        skos:topConceptOf  <http://www.linked-usdl.org/ns/usdl-business-roles> .

attr:attr-reputation  a      usdl-pref:ServiceAttribute ;
        dcterms:created      "2014-05-23T21:21:41+03:00"^^xsd:dateTime ;
        dcterms:description  "It is related to the reputation of the Service provider and of the cloud service offerings that are provided"^^xsd:string ;
        dcterms:identifier   "attr-reputation"^^xsd:string ;
        dcterms:modified     "2014-07-18T16:26:05+03:00"^^xsd:dateTime ;
        dcterms:title        "Reputation"^^xsd:string ;
        skos:broader         attr:attr-root .

usdl-sla-cb:FuzzyValue
        a                 owl:Class , rdfs:Class ;
        rdfs:comment      "<p>FuzzyValue extends the notion of quantitative value specified in Good Relations to fuzzy values as specified by the Broker@Cloud optimization mechanism. This class is used by the optimization mechanism and preferences specification developed in the Broker@Cloud project for specification of imprecise (fuzzy) values in consumer preferences specifications.</p>"@en ;
        rdfs:isDefinedBy  usdl-core-cb: ;
        rdfs:label        "Fuzzy Value"@en ;
        rdfs:subClassOf   gr:QuantitativeValueFloat .

gr:depth  a                 owl:ObjectProperty ;
        rdfs:comment        "The depth of the product.\nTypical unit code(s): CMT for centimeters, INH for inches"@en ;
        rdfs:domain         [ a            owl:Class ;
                              owl:unionOf  ( gr:ProductOrService s:Product )
                            ] ;
        rdfs:isDefinedBy    <http://purl.org/goodrelations/v1> ;
        rdfs:label          "depth (0..1)"@en ;
        rdfs:range          gr:QuantitativeValue ;
        rdfs:subPropertyOf  gr:quantitativeProductOrServiceProperty .

gr:opens  a               owl:DatatypeProperty ;
        rdfs:comment      "The opening hour of the gr:Location on the given gr:DayOfWeek.\nIf no time-zone suffix is included, the time is given in the local time valid at the gr:Location.\n\nFor a time in GMT/UTC, simply add a \"Z\" following the time:\n\n09:30:10Z.\n\nAlternatively, you can specify an offset from the UTC time by adding a positive or negative time following the time:\n\n09:30:10-09:00\n\nor\n\n09:30:10+09:00.\n\nNote 1: Use 00:00:00 for the first second of the respective day and 23:59:59 for the last second of that day.\nNote 2: If a store opens at 17:00 on Saturdays and closes at 03:00:00 a.m. next morning, use 17:00:00 - 23:59:59 for Saturday and 00:00:00 - 03:00:00 for Sunday.\nNote 3: If the shop re-opens on the same day of the week or set of days of the week, you must create a second instance of gr:OpeningHoursSpecification."@en ;
        rdfs:domain       gr:OpeningHoursSpecification ;
        rdfs:isDefinedBy  <http://purl.org/goodrelations/v1> ;
        rdfs:label        "opens (1..1)"@en ;
        rdfs:range        xsd:time .

attr:attr-reputation-service-reputation
        a                    usdl-pref:ServiceAttribute ;
        dcterms:created      "2014-05-23T21:35:14+03:00"^^xsd:dateTime ;
        dcterms:description  "It is the linguistic expression of the reputation of the cloud service  as perceived by its clients"^^xsd:string ;
        dcterms:identifier   "attr-reputation-service-reputation"^^xsd:string ;
        dcterms:modified     "2014-07-18T16:26:51+03:00"^^xsd:dateTime ;
        dcterms:title        "Service Reputation"^^xsd:string ;
        skos:broader         attr:attr-reputation .

gr:ActualProductOrServiceInstance
        a                    owl:Class ;
        rdfs:comment         "DEPRECATED - This class is superseded by gr:Individual. Replace all occurrences of gr:ActualProductOrServiceInstance by gr:Individual, if possible."@en ;
        rdfs:isDefinedBy     <http://purl.org/goodrelations/v1> ;
        rdfs:label           "Actual product or service instance (DEPRECATED)"@en ;
        rdfs:subClassOf      gr:ProductOrService ;
        owl:deprecated       true ;
        owl:equivalentClass  gr:Individual .

usdl-pref:BooleanVariable
        a                 owl:Class , rdfs:Class ;
        rdfs:comment      "<p> A BooleanVariable is a special case of QualitativeVariable, used to reference a boolean value.</p> " ;
        rdfs:isDefinedBy  <http://www.linked-usdl.org/ns/usdl-pref> ;
        rdfs:label        "Boolean Variable" ;
        rdfs:subClassOf   usdl-pref:PreferenceVariable .

gr:serialNumber  a        owl:DatatypeProperty ;
        rdfs:comment      "The serial number or any alphanumeric identifier of a particular product. Note that serial number are unique only for the same brand or the same model, so you cannot infer from two occurrences of the same serial number that the objects to which they are attached are identical.\n\nThis property can also be attached to a gr:Offering in cases where the included products are not modeled in more detail."@en ;
        rdfs:domain       [ a            owl:Class ;
                            owl:unionOf  ( gr:Individual gr:Offering s:Product )
                          ] ;
        rdfs:isDefinedBy  <http://purl.org/goodrelations/v1> ;
        rdfs:label        "serial number (0..*)"@en ;
        rdfs:range        xsd:string .

usdl-pref:PreferenceVariable
        a                 owl:Class , rdfs:Class ;
        rdfs:comment      "<p>A Preference Variable is an abstract class for the subclasses QuantitativeVariable, QualitativeVariable, FuzzyVariable, and DatatypeVariable.</p>\r\n" ;
        rdfs:isDefinedBy  <http://www.linked-usdl.org/ns/usdl-pref> ;
        rdfs:label        "Preference Variable" .

s:Organization  a        owl:Class ;
        rdfs:subClassOf  gr:BusinessEntity .

attr:attr-performance-capacity
        a                    usdl-pref:ServiceAttribute ;
        dcterms:created      "2014-07-18T11:42:01Z"^^xsd:dateTime ;
        dcterms:creator      ""^^xsd:string ;
        dcterms:description  "The maximum amount of a service that a service provider can deliver while meeting agreed SLAs"^^xsd:string ;
        dcterms:identifier   "attr-performance-capacity"^^xsd:string ;
        dcterms:modified     "2014-07-18T11:42:01Z"^^xsd:dateTime ;
        dcterms:title        "Capacity"^^xsd:string ;
        skos:broader         attr:attr-performance .

s:manufacturer  a               owl:ObjectProperty ;
        owl:equivalentProperty  gr:hasManufacturer .

attr:attr-agility-elasticity-floating-ips
        a                    usdl-pref:ServiceAttribute ;
        dcterms:created      "2015-09-08T10:38:59.630+03:00"^^xsd:dateTime ;
        dcterms:description  "Number of publically accessable end points"^^xsd:string ;
        dcterms:identifier   "attr-agility-elasticity-floating-ips"^^xsd:string ;
        dcterms:modified     "2015-09-08T10:38:59.630+03:00"^^xsd:dateTime ;
        dcterms:title        "Floating IPs"^^xsd:string ;
        skos:broader         attr:attr-agility-elasticity .

attr:attr-agility-portability
        a                    usdl-pref:ServiceAttribute ;
        dcterms:created      "2014-07-18T08:16:33Z"^^xsd:dateTime ;
        dcterms:creator      ""^^xsd:string ;
        dcterms:description  "The ability of a client to easily move a service from one service provider to another with minimal disruption"^^xsd:string ;
        dcterms:identifier   "attr-agility-portability"^^xsd:string ;
        dcterms:modified     "2014-07-18T08:16:33Z"^^xsd:dateTime ;
        dcterms:title        "Portability"^^xsd:string ;
        skos:broader         attr:attr-agility .

gr:PaymentMethod  a       owl:Class ;
        rdfs:comment      "A payment method is a standardized procedure for transferring the monetary amount for a purchase. Payment methods are characterized by the legal and technical structures used, and by the organization or group carrying out the transaction. This element is mostly used for specifying the types of payment accepted by a gr:BusinessEntity.\n\nExamples: VISA, MasterCard, Diners, cash, or bank transfer in advance."@en ;
        rdfs:isDefinedBy  <http://purl.org/goodrelations/v1> ;
        rdfs:label        "Payment method"@en ;
        owl:disjointWith  gr:TypeAndQuantityNode , gr:OpeningHoursSpecification , gr:Location , gr:Brand , gr:BusinessEntityType , gr:WarrantyScope , gr:BusinessEntity , gr:DayOfWeek , gr:BusinessFunction , gr:WarrantyPromise , gr:QuantitativeValue , gr:DeliveryMethod , gr:Offering , gr:PriceSpecification .

attr:attr-performance-service-response-time-maximum
        a                    usdl-pref:ServiceAttribute ;
        dcterms:created      "2014-07-18T15:04:46+03:00"^^xsd:dateTime ;
        dcterms:description  ""^^xsd:string ;
        dcterms:identifier   "attr-performance-service-response-time-maximum"^^xsd:string ;
        dcterms:modified     "2014-07-18T15:04:46+03:00"^^xsd:dateTime ;
        dcterms:title        "Maximum Response time"^^xsd:string ;
        skos:broader         attr:attr-performance-service-response-time .

attr:attr-performance-interoperability-layer
        a                    usdl-pref:ServiceAttribute ;
        dcterms:created      "2014-07-18T12:03:51Z"^^xsd:dateTime ;
        dcterms:creator      ""^^xsd:string ;
        dcterms:description  ""^^xsd:string ;
        dcterms:identifier   "attr-performance-interoperability-layer"^^xsd:string ;
        dcterms:modified     "2014-07-18T12:03:51Z"^^xsd:dateTime ;
        dcterms:title        "Interoperability Layer"^^xsd:string ;
        skos:broader         attr:attr-performance-interoperability .

attr:attr-usability-installability
        a                    usdl-pref:ServiceAttribute ;
        dcterms:created      "2014-07-18T16:23:17+03:00"^^xsd:dateTime ;
        dcterms:description  "Installability characterizes the time and effort required to get a service ready for delivery (where applicable)"^^xsd:string ;
        dcterms:identifier   "attr-usability-installability"^^xsd:string ;
        dcterms:modified     "2014-07-18T16:23:17+03:00"^^xsd:dateTime ;
        dcterms:title        "Installability"^^xsd:string ;
        skos:broader         attr:attr-usability .

gr:billingIncrement  a    owl:DatatypeProperty ;
        rdfs:comment      "This property specifies the minimal quantity and rounding increment that will be the basis for the billing. \nThe unit of measurement is specified by the UN/CEFACT code attached to the gr:UnitPriceSpecification via the gr:hasUnitOfMeasurement property.\n\nExamples: \n- The price for gasoline is 4 USD per gallon at the pump, but you will be charged in units of 0.1 gallons.\n- The price for legal consulting is 100 USD per hour, but you will be charged in units of 15 minutes.\n\nThis property makes sense only for instances of gr:Offering that include not more than one type of good or service."@en ;
        rdfs:domain       gr:UnitPriceSpecification ;
        rdfs:isDefinedBy  <http://purl.org/goodrelations/v1> ;
        rdfs:label        "billing increment (0..1)"@en ;
        rdfs:range        xsd:float .

attr:attr-financial  a       usdl-pref:ServiceAttribute ;
        dcterms:created      "2014-07-18T12:22:34+03:00"^^xsd:dateTime ;
        dcterms:description  "It is related to the amount of money spent on the service by the client"^^xsd:string ;
        dcterms:identifier   "attr-financial"^^xsd:string ;
        dcterms:modified     "2014-07-18T12:22:34+03:00"^^xsd:dateTime ;
        dcterms:title        "Financial"^^xsd:string ;
        skos:broader         attr:attr-root .

<http://www.linked-usdl.org/ns/usdl-business-roles>
        a                              owl:Ontology , skos:ConceptScheme ;
        dcterms:creator                usdl-core:tleidig , usdl-core:cpedrinaci , usdl-core:jcardoso ;
        dcterms:description            "<p>This vocabulary provides the core business roles contemplated within Linked USDL. The taxonomy provided here is a minimal reference one. Extensions or replacements for this could be defined an used within applications in the very same way by refining BusinessRole or creating further SKOS concept schemes. </p>"@en ;
        dcterms:modified               "2013-02-11"^^xsd:date , "2014-01-14"^^xsd:date ;
        dcterms:title                  "Linked USDL Basic Business Roles concept scheme" ;
        vann:preferredNamespacePrefix  "usdl-br" ;
        vann:preferredNamespaceUri     "http://www.linked-usdl.org/ns/usdl-business-roles#" ;
        skos:hasTopConcept             <http://www.linked-usdl.org/ns/regulator> , <http://www.linked-usdl.org/ns/producer> , <http://www.linked-usdl.org/ns/customer> , <http://www.linked-usdl.org/ns/provider> , <http://www.linked-usdl.org/ns/intermediary> , <http://www.linked-usdl.org/ns/consumer> ;
        skos:prefLabel                 "Business Roles"@en ;
        foaf:page                      <http://www.linked-usdl.org/ns/usdl-business-roles.html> .

gr:Brand  a               owl:Class ;
        rdfs:comment      "A brand is the identity of a specific product, service, or business. Use foaf:logo for attaching a brand logo and gr:name or rdfs:label for attaching the brand name.\t\n\n(Source: Wikipedia, the free encyclopedia, see http://en.wikipedia.org/wiki/Brand)"@en ;
        rdfs:isDefinedBy  <http://purl.org/goodrelations/v1> ;
        rdfs:label        "Brand"@en ;
        owl:disjointWith  gr:PaymentMethod , gr:QuantitativeValue , gr:WarrantyPromise , gr:TypeAndQuantityNode , gr:BusinessFunction , gr:DayOfWeek , gr:PriceSpecification , gr:ProductOrService , gr:Offering , gr:Location , gr:DeliveryMethod , gr:WarrantyScope , gr:OpeningHoursSpecification , gr:BusinessEntityType , gr:BusinessEntity .

gr:OpeningHoursSpecification
        a                 owl:Class ;
        rdfs:comment      "This is a conceptual entity that holds together all information about the opening hours on a given day (gr:DayOfWeek)."@en ;
        rdfs:isDefinedBy  <http://purl.org/goodrelations/v1> ;
        rdfs:label        "Opening hours specification"@en ;
        owl:disjointWith  gr:BusinessEntity , gr:BusinessFunction , gr:DayOfWeek , gr:WarrantyScope , gr:TypeAndQuantityNode , gr:WarrantyPromise , gr:ProductOrService , gr:PriceSpecification , gr:PaymentMethod , gr:Brand , gr:DeliveryMethod , gr:Offering , gr:BusinessEntityType , gr:QuantitativeValue , gr:Location .

usdl-core:tleidig  a  foaf:Person ;
        foaf:name  "Torsten Leidig" .

gr:condition  a           owl:DatatypeProperty ;
        rdfs:comment      "A textual description of the condition of the product or service, or the products or services included in the offer (when attached to a gr:Offering)"@en ;
        rdfs:domain       [ a            owl:Class ;
                            owl:unionOf  ( gr:Offering gr:ProductOrService s:Product )
                          ] ;
        rdfs:isDefinedBy  <http://purl.org/goodrelations/v1> ;
        rdfs:label        "condition (0..1)"@en ;
        rdfs:range        rdfs:Literal .

attr:attr-performance-accuracy
        a                    usdl-pref:ServiceAttribute ;
        dcterms:created      "2014-07-18T15:01:37+03:00"^^xsd:dateTime ;
        dcterms:description  "The extent to which a service adheres to its requirements"^^xsd:string ;
        dcterms:identifier   "attr-performance-accuracy"^^xsd:string ;
        dcterms:modified     "2014-07-18T15:01:37+03:00"^^xsd:dateTime ;
        dcterms:title        "Accuracy"^^xsd:string ;
        skos:broader         attr:attr-performance .

usdl-core:EntityInvolvement
        a                 owl:Class , rdfs:Class ;
        rdfs:comment      "<p>EntityInvolvement helps captures a ternary relationship between Services, the BusinessEntities involved in the service process, and the Role they play, e.g., provider, intermediary, etc. This enables specifying, for instance the fact that a given insurance service is provided by a certain company, or that a third party is actually involved in the service delivery chain.</p>"@en ;
        rdfs:isDefinedBy  <http://www.linked-usdl.org/ns/usdl-core> ;
        rdfs:label        "Entity Involvement"@en .

gr:hasMaxValueFloat  a      owl:DatatypeProperty ;
        rdfs:comment        "This property captures the upper limit of a gr:QuantitativeValueFloat instance."@en ;
        rdfs:domain         gr:QuantitativeValueFloat ;
        rdfs:isDefinedBy    <http://purl.org/goodrelations/v1> ;
        rdfs:label          "has max value float (1..1)"@en ;
        rdfs:range          xsd:float ;
        rdfs:subPropertyOf  gr:hasMaxValue .

gr:hasPriceSpecification
        a                 owl:ObjectProperty ;
        rdfs:comment      "This links a gr:Offering to a gr:PriceSpecification or specifications. There can be unit price specifications, payment charge specifications, and delivery charge specifications. For each type, multiple specifications for the same gr:Offering are possible, e.g. for different quantity ranges or for different currencies, or for different combinations of gr:DeliveryMethod and target destinations.\n\nRecommended retail prices etc. can be marked by the gr:priceType property of the gr:UnitPriceSpecification."@en ;
        rdfs:domain       [ a            owl:Class ;
                            owl:unionOf  ( gr:Offering s:Offer )
                          ] ;
        rdfs:isDefinedBy  <http://purl.org/goodrelations/v1> ;
        rdfs:label        "has price specification (0..*)"@en ;
        rdfs:range        gr:PriceSpecification .

gr:color  a                 owl:DatatypeProperty ;
        rdfs:comment        "The color of the product."@en ;
        rdfs:domain         [ a            owl:Class ;
                              owl:unionOf  ( gr:ProductOrService s:Product )
                            ] ;
        rdfs:isDefinedBy    <http://purl.org/goodrelations/v1> ;
        rdfs:label          "color (0..1)"@en ;
        rdfs:range          rdfs:Literal ;
        rdfs:subPropertyOf  gr:datatypeProductOrServiceProperty .

attr:attr-assurance-resiliency-fault-tolerance
        a                    usdl-pref:ServiceAttribute ;
        dcterms:created      "2014-07-18T08:54:24Z"^^xsd:dateTime ;
        dcterms:creator      ""^^xsd:string ;
        dcterms:description  "The ability of a service to continue to operate properly in the event of a failure in one or more of its components"^^xsd:string ;
        dcterms:identifier   "attr-assurance-resiliency-fault-tolerance"^^xsd:string ;
        dcterms:modified     "2014-07-18T08:54:24Z"^^xsd:dateTime ;
        dcterms:title        "Resiliency/Fault Tolerance"^^xsd:string ;
        skos:broader         attr:attr-assurance .

gr:MasterCard  a          gr:PaymentMethodCreditCard ;
        rdfs:comment      "Payment by credit or debit cards issued by the MasterCard network."@en ;
        rdfs:isDefinedBy  <http://purl.org/goodrelations/v1> ;
        rdfs:label        "MasterCard (payment method)"@en .

gr:ProvideService  a      gr:BusinessFunction ;
        rdfs:comment      "This gr:BusinessFunction indicates that the gr:BusinessEntity offers (or seeks) the respective type of service.\n\nNote: Maintain and Repair are also types of Services. However, products and services ontologies often provide classes for tangible products as well as for types of services. The business function gr:ProvideService is to be used with such goods that are services, while gr:Maintain and gr:Repair can be used with goods for which only the class of product exists in the ontology, but not the respective type of service.\n\nExample: Car maintenance could be expressed both as \"provide the service car maintenance\" or \"maintain cars\"."@en ;
        rdfs:isDefinedBy  <http://purl.org/goodrelations/v1> ;
        rdfs:label        "Provide service (business function)"@en .

attr:attr-assurance-service-stability-memory
        a                    usdl-pref:ServiceAttribute ;
        dcterms:created      "2014-05-23T18:29:30Z"^^xsd:dateTime ;
        dcterms:description  ""^^xsd:string ;
        dcterms:identifier   "attr-assurance-service-stability-memory"^^xsd:string ;
        dcterms:modified     "2014-05-23T18:29:30Z"^^xsd:dateTime ;
        dcterms:title        "Memory"^^xsd:string ;
        skos:broader         attr:attr-assurance-service-stability .

usdl-testing:TestAdequacyCriteria
        a                 owl:Class , rdfs:Class ;
        rdfs:comment      "<p> Test Adequacy Criteria serves as a root class for a taxonomy providing vocabulary for classification of the test adequacy criteria of a testing method. </p>"@en ;
        rdfs:isDefinedBy  <http://www.linked-usdl.org/ns/usdl-core/cloud-broker/testing> ;
        rdfs:label        "Test Adequacy Criteria"@en ;
        rdfs:subClassOf   skos:Concept .

usdl-core:InteractionType
        rdfs:comment      "<p>This concept covers the kinds of interactions that an entity may take place within an InteractionPoint. One may define as many InteractionTypes as necessary by defining subclasses of InteractionType or by creating SKOS concept schemes. For completeness Linked USDL Core provides a basic concept scheme for the main interaction types that can be used out of the box or as reference for specific extensions. See Linked USDL Interaction Types Module.</p>"@en ;
        rdfs:isDefinedBy  <http://www.linked-usdl.org/ns/usdl-core> ;
        rdfs:label        "Interaction Type"@en ;
        rdfs:subClassOf   skos:Concept .

usdl-sla-cb:hasMaxKernel
        a                   rdf:Property ;
        rdfs:comment        "<p>Indicates a max kernel.</p>"@en ;
        rdfs:domain         usdl-sla-cb:FuzzyValue ;
        rdfs:isDefinedBy    usdl-core-cb: ;
        rdfs:label          "has max kernel"@en ;
        rdfs:range          xsd:float ;
        rdfs:subPropertyOf  gr:hasMaxValueFloat .

usdl-testing:TestingProcedure
        a                 owl:Class , rdfs:Class ;
        rdfs:comment      "<p>Testing Procedure serves as anchor to attach testing instructions and the testing method to be used with the service description.</p>"@en ;
        rdfs:isDefinedBy  <http://www.linked-usdl.org/ns/usdl-core/cloud-broker/testing> ;
        rdfs:label        "Testing Procedure"@en .

s:name  a                       owl:DatatypeProperty ;
        owl:equivalentProperty  gr:name .

gr:appliesToPaymentMethod
        a                 owl:ObjectProperty ;
        rdfs:comment      "This property specifies the gr:PaymentMethod to which the gr:PaymentChargeSpecification applies."@en ;
        rdfs:domain       gr:PaymentChargeSpecification ;
        rdfs:isDefinedBy  <http://purl.org/goodrelations/v1> ;
        rdfs:label        "applies to payment method (1..*)"@en ;
        rdfs:range        gr:PaymentMethod .

gr:hasDUNS  a             owl:DatatypeProperty ;
        rdfs:comment      "The Dun & Bradstreet DUNS number for identifying a gr:BusinessEntity. The Dun & Bradstreet DUNS is a nine-digit number used to identify legal entities (but usually not branches or locations of logistical importance only)."@en ;
        rdfs:domain       [ a            owl:Class ;
                            owl:unionOf  ( gr:BusinessEntity s:Organization )
                          ] ;
        rdfs:isDefinedBy  <http://purl.org/goodrelations/v1> ;
        rdfs:label        "has DUNS (0..1)"@en ;
        rdfs:range        xsd:string .

gr:Dispose  a             gr:BusinessFunction ;
        rdfs:comment      "This gr:BusinessFunction indicates that the gr:BusinessEntity offers (or seeks) the acceptance of the specified gr:ProductOrService for proper disposal, recycling, or any other kind of allowed usages, freeing the current owner from all rights and obligations of ownership."@en ;
        rdfs:isDefinedBy  <http://purl.org/goodrelations/v1> ;
        rdfs:label        "Dispose (business function)"@en .

usdl-testing:ExploratoryTesting
        a                  usdl-testing:TestingGoal ;
        rdfs:label         "Exploratory Testing"@en ;
        skos:altLabel      "Exploratory Testing"@en ;
        skos:definition    "<p>A testing method is an exploratory testing method.</p>"@en ;
        skos:inScheme      usdl-testing:TestingGoalClassificationScheme ;
        skos:prefLabel     "Exploratory Testing"@en ;
        skos:topConceptOf  usdl-testing:TestingGoalClassificationScheme .

gr:valueAddedTaxIncluded
        a                 owl:DatatypeProperty ;
        rdfs:comment      "This property specifies whether the applicable value-added tax (VAT)  is included in the price of the gr:PriceSpecification or not.\n\nNote: This is a simple representation which may not properly reflect all details of local taxation."@en ;
        rdfs:domain       gr:PriceSpecification ;
        rdfs:isDefinedBy  <http://purl.org/goodrelations/v1> ;
        rdfs:label        "value added tax included (0..1)"@en ;
        rdfs:range        xsd:boolean .

attr:attr-security-retention-disposition
        a                    usdl-pref:ServiceAttribute ;
        dcterms:created      "2014-07-18T12:56:25Z"^^xsd:dateTime ;
        dcterms:creator      ""^^xsd:string ;
        dcterms:description  "The service provider's data retention and disposition processes meet the clients' requirements"^^xsd:string ;
        dcterms:identifier   "attr-security-retention-disposition"^^xsd:string ;
        dcterms:modified     "2014-07-18T12:56:25Z"^^xsd:dateTime ;
        dcterms:title        "Retention/Disposition"^^xsd:string ;
        skos:broader         attr:attr-security .

attr:attr-financial-cost-operation-cost
        a                    usdl-pref:ServiceAttribute ;
        dcterms:created      "2014-05-23T18:32:03Z"^^xsd:dateTime ;
        dcterms:creator      ""^^xsd:string ;
        dcterms:description  ""^^xsd:string ;
        dcterms:identifier   "attr-financial-cost-operation-cost"^^xsd:string ;
        dcterms:modified     "2014-07-18T09:25:18Z"^^xsd:dateTime ;
        dcterms:title        "Operating cost"^^xsd:string ;
        skos:broader         attr:attr-financial-cost .

gr:BusinessFunction  a    owl:Class ;
        rdfs:comment      "The business function specifies the type of activity or access (i.e., the bundle of rights) offered by the gr:BusinessEntity on the gr:ProductOrService through the gr:Offering. Typical are sell, rental or lease, maintenance or repair, manufacture / produce, recycle / dispose, engineering / construction, or installation.\n\nLicenses and other proprietary specifications of access rights are also instances of this class.\n\nExamples: A particular offering made by Miller Rentals Ltd. says that they (1) sell Volkswagen Golf convertibles, (2) lease out a particular Ford pick-up truck, and (3) dispose car wrecks of any make and model."@en ;
        rdfs:isDefinedBy  <http://purl.org/goodrelations/v1> ;
        rdfs:label        "Business function"@en ;
        owl:disjointWith  gr:WarrantyPromise , gr:PaymentMethod , gr:PriceSpecification , gr:BusinessEntityType , gr:Location , gr:ProductOrService , gr:Offering , gr:TypeAndQuantityNode , gr:WarrantyScope , gr:OpeningHoursSpecification , gr:QuantitativeValue , gr:BusinessEntity , gr:Brand , gr:DeliveryMethod , gr:DayOfWeek .

gr:hasNAICS  a            owl:DatatypeProperty ;
        rdfs:comment      "The North American Industry Classification System (NAICS) code for a particular gr:BusinessEntity.\nSee http://www.census.gov/eos/www/naics/ for more details.\n\nNote: While NAICS codes are sometimes misused for classifying products or services, they are designed and suited only for classifying business establishments."@en ;
        rdfs:domain       [ a            owl:Class ;
                            owl:unionOf  ( gr:BusinessEntity s:Organization )
                          ] ;
        rdfs:isDefinedBy  <http://purl.org/goodrelations/v1> ;
        rdfs:label        "has NAICS (0..*)"@en ;
        rdfs:range        xsd:int .

usdl-pref:hasPreference
        a                 rdf:Property ;
        rdfs:comment      "<p>Consumer preference descriptions </p>\r\n" ;
        rdfs:domain       usdl-pref:ConsumerPreferenceProfile ;
        rdfs:isDefinedBy  <http://www.linked-usdl.org/ns/usdl-pref> ;
        rdfs:label        "has preference" ;
        rdfs:range        usdl-pref:ConsumerPreference .

gr:validFrom  a           owl:DatatypeProperty ;
        rdfs:comment      "This property specifies the beginning of the validity of the gr:Offering, gr:PriceSpecification, gr:License, or gr:OpeningHoursSpecification.\nA time-zone should be specified. For a time in GMT/UTC, simply add a \"Z\" following the time:\n\n2008-05-30T09:30:10Z.\n\nAlternatively, you can specify an offset from the UTC time by adding a positive or negative time following the time:\n\n2008-05-30T09:30:10-09:00\n\nor\n\n2008-05-30T09:30:10+09:00.\n\nNote: If multiple contradicting instances of a gr:Offering, gr:PriceSpecification, or gr:OpeningHoursSpecification exist, it is a good heuristics to assume that\n1. Information with validity information for the respective period of time ranks higher than information without validity information.\n2. Among conflicting nodes both having validity information, the one with the shorter validity span ranks higher."@en ;
        rdfs:domain       [ a            owl:Class ;
                            owl:unionOf  ( gr:Offering gr:OpeningHoursSpecification gr:PriceSpecification gr:License s:Offer )
                          ] ;
        rdfs:isDefinedBy  <http://purl.org/goodrelations/v1> ;
        rdfs:label        "valid from (0..1)"@en ;
        rdfs:range        xsd:dateTime .

usdl-core:SAP-Karlsruhe
        a              foaf:Organization ;
        foaf:homepage  <http://www.sap.com> ;
        foaf:member    usdl-core:tleidig ;
        foaf:name      "SAP Research Center CEC Karlsruhe, SAP AG" .

gr:DeliveryChargeSpecification
        a                 owl:Class ;
        rdfs:comment      "A delivery charge specification is a conceptual entity that specifies the additional costs asked for the delivery of a given gr:Offering using a particular gr:DeliveryMethod by the respective gr:BusinessEntity. A delivery charge specification is characterized by (1) a monetary amount per order, specified as a literal value of type float in combination with a currency, (2) the delivery method, (3) the target country or region, and (4)  whether this charge includes local sales taxes, namely VAT.\nA gr:Offering may be linked to multiple gr:DeliveryChargeSpecification nodes that specify alternative charges for disjoint combinations of target countries or regions, and delivery methods.\n\nExamples: Delivery by direct download is free of charge worldwide, delivery by UPS to Germany is 10 Euros per order, delivery by mail within the US is 5 Euros per order.\n\nThe total amount of this charge is specified as a float value of the gr:hasCurrencyValue property. The currency is specified via the gr:hasCurrency datatype property. Whether the price includes VAT or not is indicated by the gr:valueAddedTaxIncluded property. The gr:DeliveryMethod to which this charge applies is specified using the gr:appliesToDeliveryMethod object property. The region or regions to which this charge applies is specified using the gr:eligibleRegions property, which uses ISO 3166-1 and ISO 3166-2 codes.\n\nIf the price can only be given as a range, use gr:hasMaxCurrencyValue and gr:hasMinCurrencyValue for the upper and lower bounds.\n\nImportant: When querying for the price, always use gr:hasMaxCurrencyValue and gr:hasMinCurrencyValue."@en ;
        rdfs:isDefinedBy  <http://purl.org/goodrelations/v1> ;
        rdfs:label        "Delivery charge specification"@en ;
        rdfs:subClassOf   gr:PriceSpecification ;
        owl:disjointWith  gr:UnitPriceSpecification , gr:PaymentChargeSpecification .

dcterms:license  a  owl:AnnotationProperty .

usdl-pref:DatatypeVariable
        a                 owl:Class , rdfs:Class ;
        rdfs:comment      "<p> A DatatypeVariable is used to reference a datatype value.</p> " ;
        rdfs:isDefinedBy  <http://www.linked-usdl.org/ns/usdl-pref> ;
        rdfs:label        "Datatype Variable" ;
        rdfs:subClassOf   usdl-pref:PreferenceVariable .

attr:attr-assurance-serviceability-free-support
        a                    usdl-pref:ServiceAttribute ;
        dcterms:created      "2014-05-23T21:29:49+03:00"^^xsd:dateTime ;
        dcterms:description  ""^^xsd:string ;
        dcterms:identifier   "attr-assurance-serviceability-free-support"^^xsd:string ;
        dcterms:modified     "2014-05-23T21:29:49+03:00"^^xsd:dateTime ;
        dcterms:title        "Free Support"^^xsd:string ;
        skos:broader         attr:attr-assurance-serviceability .

attr:attr-assurance-reliability
        a                    usdl-pref:ServiceAttribute ;
        dcterms:created      "2014-07-18T08:53:48Z"^^xsd:dateTime ;
        dcterms:creator      ""^^xsd:string ;
        dcterms:description  "It reflects measures of how a service operates without failure under given conditions during a given time period"^^xsd:string ;
        dcterms:identifier   "attr-assurance-reliability"^^xsd:string ;
        dcterms:modified     "2014-07-18T08:53:48Z"^^xsd:dateTime ;
        dcterms:title        "Reliability"^^xsd:string ;
        skos:broader         attr:attr-assurance .

attr:attr-accountability-ownership
        a                    usdl-pref:ServiceAttribute ;
        dcterms:created      "2014-07-18T07:34:26Z"^^xsd:dateTime ;
        dcterms:creator      ""^^xsd:string ;
        dcterms:description  "The level of rights a client has over client data, software licenses, and intellectual property associated with a service"^^xsd:string ;
        dcterms:identifier   "attr-accountability-ownership"^^xsd:string ;
        dcterms:modified     "2014-07-18T07:34:26Z"^^xsd:dateTime ;
        dcterms:title        "Ownership"^^xsd:string ;
        skos:broader         attr:attr-accountability .

attr:attr-security-management
        a                    usdl-pref:ServiceAttribute ;
        dcterms:created      "2014-07-18T15:56:50+03:00"^^xsd:dateTime ;
        dcterms:description  "The capabilities of service providers to ensure application, data, and infrastructure security based on the security requirements of the client"^^xsd:string ;
        dcterms:identifier   "attr-security-management"^^xsd:string ;
        dcterms:modified     "2014-07-18T15:56:50+03:00"^^xsd:dateTime ;
        dcterms:title        "Security Management"^^xsd:string ;
        skos:broader         attr:attr-security .

attr:attr-assurance-serviceability-os-support
        a                    usdl-pref:ServiceAttribute ;
        dcterms:created      "2014-07-18T09:14:14Z"^^xsd:dateTime ;
        dcterms:creator      ""^^xsd:string ;
        dcterms:description  ""^^xsd:string ;
        dcterms:identifier   "attr-assurance-serviceability-os-support"^^xsd:string ;
        dcterms:modified     "2014-07-18T09:14:14Z"^^xsd:dateTime ;
        dcterms:title        "Operating Systems Support"^^xsd:string ;
        skos:broader         attr:attr-assurance-serviceability .

usdl-core:yields  a       rdf:Property ;
        rdfs:comment      "<p>Outcome yielded by an InteractionPoint.</p>"@en ;
        rdfs:domain       usdl-core:InteractionPoint ;
        rdfs:isDefinedBy  <http://www.linked-usdl.org/ns/usdl-core> ;
        rdfs:label        "yields"@en ;
        rdfs:range        rdfs:Class .

attr:attr-reputation-contracting-experience
        a                    usdl-pref:ServiceAttribute ;
        dcterms:created      "2014-07-18T13:31:30Z"^^xsd:dateTime ;
        dcterms:creator      ""^^xsd:string ;
        dcterms:description  "Indicators of client effort and satisfaction with the process of entering into the agreements required to use a service"^^xsd:string ;
        dcterms:identifier   "attr-reputation-contracting-experience"^^xsd:string ;
        dcterms:modified     "2014-07-18T13:31:30Z"^^xsd:dateTime ;
        dcterms:title        "Contracting Experience"^^xsd:string ;
        skos:broader         attr:attr-reputation .

attr:attr-performance-capacity-turbo-frequency
        a                    usdl-pref:ServiceAttribute ;
        dcterms:created      "2014-07-18T11:57:11Z"^^xsd:dateTime ;
        dcterms:creator      ""^^xsd:string ;
        dcterms:description  ""^^xsd:string ;
        dcterms:identifier   "attr-performance-capacity-turbo-frequency"^^xsd:string ;
        dcterms:modified     "2014-07-18T11:57:11Z"^^xsd:dateTime ;
        dcterms:title        "Turbo Frequency"^^xsd:string ;
        skos:broader         attr:attr-performance-capacity .

usdl-sla-cb:fuzzyServiceProperty
        a                   rdf:Property ;
        rdfs:comment        "<p>Indicates a fuzzy service property.</p>"@en ;
        rdfs:domain         usdl-core:Service ;
        rdfs:isDefinedBy    usdl-core-cb: ;
        rdfs:label          "fuzzy service property"@en ;
        rdfs:range          usdl-sla-cb:FuzzyValue ;
        rdfs:subPropertyOf  gr:hasQuantitativeProductOrServiceProperty .

gr:hasMaxValueInteger
        a                   owl:DatatypeProperty ;
        rdfs:comment        "This property captures the upper limit of a gr:QuantitativeValueInteger instance."@en ;
        rdfs:domain         gr:QuantitativeValueInteger ;
        rdfs:isDefinedBy    <http://purl.org/goodrelations/v1> ;
        rdfs:label          "has max value integer (1..1)"@en ;
        rdfs:range          xsd:int ;
        rdfs:subPropertyOf  gr:hasMaxValue .

usdl-core:KMi  a       foaf:Organization ;
        foaf:homepage  <http://kmi.open.ac.uk> ;
        foaf:member    usdl-core:cpedrinaci ;
        foaf:name      "Knowledge Media Institute, The Open University" .

gr:DeliveryMethod  a      owl:Class ;
        rdfs:comment      "A delivery method is a standardized procedure for transferring the product or service to the destination of fulfilment chosen by the customer. Delivery methods are characterized by the means of transportation used, and by the organization or group that is the contracting party for the sending gr:BusinessEntity (this is important, since the contracted party may subcontract the fulfilment to smaller, regional businesses).\n\nExamples: Delivery by mail, delivery by direct download, delivery by UPS"@en ;
        rdfs:isDefinedBy  <http://purl.org/goodrelations/v1> ;
        rdfs:label        "Delivery method"@en ;
        owl:disjointWith  gr:BusinessFunction , gr:WarrantyPromise , gr:DayOfWeek , gr:QuantitativeValue , gr:Brand , gr:ProductOrService , gr:BusinessEntity , gr:Offering , gr:Location , gr:WarrantyScope , gr:PriceSpecification , gr:PaymentMethod , gr:TypeAndQuantityNode , gr:OpeningHoursSpecification , gr:BusinessEntityType .

usdl-testing:afriesen
        a          foaf:Person ;
        foaf:name  "Andreas Friesen" .

usdl-testing:hasStrategy
        a                 rdf:Property ;
        rdfs:comment      "<p>Connects TestingMethod to TestGenerationStrategy classification dimension.</p>"@en ;
        rdfs:domain       usdl-testing:TestingMethod ;
        rdfs:isDefinedBy  <http://www.linked-usdl.org/ns/usdl-core/cloud-broker/testing> ;
        rdfs:label        "has strategy"@en ;
        rdfs:range        usdl-testing:TestGenerationStrategy .

attr:attr-assurance-serviceability-support-satisfaction
        a                    usdl-pref:ServiceAttribute ;
        dcterms:created      "2014-05-23T18:30:36Z"^^xsd:dateTime ;
        dcterms:description  ""^^xsd:string ;
        dcterms:identifier   "attr-assurance-serviceability-support-satisfaction"^^xsd:string ;
        dcterms:modified     "2014-05-23T18:30:36Z"^^xsd:dateTime ;
        dcterms:title        "Support satisfaction"^^xsd:string ;
        skos:broader         attr:attr-assurance-serviceability .

usdl-testing:TestingScaleClassificationScheme
        a                    skos:ConceptScheme ;
        dcterms:description  "<p>This vocabulary provides the concepts to classify testing scale dimension. </p>"@en ;
        dcterms:title        "Testing Scale classification concept scheme" ;
        skos:hasTopConcept   usdl-testing:SystemTesting , usdl-testing:IntegrationTesting , usdl-testing:UnitTesting ;
        skos:prefLabel       "Testing Scale Classification"@en .

usdl-testing:hasCode  a   rdf:Property ;
        rdfs:comment      "<p>Can be used to characterize the TestingMethod by a (de facto) standardized code. </p>"@en ;
        rdfs:domain       usdl-testing:TestingMethod ;
        rdfs:isDefinedBy  <http://www.linked-usdl.org/ns/usdl-core/cloud-broker/testing> ;
        rdfs:label        "has code"@en ;
        rdfs:range        xsd:String .

gr:hasEligibleQuantity
        a                 owl:ObjectProperty ;
        rdfs:comment      "This specifies the interval and unit of measurement of ordering quantities for which the gr:Offering or gr:PriceSpecification is valid. This allows e.g. specifying that a certain freight charge is valid only for a certain quantity.\nNote that if an offering is a bundle, i.e. it consists of more than one unit of a single type of good, or if the unit of measurement for the good is different from unit (Common Code C62), then gr:hasEligibleQuantity refers to units of this bundle. In other words, \"C62\" for \"Units or pieces\" is usually the appropriate unit of measurement."@en ;
        rdfs:domain       [ a            owl:Class ;
                            owl:unionOf  ( gr:Offering gr:PriceSpecification s:Offer )
                          ] ;
        rdfs:isDefinedBy  <http://purl.org/goodrelations/v1> ;
        rdfs:label        "has eligible quantity (0..1)"@en ;
        rdfs:range        gr:QuantitativeValue .

attr:attr-performance-interoperability-level
        a                    usdl-pref:ServiceAttribute ;
        dcterms:created      "2014-07-18T12:04:06Z"^^xsd:dateTime ;
        dcterms:creator      ""^^xsd:string ;
        dcterms:description  ""^^xsd:string ;
        dcterms:identifier   "attr-performance-interoperability-level"^^xsd:string ;
        dcterms:modified     "2014-07-18T12:04:06Z"^^xsd:dateTime ;
        dcterms:title        "Interoperability level"^^xsd:string ;
        skos:broader         attr:attr-performance-interoperability .

gr:typeOfGood  a          owl:ObjectProperty ;
        rdfs:comment      "This specifies the gr:ProductOrService that the gr:TypeAndQuantityNode is referring to."@en ;
        rdfs:domain       gr:TypeAndQuantityNode ;
        rdfs:isDefinedBy  <http://purl.org/goodrelations/v1> ;
        rdfs:label        "type of good (1..1)"@en ;
        rdfs:range        [ a            owl:Class ;
                            owl:unionOf  ( gr:Individual gr:SomeItems )
                          ] .

attr:attr-agility-adaptability
        a                    usdl-pref:ServiceAttribute ;
        dcterms:created      "2014-07-18T08:13:04Z"^^xsd:dateTime ;
        dcterms:creator      ""^^xsd:string ;
        dcterms:description  "The ability of the service provider to adjust to changes in client requirements"^^xsd:string ;
        dcterms:identifier   "attr-agility-adaptability"^^xsd:string ;
        dcterms:modified     "2014-07-18T08:13:04Z"^^xsd:dateTime ;
        dcterms:title        "Adaptability"^^xsd:string ;
        skos:broader         attr:attr-agility .

attr:attr-performance-functionality-features
        a                    usdl-pref:ServiceAttribute ;
        dcterms:created      "2014-07-18T12:02:21Z"^^xsd:dateTime ;
        dcterms:creator      ""^^xsd:string ;
        dcterms:description  ""^^xsd:string ;
        dcterms:identifier   "attr-performance-functionality-features"^^xsd:string ;
        dcterms:modified     "2014-07-18T12:02:21Z"^^xsd:dateTime ;
        dcterms:title        "Features"^^xsd:string ;
        skos:broader         attr:attr-performance-functionality .

attr:attr-performance-capacity-clock-speed
        a                    usdl-pref:ServiceAttribute ;
        dcterms:created      "2014-07-18T11:56:52Z"^^xsd:dateTime ;
        dcterms:creator      ""^^xsd:string ;
        dcterms:description  ""^^xsd:string ;
        dcterms:identifier   "attr-performance-capacity-clock-speed"^^xsd:string ;
        dcterms:modified     "2014-07-18T11:56:52Z"^^xsd:dateTime ;
        dcterms:title        "Clock Speed"^^xsd:string ;
        skos:broader         attr:attr-performance-capacity .

attr:attr-performance-capacity-storage-throughput
        a                    usdl-pref:ServiceAttribute ;
        dcterms:created      "2014-07-18T11:58:20Z"^^xsd:dateTime ;
        dcterms:creator      ""^^xsd:string ;
        dcterms:description  ""^^xsd:string ;
        dcterms:identifier   "attr-performance-capacity-storage-throughput"^^xsd:string ;
        dcterms:modified     "2014-07-18T11:58:20Z"^^xsd:dateTime ;
        dcterms:title        "Storage Throughput"^^xsd:string ;
        skos:broader         attr:attr-performance-capacity .

attr:attr-reputation-sustainability-economical-impact
        a                    usdl-pref:ServiceAttribute ;
        dcterms:created      "2014-07-18T13:34:41Z"^^xsd:dateTime ;
        dcterms:creator      ""^^xsd:string ;
        dcterms:description  ""^^xsd:string ;
        dcterms:identifier   "attr-reputation-sustainability-economical-impact"^^xsd:string ;
        dcterms:modified     "2014-07-18T13:34:41Z"^^xsd:dateTime ;
        dcterms:title        "Economical impact"^^xsd:string ;
        skos:broader         attr:attr-reputation-sustainability .

gr:hasPOS  a              owl:ObjectProperty ;
        rdfs:comment      "This property states that the respective gr:Location is a point of sale for the respective gr:BusinessEntity. It allows linking those two types of entities without the need for a particular gr:Offering."@en ;
        rdfs:domain       [ a            owl:Class ;
                            owl:unionOf  ( gr:BusinessEntity s:Organization )
                          ] ;
        rdfs:isDefinedBy  <http://purl.org/goodrelations/v1> ;
        rdfs:label        "has POS (0..*)"@en ;
        rdfs:range        gr:Location .

gr:JCB  a                 gr:PaymentMethodCreditCard ;
        rdfs:comment      "Payment by credit or debit cards issued by the JCB network."@en ;
        rdfs:isDefinedBy  <http://purl.org/goodrelations/v1> ;
        rdfs:label        "JCB (payment method)"@en .

gr:hasManufacturer  a     owl:ObjectProperty ;
        rdfs:comment      "This object property links a gr:ProductOrService to the gr:BusinessEntity that produces it. Mostly used with gr:ProductOrServiceModel."@en ;
        rdfs:domain       [ a            owl:Class ;
                            owl:unionOf  ( gr:ProductOrService s:Product )
                          ] ;
        rdfs:isDefinedBy  <http://purl.org/goodrelations/v1> ;
        rdfs:label        "has manufacturer (0..1)"@en ;
        rdfs:range        gr:BusinessEntity .

gr:ProductOrServicesSomeInstancesPlaceholder
        a                    owl:Class ;
        rdfs:comment         "DEPRECATED - This class is superseded by gr:SomeItems. Replace all occurrences of gr:ProductOrServicesSomeInstancesPlaceholder by gr:SomeItems, if possible."@en ;
        rdfs:isDefinedBy     <http://purl.org/goodrelations/v1> ;
        rdfs:label           "Product or services some instances placeholder (DEPRECATED)"@en ;
        rdfs:subClassOf      gr:ProductOrService ;
        owl:deprecated       true ;
        owl:equivalentClass  gr:SomeItems .

attr:attr-performance-capacity-num-of-threads-per-core
        a                    usdl-pref:ServiceAttribute ;
        dcterms:created      "2014-07-18T11:56:30Z"^^xsd:dateTime ;
        dcterms:creator      ""^^xsd:string ;
        dcterms:description  ""^^xsd:string ;
        dcterms:identifier   "attr-performance-capacity-num-of-threads-per-core"^^xsd:string ;
        dcterms:modified     "2014-07-18T11:56:30Z"^^xsd:dateTime ;
        dcterms:title        "Number of Threads per Core"^^xsd:string ;
        skos:broader         attr:attr-performance-capacity .

attr:attr-security-management-encryption-type
        a                    usdl-pref:ServiceAttribute ;
        dcterms:created      "2014-07-18T15:57:28+03:00"^^xsd:dateTime ;
        dcterms:description  ""^^xsd:string ;
        dcterms:identifier   "attr-security-management-encryption-type"^^xsd:string ;
        dcterms:modified     "2014-07-18T15:57:28+03:00"^^xsd:dateTime ;
        dcterms:title        "Encryption Type"^^xsd:string ;
        skos:broader         attr:attr-security-management .

<http://www.linked-usdl.org/ns/provider>
        a                  usdl-core:BusinessRole ;
        rdfs:label         "Provider"@en ;
        skos:altLabel      "Supplier"@en ;
        skos:definition    "<p>A Provider is the entity responsible for providing the Service.</p>"@en ;
        skos:inScheme      <http://www.linked-usdl.org/ns/usdl-business-roles> ;
        skos:prefLabel     "Provider"@en ;
        skos:topConceptOf  <http://www.linked-usdl.org/ns/usdl-business-roles> .

usdl-testing:UnitTesting
        a                  usdl-testing:TestingScale ;
        rdfs:label         "Unit Testing"@en ;
        skos:altLabel      "Unit Testing"@en ;
        skos:definition    "<p>A testing method is a unit testing method.</p>"@en ;
        skos:inScheme      usdl-testing:TestingScaleClassificationScheme ;
        skos:prefLabel     "Unit Testing"@en ;
        skos:topConceptOf  usdl-testing:TestingScaleClassificationScheme .

usdl-sla-cb:hasMinSupport
        a                   rdf:Property ;
        rdfs:comment        "<p>Indicates a min support.</p>"@en ;
        rdfs:domain         usdl-sla-cb:FuzzyValue ;
        rdfs:isDefinedBy    usdl-core-cb: ;
        rdfs:label          "has min support"@en ;
        rdfs:range          xsd:float ;
        rdfs:subPropertyOf  gr:hasMinValueFloat .

gr:hasMPN  a                owl:DatatypeProperty ;
        rdfs:comment        "The Manufacturer Part Number or MPN is a unique identifier for a product, service, or bundle from the perspective of a particular manufacturer. MPNs can be assigned to products or product datasheets, or bundles. Accordingly, the domain of this property is the union of gr:ProductOrService (the common superclass of goods and datasheets), and gr:Offering.\n\nImportant: Be careful when assuming two products or services instances or offering instances to be identical based on the MPN. Since MPNs are unique only for the same gr:BusinessEntity, this holds only when the two MPN values refer to the same gr:BusinessEntity. Such can be done by taking into account the provenance of the data. \n\nUsually, the properties gr:hasEAN_UCC-13 and gr:hasGTIN-14 are much more reliable identifiers, because they are globally unique.\n\nSee also http://en.wikipedia.org/wiki/Part_number"@en ;
        rdfs:domain         [ a            owl:Class ;
                              owl:unionOf  ( gr:Offering gr:ProductOrService s:Product )
                            ] ;
        rdfs:isDefinedBy    <http://purl.org/goodrelations/v1> ;
        rdfs:label          "has MPN (0..*)"@en ;
        rdfs:range          xsd:string ;
        rdfs:subPropertyOf  s:productID .

<http://www.linked-usdl.org/ns/on-site>
        a                  usdl-core:InteractionType ;
        rdfs:label         "On-site"@en ;
        skos:altLabel      "On-site Interaction"@en ;
        skos:definition    "<p>The interaction between the two parties requires to take place on-site, e.g., for most hair-dressing services you need to go to their place to cut your hair.</p>"@en ;
        skos:inScheme      <http://www.linked-usdl.org/ns/usdl-interaction-types> ;
        skos:prefLabel     "On-site"@en ;
        skos:topConceptOf  <http://www.linked-usdl.org/ns/usdl-interaction-types> .

gr:Discover  a            gr:PaymentMethodCreditCard ;
        rdfs:comment      "Payment by credit or debit cards issued by the Discover network."@en ;
        rdfs:isDefinedBy  <http://purl.org/goodrelations/v1> ;
        rdfs:label        "Discover (payment method)"@en .

gr:hasEAN_UCC-13  a         owl:DatatypeProperty ;
        rdfs:comment        "The EAN·UCC-13 code of the given gr:ProductOrService or gr:Offering. This code is now officially called GTIN-13 (Global Trade Identifier Number) or EAN·UCC-13. Former 12-digit UPC codes can be converted into EAN·UCC-13 code by simply adding a preceeding zero.\n\nNote 1: When using this property for searching by 12-digit UPC codes, you must add a preceeding zero digit.\nNote 2: As of January 1, 2007, the former ISBN numbers for books etc. have been integrated into the EAN·UCC-13 code. For each old ISBN-10 code, there exists a proper translation into EAN·UCC-13 by adding \"978\" or \"979\" as prefix. Since the old ISBN-10 is now deprecated, GoodRelations does not provide a property for ISBNs."@en ;
        rdfs:domain         [ a            owl:Class ;
                              owl:unionOf  ( gr:Offering gr:ProductOrService s:Product )
                            ] ;
        rdfs:isDefinedBy    <http://purl.org/goodrelations/v1> ;
        rdfs:label          "has EAN/UCC-13 (0..*)"@en ;
        rdfs:range          xsd:string ;
        rdfs:subPropertyOf  s:productID .

attr:attr-security-proactive-threat-vulnerability-management-firewall-utm
        a                    usdl-pref:ServiceAttribute ;
        dcterms:created      "2014-07-18T12:55:50Z"^^xsd:dateTime ;
        dcterms:creator      ""^^xsd:string ;
        dcterms:description  ""^^xsd:string ;
        dcterms:identifier   "attr-security-proactive-threat-vulnerability-management-firewall-utm"^^xsd:string ;
        dcterms:modified     "2014-07-18T12:55:50Z"^^xsd:dateTime ;
        dcterms:title        "Firewall (UTM-unified threat management)"^^xsd:string ;
        skos:broader         attr:attr-security-proactive-threat-vulnerability-management .
